# baseURI: https://w3id.org/isoprops
# imports: http://inf.bi.rub.de/ontology/dt
# prefix: isoprops

@prefix dc: <http://purl.org/dc/terms/> .
@prefix dcat: <http://www.w3.org/ns/dcat#> .
@prefix ex: <http://www.example.com/property#> .
@prefix isoprops: <https://w3id.org/isoprops#> .
@prefix opm: <https://w3id.org/opm#> .
@prefix owl: <http://www.w3.org/2002/07/owl#> .
@prefix qudt: <http://qudt.org/schema/qudt/> .
@prefix rdf: <http://www.w3.org/1999/02/22-rdf-syntax-ns#> .
@prefix rdfs: <http://www.w3.org/2000/01/rdf-schema#> .
@prefix schema: <https://schema.org/> .
@prefix sh: <http://www.w3.org/ns/shacl#> .
@prefix skos: <http://www.w3.org/2004/02/skos/core#> .
@prefix unit: <http://qudt.org/vocab/unit/> .
@prefix vann: <http://purl.org/vocab/vann/> .
@prefix voaf: <http://purl.org/vocommons/voaf#> .
@prefix xsd: <http://www.w3.org/2001/XMLSchema#> .

<http://inf.bi.rub.de/ontology/dt#hasExternalDictionaryReference>
  owl:equivalentProperty <http://inf.bi.rub.de/ontology/dt#hasExternalDictionaryReference> ;
.
dcat:accessURL
  rdf:type owl:AnnotationProperty ;
.
<https://w3id.org/isoprops>
  rdf:type owl:Ontology ;
  dc:created "2019-01-01"^^xsd:date ;
  dc:creator [
      rdf:type schema:Person ;
      schema:email <mailto:philipp.hagedorn-n6v@rub.de> ;
      schema:identifier <https://orcid.org/0000-0002-6249-243X> ;
      schema:memberOf [
          schema:identifier <https://www.inf.bi.ruhr-uni-bochum.de/iib/lehrstuhl/mitarbeiter/philipp_hagedorn.html.en> ;
          schema:name "Ruhr University Bochum" ;
        ] ;
      schema:name "Philipp Hagedorn" ;
    ] ;
  dc:creator [
      rdf:type schema:Person ;
      schema:email <mailto:sven.zentgraf@rub.de> ;
      schema:identifier <https://orcid.org/0000-0001-6058-7614> ;
      schema:memberOf [
          schema:identifier <https://www.inf.bi.ruhr-uni-bochum.de/iib/lehrstuhl/mitarbeiter/sven_zentgraf.html.en> ;
          schema:name "Ruhr University Bochum" ;
        ] ;
      schema:name "Sven Zentgraf" ;
    ] ;
  dc:issued "2021-12-06"^^xsd:date ;
  dc:license <https://creativecommons.org/licenses/by/4.0/> ;
  dc:modified "2024-04-24"^^xsd:date ;
  dc:publisher [
      rdf:type schema:Organization ;
      schema:identifier <https://www.inf.bi.rub.de> ;
      schema:name "Chair of Computing in Engineering, Ruhr University Bochum" ;
      schema:parentOrganization [
          rdf:type schema:Organization ;
          schema:name "Ruhr University Bochum, Germany" ;
        ] ;
    ] ;
  vann:preferredNamespacePrefix "isoprops" ;
  vann:preferredNamespaceUri <https://w3id.org/isoprops> ;
  rdfs:comment """The ISO Property (ISOProps) ontology maps the data model of the ISO 23386 for the describing, creating, and maintenance of properties in interconnected data dictionaries.

The namespace for ISOProps terms is [https://w3id.org/isoprops](https://w3id.org/isoprops)

The preferred prefix for the ISOProps namespace is `isoprops`.

## Ontology Overview 
![IDDO Ontology](Ontology_Overview.png \"Ontology\")

## Assigning an ISOProps Property to a Feature of Interest
![Property_Assignment](Property_Assignment.png \"Property_Assignment\")

## Relation between DCAT vocabulary and the ISOProps ontology
![DataCatalog_Overview](DataCatalog_Overview.png \"DataCatalog_Overview\")
""" ;
  rdfs:label "The ISO Property Ontology (ISOProps)" ;
  rdfs:seeAlso <https://www.iso.org/standard/75401.html> ;
  owl:imports <http://inf.bi.rub.de/ontology/dt> ;
  owl:versionIRI <https://w3id.org/isoprops> ;
  owl:versionInfo "v2.1" ;
  skos:example <https://rub-informatik-im-bauwesen.github.io/iddo/Ontology_Overview.png> ;
  

  skos:historyNote """
  v2.1: renamed from IDDO to ISOProps
  v2.0: update
  
  v0.3: dcat usage update 
  
  v0.2: ontology update 

v0.1: initial ontology for BIMSTRUCT project 
  """ ;
  schema:codeRepository <https://github.com/RUB-Informatik-im-Bauwesen/ir-ontologies/tree/main/isoprops> ;
.
isoprops:AssignedProperty
  rdf:type owl:Class ;
  rdfs:comment "Repraesentiert die Zweisung eines Merkmals und einer Merkmalszustandes an ein Feature of Interest (FOI)"@de-DE ;
  rdfs:comment "Represents the assignment of a property and a property state to a feature of interest (FOI)." ;
  rdfs:label "Assigned property" ;
  rdfs:label "Zugewiesenes Merkmal"@de-DE ;
  rdfs:subClassOf <http://www.w3id.org/opm#Property> ;
  rdfs:subClassOf [
      rdf:type owl:Restriction ;
      owl:cardinality 1 ;
      owl:onProperty isoprops:hasPropertyReference ;
    ] ;
  rdfs:subClassOf [
      rdf:type owl:Restriction ;
      owl:minCardinality 1 ;
      owl:onProperty <http://www.w3id.org/opm#hasPropertyState> ;
    ] ;
.
isoprops:BoundaryLimitMax
  rdf:type rdfs:Class ;
  rdfs:comment "Boundary limit  interval consisting of the the upper (maxValue) interval boundary" ;
  rdfs:comment "Grenzwertintervall bestehend aus der oberen(maxValue) Intervallgrenze"@de-DE ;
  rdfs:label "Maximum Boundary Limit" ;
  rdfs:label "Oberer Grenzwert"@de-DE ;
  rdfs:subClassOf owl:Thing ;
  rdfs:subClassOf schema:PropertyValue ;
  rdfs:subClassOf [
      rdf:type owl:Restriction ;
      owl:cardinality 1 ;
      owl:onProperty schema:value ;
    ] ;
  rdfs:subClassOf [
      rdf:type owl:Restriction ;
      owl:cardinality "1"^^xsd:nonNegativeInteger ;
      owl:onProperty isoprops:hasUnit ;
    ] ;
  rdfs:subClassOf [
      rdf:type owl:Restriction ;
      owl:onDataRange xsd:boolean ;
      owl:onProperty isoprops:Inclusive ;
      owl:qualifiedCardinality "1"^^xsd:nonNegativeInteger ;
    ] ;
  skos:scopeNote "PA040" ;
  isoprops:code "PA040" ;
  isoprops:code "PA040"@de-DE ;
.
isoprops:BoundaryLimitMin
  rdf:type rdfs:Class ;
  rdfs:comment "Boundary limit interval consisting of the lower(minValue) interval boundary" ;
  rdfs:comment "Grenzwertintervall bestehend aus der unteren(minValue) Intervallgrenze"@de-DE ;
  rdfs:label "Minimum Boundary Limit" ;
  rdfs:label "Unterer Grenzwert"@de-DE ;
  rdfs:subClassOf owl:Thing ;
  rdfs:subClassOf schema:PropertyValue ;
  rdfs:subClassOf [
      rdf:type owl:Restriction ;
      owl:cardinality 1 ;
      owl:onProperty schema:value ;
    ] ;
  rdfs:subClassOf [
      rdf:type owl:Restriction ;
      owl:cardinality "1"^^xsd:nonNegativeInteger ;
      owl:onProperty isoprops:hasUnit ;
    ] ;
  rdfs:subClassOf [
      rdf:type owl:Restriction ;
      owl:onDataRange xsd:boolean ;
      owl:onProperty isoprops:Inclusive ;
      owl:qualifiedCardinality "1"^^xsd:nonNegativeInteger ;
    ] ;
  skos:scopeNote "PA040" ;
  isoprops:code "PA040" ;
  isoprops:code "PA040"@de-DE ;
.
isoprops:BoundaryValue
  rdf:type rdfs:Class ;
  rdfs:comment "Paar (Liste von Grenzwert-Intervallen moeglicher Werte fuer das Merkmal, Einheit)"@de-DE ;
  rdfs:comment "Pair  (List of boundary intervals of possible values for the property, unit)" ;
  rdfs:label "Boundary values list" ;
  rdfs:label "Grenzwertliste"@de-DE ;
  rdfs:subClassOf owl:Thing ;
  rdfs:subClassOf [
      rdf:type owl:Restriction ;
      owl:maxQualifiedCardinality "1"^^xsd:nonNegativeInteger ;
      owl:onClass isoprops:BoundaryLimitMax ;
      owl:onProperty isoprops:hasBoundaryLimit ;
    ] ;
  rdfs:subClassOf [
      rdf:type owl:Restriction ;
      owl:maxQualifiedCardinality "1"^^xsd:nonNegativeInteger ;
      owl:onClass isoprops:BoundaryLimitMin ;
      owl:onProperty isoprops:hasBoundaryLimit ;
    ] ;
  skos:scopeNote "PA040" ;
  isoprops:code "PA040" ;
  isoprops:code "PA040"@de-DE ;
.
isoprops:CategoryOfGroupOfProperties
  rdf:type owl:DatatypeProperty ;
  rdfs:comment "Gibt die Kategorie der erstellten Merkmalsgruppe an"@de-DE ;
  rdfs:comment "Specifies the category of the created property group" ;
  rdfs:domain isoprops:GroupOfProperties ;
  rdfs:label "Category of group of properties" ;
  rdfs:label "Kategorie der Merkmalsgruppe"@de-DE ;
  rdfs:range [
      rdf:type rdfs:Datatype ;
      owl:oneOf (
          "Alternative use"
          "Class"
          "Composed property"
          "Domain"
          "Reference document"
        ) ;
    ] ;
  rdfs:subPropertyOf owl:topDataProperty ;
  skos:example "Alternative use" ;
  skos:example "Class" ;
  skos:example "Composed property" ;
  skos:example "Domain" ;
  skos:example "Reference document" ;
  skos:scopeNote "GA022" ;
  isoprops:code "GA022" ;
  isoprops:code "GA022"@de-DE ;
.
isoprops:CountryOfOrigin
  rdf:type owl:DatatypeProperty ;
  rdfs:comment "Country from where the requirement for this property/group of properties originated" ;
  rdfs:comment "Land, aus dem die Anforderung an dieses Merkmal/dieser Merkmalsgruppe stammt"@de-DE ;
  rdfs:domain isoprops:GroupOfProperties ;
  rdfs:domain isoprops:Property ;
  rdfs:label "Country of origin" ;
  rdfs:label "Ursprungsland"@de-DE ;
  rdfs:range xsd:string ;
  rdfs:subPropertyOf owl:topDataProperty ;
  skos:scopeNote "PA026/GA021" ;
  isoprops:code "PA026/GA021" ;
  isoprops:code "PA026/GA021"@de-DE ;
.
isoprops:CountryOfUse
  rdf:type owl:DatatypeProperty ;
  rdfs:comment "Country (group of countries, continent) in which the property is relevant for the market the stakeholders operate in" ;
  rdfs:comment "Land (Gruppe von Laendern, Kon-tinent), in dem das Merkmal/die Merkmalsgruppe fuer den Markt, auf dem die Beteiligten arbeiten, relevant ist"@de-DE ;
  rdfs:domain isoprops:GroupOfProperties ;
  rdfs:domain isoprops:Property ;
  rdfs:label "Country of use" ;
  rdfs:label "Land der Verwendung"@de-DE ;
  rdfs:range xsd:string ;
  rdfs:subPropertyOf owl:topDataProperty ;
  skos:scopeNote "PA024/GA019" ;
  isoprops:code "PA024/GA019" ;
  isoprops:code "PA024/GA019"@de-DE ;
.
isoprops:CreatorsLanguage
  rdf:type owl:DatatypeProperty ;
  rdfs:comment "Satz, der den Grund fuer die Ab-lehnung erlaeutert, der erklaeren kann, wie Werte umzurechnen sind, damit sie dem neuen Merkmal entsprechen; diese Er-laeuterung muss in internatio-nalem Englisch (EN) geschrieben werden"@de-DE ;
  rdfs:comment "Sentence explaining the reason of the deprecation, which can explain how to convert values to conform to the new property; this explanation has to be written in international English (EN)" ;
  rdfs:domain isoprops:GroupOfProperties ;
  rdfs:domain isoprops:Property ;
  rdfs:label "Creator's language" ;
  rdfs:label "Erlaeuterung fuer die Ablehnung"@de-DE ;
  rdfs:range xsd:string ;
  rdfs:subPropertyOf owl:topDataProperty ;
  skos:scopeNote "PA015/GA015" ;
  isoprops:code "PA015/GA015" ;
  isoprops:code "PA015/GA015"@de-DE ;
.
isoprops:DataType
  rdf:type owl:DatatypeProperty ;
  rdfs:comment """Format for expressing the value of the property
This can be understood as the storage type from a software perspective
In case of a dynamic property the value of this attribute is the datatype of the result of the calculation by the formula""" ;
  rdfs:comment """Format fuer die Angabe des Wertes des Merkmals
dies kann aus einer Soft-ware-Perspektive als Speiche-rungsart verstanden werden
im Falle eines dynamischen Merkmals ist der Wert dieses Attributs der Datentyp des Er-gebnisses der Berechnung mit der Gleichung"""@de-DE ;
  rdfs:domain isoprops:Property ;
  rdfs:label "Data type" ;
  rdfs:label "Datentyp (GUID)"@de-DE ;
  rdfs:range xsd:string ;
  rdfs:subPropertyOf owl:topDataProperty ;
  skos:scopeNote "PA030" ;
  isoprops:code "PA030" ;
  isoprops:code "PA030"@de-DE ;
.
isoprops:DateOfActivation
  rdf:type owl:DatatypeProperty ;
  rdfs:comment "Date after when the property can be used" ;
  rdfs:comment "Datum, nach dem das Merkmal verwendet werden kann"@de-DE ;
  rdfs:domain isoprops:GroupOfProperties ;
  rdfs:domain isoprops:Property ;
  rdfs:label "Date of activation" ;
  rdfs:label "Datum der Aktivierung"@de-DE ;
  rdfs:range xsd:dateTime ;
  rdfs:subPropertyOf owl:topDataProperty ;
  skos:scopeNote "PA04/GA04" ;
  isoprops:code "PA004/GA004" ;
  isoprops:code "PA004/GA004"@de-DE ;
.
isoprops:DateOfCreation
  rdf:type owl:DatatypeProperty ;
  rdfs:comment "Date of validation of the property creation request by experts" ;
  rdfs:comment "Datum der Validierung der An-frage zur Erstellung des Merkmals durch Sachverstaendige"@de-DE ;
  rdfs:domain isoprops:GroupOfProperties ;
  rdfs:domain isoprops:Property ;
  rdfs:label "Date of creation" ;
  rdfs:label "Datum der Erstellung"@de-DE ;
  rdfs:range xsd:dateTime ;
  rdfs:subPropertyOf owl:topDataProperty ;
  skos:scopeNote "PA003/GA003" ;
  isoprops:code "PA003/GA003" ;
  isoprops:code "PA003/GA003"@de-DE ;
.
isoprops:DateOfDeactivation
  rdf:type owl:DatatypeProperty ;
  rdfs:comment "Date of deactivation" ;
  rdfs:comment "Datum der Deaktivierung"@de-DE ;
  rdfs:domain isoprops:GroupOfProperties ;
  rdfs:domain isoprops:Property ;
  rdfs:label "Date of deactivation" ;
  rdfs:label "Datum der Deaktivierung"@de-DE ;
  rdfs:range xsd:dateTime ;
  rdfs:subPropertyOf owl:topDataProperty ;
  skos:scopeNote "PA008/GA008" ;
  isoprops:code "PA008/GA008" ;
  isoprops:code "PA008/GA008"@de-DE ;
.
isoprops:DateOfLastChange
  rdf:type owl:DatatypeProperty ;
  rdfs:comment "Date of validation of the last change request by experts" ;
  rdfs:comment "Datum der Validierung der letzten Aenderungsanfrage durch Sachverstaendige"@de-DE ;
  rdfs:domain isoprops:GroupOfProperties ;
  rdfs:domain isoprops:Property ;
  rdfs:label "Date of last change" ;
  rdfs:label "Datum der letzten Aenderung"@de-DE ;
  rdfs:range xsd:dateTime ;
  rdfs:subPropertyOf owl:topDataProperty ;
  skos:scopeNote "PA005/GA005" ;
  isoprops:code "PA005/GA005" ;
  isoprops:code "PA005/GA005"@de-DE ;
.
isoprops:DateOfRevision
  rdf:type owl:DatatypeProperty ;
  rdfs:comment "Date of revision" ;
  rdfs:comment "Datum der Ueberarbeitung"@de-DE ;
  rdfs:domain isoprops:GroupOfProperties ;
  rdfs:domain isoprops:Property ;
  rdfs:label "Date of revision" ;
  rdfs:label "Datum der Ueberarbeitung"@de-DE ;
  rdfs:range xsd:dateTime ;
  rdfs:subPropertyOf owl:topDataProperty ;
  skos:scopeNote "PA006/GA006" ;
  isoprops:code "PA006/GA006" ;
  isoprops:code "PA006/GA006"@de-DE ;
.
isoprops:DateOfVersion
  rdf:type owl:DatatypeProperty ;
  rdfs:comment "Date of version" ;
  rdfs:comment "Datum der Version"@de-DE ;
  rdfs:domain isoprops:GroupOfProperties ;
  rdfs:domain isoprops:Property ;
  rdfs:label "Date of version" ;
  rdfs:label "Datum der Version"@de-DE ;
  rdfs:range xsd:dateTime ;
  rdfs:subPropertyOf owl:topDataProperty ;
  skos:scopeNote "PA007/GA007" ;
  isoprops:code "PA007/GA007" ;
  isoprops:code "PA007/GA007"@de-DE ;
.
isoprops:DefiningValueItem
  rdf:type rdfs:Class ;
  rdfs:comment "Contains a defining value of an array in the form of a literal" ;
  rdfs:comment "Enthaelt einen definierenden Wert eines Arrays in Form eines Literals"@de-DE ;
  rdfs:label "Definierender Wert-Item"@de-DE ;
  rdfs:label "Defining value item" ;
  rdfs:subClassOf owl:Thing ;
  rdfs:subClassOf schema:PropertyValue ;
  rdfs:subClassOf [
      rdf:type owl:Restriction ;
      owl:cardinality 1 ;
      owl:onProperty schema:value ;
    ] ;
  skos:scopeNote "PA035" ;
  isoprops:code "PA035" ;
  isoprops:code "PA035"@de-DE ;
.
isoprops:DefiningValuesList
  rdf:type rdfs:Class ;
  rdfs:comment "Im Falle eines Feldes liefert dieses Attribut die definierenden Werte, sofern zutreffend, der Datentyp wird durch das Attribut PA030 angegeben"@de-DE ;
  rdfs:comment "In case of an array, this attribute provides the defining values when applicable, the datatype is given by the attribute PA030" ;
  rdfs:label "Defining values list" ;
  rdfs:label "Liste definierender Werte"@de-DE ;
  rdfs:subClassOf owl:Thing ;
  rdfs:subClassOf [
      rdf:type owl:Restriction ;
      owl:minCardinality 1 ;
      owl:onProperty isoprops:DefiningValueItem ;
    ] ;
  skos:scopeNote "PA035" ;
  isoprops:code "PA035" ;
  isoprops:code "PA035"@de-DE ;
.
isoprops:DefinitionInLanguage
  rdf:type owl:DatatypeProperty ;
  rdfs:comment "List of pairs (definition of the property/group of properties, language)" ;
  rdfs:comment "Liste von Paaren (Definition des Merkmals/der Merkmalsgruppe, Sprache)"@de-DE ;
  rdfs:domain isoprops:GroupOfProperties ;
  rdfs:domain isoprops:Property ;
  rdfs:label "Definition in Sprache N"@de-DE ;
  rdfs:label "Definition of in language N" ;
  rdfs:range rdf:langString ;
  rdfs:subPropertyOf owl:topDataProperty ;
  skos:scopeNote "PA016/GA016" ;
  isoprops:code "PA016/GA016" ;
  isoprops:code "PA016/GA016"@de-DE ;
.
isoprops:DeprecationExplanation
  rdf:type owl:DatatypeProperty ;
  rdfs:comment "Satz, der den Grund fuer die Ablehnung erlaeutert, der erklaeren kann, wie Werte umzurechnen sind, damit sie dem neuen Merkmal/der neuen Merkmalsgruppe entsprechen; diese Erlaeuterung muss in internationalem Englisch (EN) geschrieben werden"@de-DE ;
  rdfs:comment "Sentence explaining the reason of the deprecation, which can explain how to convert values to conform to the new property/group of properties; this explanation has to be written in international English (EN)" ;
  rdfs:domain isoprops:GroupOfProperties ;
  rdfs:domain isoprops:Property ;
  rdfs:label "Deprecation explanation" ;
  rdfs:label "Erlaeuterung fuer die Ablehnung"@de-DE ;
  rdfs:range rdf:langString ;
  rdfs:subPropertyOf owl:topDataProperty ;
  skos:scopeNote "PA013/GA013" ;
  isoprops:code "PA013/GA013" ;
  isoprops:code "PA013/GA013"@de-DE ;
.
isoprops:DescriptionInLanguage
  rdf:type owl:DatatypeProperty ;
  rdfs:comment "List of pairs (Description of the property, language)" ;
  rdfs:comment "Liste von Paaren (Beschreibung des Merkmals, Sprache)"@de-DE ;
  rdfs:domain isoprops:Property ;
  rdfs:label "Beschreibung in Sprache N"@de-DE ;
  rdfs:label "Description in language N" ;
  rdfs:range rdf:langString ;
  rdfs:subPropertyOf owl:topDataProperty ;
  skos:scopeNote "PA019" ;
  isoprops:code "PA019" ;
  isoprops:code "PA019"@de-DE ;
.
isoprops:Dictionary
  rdf:type owl:Class ;
  rdfs:comment "Centralized repository of information about data such as meaning, relationships to other data, origin, usage and format" ;
  rdfs:comment "Zentralisiertes Repository von Informationen ueber Daten, wie z. B. Bedeutung, Beziehungen zu anderen Daten, Ursprung, Verwendung und Format"@de-DE ;
  rdfs:label "Data dictionary" ;
  rdfs:label "Datenkatalog"@de-DE ;
  rdfs:subClassOf dcat:Catalog ;
  rdfs:subClassOf [
      rdf:type owl:Restriction ;
      owl:cardinality 1 ;
      owl:onProperty dc:description ;
    ] ;
  rdfs:subClassOf [
      rdf:type owl:Restriction ;
      owl:cardinality 1 ;
      owl:onProperty dc:identifier ;
    ] ;
  rdfs:subClassOf [
      rdf:type owl:Restriction ;
      owl:cardinality 1 ;
      owl:onProperty dc:issued ;
    ] ;
  rdfs:subClassOf [
      rdf:type owl:Restriction ;
      owl:cardinality 1 ;
      owl:onProperty dc:publisher ;
    ] ;
  rdfs:subClassOf [
      rdf:type owl:Restriction ;
      owl:cardinality 1 ;
      owl:onProperty dc:title ;
    ] ;
  rdfs:subClassOf [
      rdf:type owl:Restriction ;
      owl:cardinality 1 ;
      owl:onProperty dc:type ;
    ] ;
  rdfs:subClassOf [
      rdf:type owl:Restriction ;
      owl:minCardinality 1 ;
      owl:onProperty isoprops:hasDictionarySubset ;
    ] ;
.
isoprops:DictionaryReferenceDocument
  rdf:type owl:Class ;
  rdfs:comment "Publication that is consulted to find specific information, particularly in a technical or scientific domain" ;
  rdfs:comment "Publikation, die hinzugezogen wird, um bestimmte Informationen zu finden, insbesondere in einer technischen oder wissenschaftlichen Domaene"@de-DE ;
  rdfs:label "Reference document" ;
  rdfs:label "Referenzdokument"@de-DE ;
  rdfs:subClassOf dcat:Distribution ;
  rdfs:subClassOf [
      rdf:type owl:Restriction ;
      owl:cardinality 1 ;
      owl:onProperty isoprops:hasPropertyGroupReference ;
    ] ;
.
isoprops:DictionarySubset
  rdf:type owl:Class ;
  rdfs:comment "Defines a subset or subgrouping of a data catalog" ;
  rdfs:comment "Definiert eine Teilmenge oder Untergruppierung eines Datenkatalogs"@de-DE ;
  rdfs:label "Dictionary subset" ;
  rdfs:label "Teilmenge des Datenkatalogs"@de-DE ;
  rdfs:subClassOf dcat:Dataset ;
  rdfs:subClassOf [
      rdf:type owl:Restriction ;
      owl:cardinality 1 ;
      owl:onProperty dc:description ;
    ] ;
  rdfs:subClassOf [
      rdf:type owl:Restriction ;
      owl:cardinality 1 ;
      owl:onProperty dc:title ;
    ] ;
  rdfs:subClassOf [
      rdf:type owl:Restriction ;
      owl:cardinality 1 ;
      owl:onProperty dcat:accessURL ;
    ] ;
  rdfs:subClassOf [
      rdf:type owl:Restriction ;
      owl:cardinality 1 ;
      owl:onProperty isoprops:hasDictionaryReferenceDocument ;
    ] ;
.
isoprops:DigitalFormatItem
  rdf:type rdfs:Class ;
  rdfs:comment """Paar fuer den digitalen Texttyp (Praezision, Masseinheit)
Praezision ist die Anzahl signifikanter Stellen"""@de-DE ;
  rdfs:comment """Pair for digital text type (precision, unit)
Precision is the number of significant digits""" ;
  rdfs:label "Digital format item" ;
  rdfs:label "Digitales Format-Item"@de-DE ;
  rdfs:subClassOf owl:Thing ;
  rdfs:subClassOf [
      rdf:type owl:Restriction ;
      owl:onClass qudt:Unit ;
      owl:onProperty isoprops:hasUnit ;
      owl:qualifiedCardinality "1"^^xsd:nonNegativeInteger ;
    ] ;
  rdfs:subClassOf [
      rdf:type owl:Restriction ;
      owl:onDataRange xsd:decimal ;
      owl:onProperty isoprops:Precision ;
      owl:qualifiedCardinality 1 ;
    ] ;
  skos:scopeNote "PA037" ;
  isoprops:code "PA037" ;
  isoprops:code "PA037"@de-DE ;
.
isoprops:DynamicProperty
  rdf:type owl:DatatypeProperty ;
  rdfs:comment "If this is a dynamic property, the value is dependent on the parameters provided in the attribute PA032" ;
  rdfs:comment "Wenn es sich um ein dynamisches Merkmal handelt, haengt der Wert von den im Attribut PA032 bereitgestellten Parametern ab"@de-DE ;
  rdfs:label "Dynamic Property" ;
  rdfs:label "Dynamisches Merkmal"@de-DE ;
  rdfs:range [
      rdf:type rdfs:Datatype ;
      owl:oneOf (
          "yes"
          "no"
        ) ;
    ] ;
  rdfs:subPropertyOf owl:topDataProperty ;
  skos:example "no" ;
  skos:example "yes" ;
  skos:scopeNote "PA031" ;
  isoprops:code "PA031" ;
  isoprops:code "PA031"@de-DE ;
.
isoprops:Encoding
  rdf:type owl:DatatypeProperty ;
  rdfs:comment "Die Verschluesselung wird nach Name der Codierungsnorm von IANA, RFC 2978 festgelegt"@de-DE ;
  rdfs:comment "The encoding is set according to Name of encoding standard of IANA, RFC 2978" ;
  rdfs:domain isoprops:TextFormatItem ;
  rdfs:label "Encoding" ;
  rdfs:label "Kodierung"@de-DE ;
  rdfs:range xsd:string ;
  rdfs:subPropertyOf owl:topDataProperty ;
  skos:scopeNote "PA038" ;
  isoprops:code "PA038" ;
  isoprops:code "PA038"@de-DE ;
.
isoprops:ExampleInLanguage
  rdf:type owl:DatatypeProperty ;
  rdfs:comment "List of pairs (example of the property, language)" ;
  rdfs:comment "Liste von Paaren (Beispiel des Merkmals, Sprache)"@de-DE ;
  rdfs:domain isoprops:Property ;
  rdfs:label "Beispiel in Sprache N"@de-DE ;
  rdfs:label "Example in language N" ;
  rdfs:range rdf:langString ;
  rdfs:subPropertyOf owl:topDataProperty ;
  skos:scopeNote "PA019" ;
  isoprops:code "PA019" ;
  isoprops:code "PA019"@de-DE ;
.
isoprops:ExternalDictionaryReference
  rdf:type rdfs:Class ;
  rdfs:comment """Paar (interner Merkmalsbezeichner, entsprechender Datenkatalog-Bezeichner)
Dieses Attribut sollte fuer die Vertraeglichkeit zwischen bereits vorhandenen Merkmalen verwendet werden"""@de-DE ;
  rdfs:comment """Pair (property internal identifier, corresponding data dictionary identifier)
This attribute should be used for compatibility between already existing properties""" ;
  rdfs:label "External Dictionary Reference " ;
  rdfs:label "External Dictionary Reference"@de-DE ;
  rdfs:subClassOf owl:Thing ;
  rdfs:subClassOf [
      rdf:type owl:Restriction ;
      owl:cardinality "1"^^xsd:nonNegativeInteger ;
      owl:onProperty <http://inf.bi.rub.de/ontology/dt#hasExternalDictionary> ;
    ] ;
  rdfs:subClassOf [
      rdf:type owl:Restriction ;
      owl:cardinality "1"^^xsd:nonNegativeInteger ;
      owl:onProperty <http://inf.bi.rub.de/ontology/dt#hasExternalDictionaryProperty> ;
    ] ;
  owl:equivalentClass <http://inf.bi.rub.de/ontology/dt#ExternalDictionaryReference> ;
.
isoprops:GloballyUniqueIdentifier
  rdf:type owl:DatatypeProperty ;
  rdfs:comment "Eindeutiger Bezeichner, der mit dem in RFC 4122 beschriebenen Algorithmus erzeugt wird"@de-DE ;
  rdfs:comment "Unique identifier generated using the algorithm denoted in RFC 4122" ;
  rdfs:domain isoprops:GroupOfProperties ;
  rdfs:domain isoprops:Property ;
  rdfs:label "Global eindeutiger Bezeichner (GUID)"@de-DE ;
  rdfs:label "Globally Unique Identifier (GUID)" ;
  rdfs:range xsd:string ;
  rdfs:subPropertyOf owl:topDataProperty ;
  skos:scopeNote "PA001/GA001" ;
  isoprops:code "PA001/GA001" ;
  isoprops:code "PA001/GA001"@de-DE ;
.
isoprops:GroupOfProperties
  rdf:type owl:Class ;
  rdfs:comment "Collection enabling the properties to be prearranged or organized" ;
  rdfs:comment "Sammlung, die es ermoeglicht, die Merkmale vorauszuplanen oder zu organisieren"@de-DE ;
  rdfs:label "Group of properties" ;
  rdfs:label "Merkmalsgruppe"@de-DE ;
  rdfs:subClassOf <http://inf.bi.rub.de/ontology/dt#LibraryComponent> ;
  rdfs:subClassOf owl:Thing ;
  rdfs:subClassOf [
      rdf:type owl:Restriction ;
      owl:maxQualifiedCardinality 1 ;
      owl:onClass isoprops:GroupOfProperties ;
      owl:onProperty isoprops:hasParentGroupOfProperties ;
    ] ;
  rdfs:subClassOf [
      rdf:type owl:Restriction ;
      owl:maxQualifiedCardinality 1 ;
      owl:onDataRange xsd:string ;
      owl:onProperty isoprops:DeprecationExplanation ;
    ] ;
  rdfs:subClassOf [
      rdf:type owl:Restriction ;
      owl:minQualifiedCardinality 0 ;
      owl:onClass isoprops:GroupOfProperties ;
      owl:onProperty isoprops:hasParentGroupOfProperties ;
    ] ;
  rdfs:subClassOf [
      rdf:type owl:Restriction ;
      owl:minQualifiedCardinality 0 ;
      owl:onClass isoprops:GroupOfProperties ;
      owl:onProperty isoprops:isReplacedByGroupOfProperties ;
    ] ;
  rdfs:subClassOf [
      rdf:type owl:Restriction ;
      owl:minQualifiedCardinality 0 ;
      owl:onClass isoprops:GroupOfProperties ;
      owl:onProperty isoprops:replacesGroupOfProperties ;
    ] ;
  rdfs:subClassOf [
      rdf:type owl:Restriction ;
      owl:minQualifiedCardinality 0 ;
      owl:onDataRange xsd:dateTime ;
      owl:onProperty isoprops:DateOfActivation ;
    ] ;
  rdfs:subClassOf [
      rdf:type owl:Restriction ;
      owl:minQualifiedCardinality 0 ;
      owl:onDataRange xsd:dateTime ;
      owl:onProperty isoprops:DateOfDeactivation ;
    ] ;
  rdfs:subClassOf [
      rdf:type owl:Restriction ;
      owl:minQualifiedCardinality 0 ;
      owl:onDataRange xsd:dateTime ;
      owl:onProperty isoprops:DateOfLastChange ;
    ] ;
  rdfs:subClassOf [
      rdf:type owl:Restriction ;
      owl:minQualifiedCardinality 0 ;
      owl:onDataRange xsd:decimal ;
      owl:onProperty isoprops:Tolerance ;
    ] ;
  rdfs:subClassOf [
      rdf:type owl:Restriction ;
      owl:minQualifiedCardinality 0 ;
      owl:onDataRange xsd:string ;
      owl:onProperty isoprops:DeprecationExplanation ;
    ] ;
  rdfs:subClassOf [
      rdf:type owl:Restriction ;
      owl:minQualifiedCardinality 0 ;
      owl:onDataRange xsd:string ;
      owl:onProperty isoprops:SubdivisionOfUse ;
    ] ;
  rdfs:subClassOf [
      rdf:type owl:Restriction ;
      owl:minQualifiedCardinality "0"^^xsd:nonNegativeInteger ;
      owl:onClass isoprops:ExternalDictionaryReference ;
      owl:onProperty isoprops:hasExternalDictionaryReference ;
    ] ;
  rdfs:subClassOf [
      rdf:type owl:Restriction ;
      owl:minQualifiedCardinality 1 ;
      owl:onDataRange xsd:string ;
      owl:onProperty isoprops:CountryOfUse ;
    ] ;
  rdfs:subClassOf [
      rdf:type owl:Restriction ;
      owl:minQualifiedCardinality 1 ;
      owl:onDataRange xsd:string ;
      owl:onProperty isoprops:DefinitionInLanguage ;
    ] ;
  rdfs:subClassOf [
      rdf:type owl:Restriction ;
      owl:minQualifiedCardinality 1 ;
      owl:onDataRange xsd:string ;
      owl:onProperty isoprops:NameInLanguage ;
    ] ;
  rdfs:subClassOf [
      rdf:type owl:Restriction ;
      owl:minQualifiedCardinality 1 ;
      owl:onDataRange xsd:string ;
      owl:onProperty isoprops:VisualRepresentation ;
    ] ;
  rdfs:subClassOf [
      rdf:type owl:Restriction ;
      owl:onDataRange xsd:dateTime ;
      owl:onProperty isoprops:DateOfCreation ;
      owl:qualifiedCardinality 1 ;
    ] ;
  rdfs:subClassOf [
      rdf:type owl:Restriction ;
      owl:onDataRange xsd:dateTime ;
      owl:onProperty isoprops:DateOfRevision ;
      owl:qualifiedCardinality 1 ;
    ] ;
  rdfs:subClassOf [
      rdf:type owl:Restriction ;
      owl:onDataRange xsd:dateTime ;
      owl:onProperty isoprops:DateOfVersion ;
      owl:qualifiedCardinality 1 ;
    ] ;
  rdfs:subClassOf [
      rdf:type owl:Restriction ;
      owl:onDataRange xsd:integer ;
      owl:onProperty isoprops:RevisionNumber ;
      owl:qualifiedCardinality 1 ;
    ] ;
  rdfs:subClassOf [
      rdf:type owl:Restriction ;
      owl:onDataRange xsd:integer ;
      owl:onProperty isoprops:VersionNumber ;
      owl:qualifiedCardinality 1 ;
    ] ;
  rdfs:subClassOf [
      rdf:type owl:Restriction ;
      owl:onDataRange xsd:string ;
      owl:onDataRange [
          rdf:type rdfs:Datatype ;
          owl:oneOf (
              "active"
              "inactive"
            ) ;
        ] ;
      owl:onProperty isoprops:Status ;
      owl:qualifiedCardinality 1 ;
    ] ;
  rdfs:subClassOf [
      rdf:type owl:Restriction ;
      owl:onDataRange xsd:string ;
      owl:onProperty isoprops:CountryOfOrigin ;
      owl:qualifiedCardinality 1 ;
    ] ;
  rdfs:subClassOf [
      rdf:type owl:Restriction ;
      owl:onDataRange xsd:string ;
      owl:onProperty isoprops:CreatorsLanguage ;
      owl:qualifiedCardinality 1 ;
    ] ;
  rdfs:subClassOf [
      rdf:type owl:Restriction ;
      owl:onDataRange xsd:string ;
      owl:onProperty isoprops:GloballyUniqueIdentifier ;
      owl:qualifiedCardinality 1 ;
    ] ;
  rdfs:subClassOf [
      rdf:type owl:Restriction ;
      owl:onDataRange [
          rdf:type rdfs:Datatype ;
          owl:oneOf (
              "Alternative use"
              "Class"
              "Composed property"
              "Domain"
              "Reference document"
            ) ;
        ] ;
      owl:onProperty isoprops:CategoryOfGroupOfProperties ;
      owl:qualifiedCardinality 1 ;
    ] ;
.
isoprops:Inclusive
  rdf:type owl:DatatypeProperty ;
  rdfs:domain isoprops:BoundaryLimitMax ;
  rdfs:domain isoprops:BoundaryLimitMin ;
  rdfs:label "inclusive" ;
  rdfs:range xsd:boolean ;
  rdfs:subPropertyOf owl:topDataProperty ;
.
isoprops:MethodOfMeasurement
  rdf:type owl:DatatypeProperty ;
  rdfs:comment "Beurteilung von Bauprodukten, um ihre Tauglichkeit entsprechend den Anforderungen in harmonisierten technischen Spezifikationen sicherzustellen" ;
  rdfs:comment "Evaluation of construction products to ensure their fitness according to requirements in harmonised technical specifications" ;
  rdfs:domain isoprops:Property ;
  rdfs:label "Messverfahren"@de-DE ;
  rdfs:label "Method of measurement" ;
  rdfs:range xsd:string ;
  rdfs:subPropertyOf owl:topDataProperty ;
  skos:scopeNote "PA029" ;
  isoprops:code "PA029" ;
  isoprops:code "PA029"@de-DE ;
.
isoprops:NameInLanguage
  rdf:type owl:DatatypeProperty ;
  rdfs:comment """List of pairs (property name and language)
This attribute can be used to add synonyms for different domains""" ;
  rdfs:comment """Liste von Paaren (Name des Merkmals und Sprache)
Dieses Attribut kann verwendet werden, um Synonyme fuer verschiedene Domaenen hinzuzufuegen"""@de-DE ;
  rdfs:domain isoprops:GroupOfProperties ;
  rdfs:domain isoprops:Property ;
  rdfs:label "Name in Sprache N"@de-DE ;
  rdfs:label "Name in language N" ;
  rdfs:range rdf:langString ;
  rdfs:subPropertyOf owl:topDataProperty ;
  skos:scopeNote "PA016/GA016" ;
  isoprops:code "PA016/GA016" ;
  isoprops:code "PA016/GA016"@de-DE ;
.
isoprops:NameOfTheDefiningValues
  rdf:type owl:DatatypeProperty ;
  rdfs:comment "Im Falle eines Feldes liefert dieses Attribut die Namen der Spaltenkoepfe, festgelegt als Liste von Paaren (Name, Sprache)"@de-DE ;
  rdfs:comment "In case of an array, this attribute provides the names of the column headers defined as a list of pairs (name, language)" ;
  rdfs:label "Name der definierenden Werte"@de-DE ;
  rdfs:label "Names of the defining values" ;
  rdfs:range rdf:langString ;
  rdfs:subPropertyOf owl:topDataProperty ;
  skos:scopeNote "PA034" ;
  isoprops:code "PA034" ;
  isoprops:code "PA034"@de-DE ;
.
isoprops:NumberOfCharacters
  rdf:type owl:DatatypeProperty ;
  rdfs:comment "Die Verschluesselung wird nach Name der Codierungsnorm von IANA, RFC 2978 festgelegt"@de-DE ;
  rdfs:comment "The encoding is set according to Name of encoding standard of IANA, RFC 2978" ;
  rdfs:domain isoprops:TextFormatItem ;
  rdfs:label "Anzahl der Zeichen"@de-DE ;
  rdfs:label "Number of Characters" ;
  rdfs:range xsd:integer ;
  rdfs:subPropertyOf owl:topDataProperty ;
  skos:scopeNote "PA038" ;
  isoprops:code "PA038" ;
  isoprops:code "PA038"@de-DE ;
.
isoprops:PhysicalQuantity
  rdf:type rdfs:Class ;
  rdfs:comment """List of pairs (physical quantity | language)
Physical quantities are expressed in International System (SI) units
Non-physical quantities such as text are expressed with the value \"without\"
This is equivalent to a measure in ISO 16739-1 and ISO 10303
Only one physical quantity can be attached to a property. This attribute is used to provide the quantity in plain text with all the needed translations""" ;
  rdfs:comment """Liste von Paaren (physikalische Groesse | Sprache)
Physikalische Groessen werden in Einheiten des Internationalen Einheitensystems (SI) angegeben
nicht physikalische Groessen wie z. B. Text werden mit dem Wert \"ohne\" angegeben
dies ist gleichbedeutend mit einem Mass in ISO 16739-1 und ISO 10303
nur eine physikalische Groesse kann einem Merkmal zugeordnet werden. Dieses Attribut wird ver-wendet, um die Groesse in Klartext mit allen benoetigten ueberset-zungen bereitzustellen."""@de-DE ;
  rdfs:label "Physical quantity" ;
  rdfs:label "Physikalische Groesse"@de-DE ;
  rdfs:subClassOf <http://inf.bi.rub.de/ontology/dt#LibraryComponent> ;
  owl:equivalentClass qudt:QuantityKind ;
.
isoprops:PossibleValues
  rdf:type rdfs:Class ;
  rdfs:comment """Moeglicher Wert fuer das Merkmal und Sprache
Werte koennen String oder Zahlen sein"""@de-DE ;
  rdfs:comment """Possible value for the property and language
Values can be string or numbers""" ;
  rdfs:label "Liste moeglicher Werte in Sprache N"@de-DE ;
  rdfs:label "Possible value in language N" ;
  rdfs:subClassOf owl:Thing ;
  rdfs:subClassOf schema:PropertyValue ;
  rdfs:subClassOf [
      rdf:type owl:Restriction ;
      owl:cardinality 1 ;
      owl:onProperty schema:value ;
    ] ;
  owl:equivalentClass <http://inf.bi.rub.de/ontology/dt#PredefinedValuesList> ;
  skos:scopeNote "PA039" ;
  isoprops:code "PA039" ;
  isoprops:code "PA039"@de-DE ;
.
isoprops:Precision
  rdf:type owl:DatatypeProperty ;
  rdfs:comment "Praezision ist die Anzahl signifi-kanter Stellen"@de-DE ;
  rdfs:comment "Precision is the number of significant digits" ;
  rdfs:domain isoprops:DigitalFormatItem ;
  rdfs:label "Tolerance" ;
  rdfs:label "Toleranz"@de-DE ;
  rdfs:range xsd:decimal ;
  rdfs:subPropertyOf owl:topDataProperty ;
  skos:scopeNote "PA037" ;
  isoprops:code "PA037" ;
  isoprops:code "PA037"@de-DE ;
.
isoprops:Property
  rdf:type owl:Class ;
  rdfs:comment "Inhaerente oder erworbene Eigenschaft eines Datenelements"@de-DE ;
  rdfs:comment "Inherent or acquired feature of an item" ;
  rdfs:label "Merkmal"@de-DE ;
  rdfs:label "Property" ;
  rdfs:subClassOf <http://inf.bi.rub.de/ontology/dt#LibraryComponent> ;
  rdfs:subClassOf owl:Thing ;
  rdfs:subClassOf [
      rdf:type owl:Restriction ;
      owl:cardinality 1 ;
      owl:onProperty isoprops:CreatorsLanguage ;
    ] ;
  rdfs:subClassOf [
      rdf:type owl:Restriction ;
      owl:maxQualifiedCardinality 1 ;
      owl:onDataRange xsd:string ;
      owl:onProperty isoprops:CountryOfOrigin ;
    ] ;
  rdfs:subClassOf [
      rdf:type owl:Restriction ;
      owl:maxQualifiedCardinality 1 ;
      owl:onDataRange xsd:string ;
      owl:onProperty isoprops:DeprecationExplanation ;
    ] ;
  rdfs:subClassOf [
      rdf:type owl:Restriction ;
      owl:minQualifiedCardinality 0 ;
      owl:onClass isoprops:DefiningValuesList ;
      owl:onProperty isoprops:hasDefiningValue ;
    ] ;
  rdfs:subClassOf [
      rdf:type owl:Restriction ;
      owl:minQualifiedCardinality 0 ;
      owl:onClass isoprops:DigitalFormatItem ;
      owl:onProperty isoprops:hasDigitalFormat ;
    ] ;
  rdfs:subClassOf [
      rdf:type owl:Restriction ;
      owl:minQualifiedCardinality 0 ;
      owl:onClass isoprops:ExternalDictionaryReference ;
      owl:onProperty isoprops:hasExternalDictionaryReference ;
    ] ;
  rdfs:subClassOf [
      rdf:type owl:Restriction ;
      owl:minQualifiedCardinality 0 ;
      owl:onClass isoprops:PossibleValues ;
      owl:onProperty isoprops:hasPossibleValues ;
    ] ;
  rdfs:subClassOf [
      rdf:type owl:Restriction ;
      owl:minQualifiedCardinality 0 ;
      owl:onClass isoprops:Property ;
      owl:onProperty isoprops:hasConnectedProperty ;
    ] ;
  rdfs:subClassOf [
      rdf:type owl:Restriction ;
      owl:minQualifiedCardinality 0 ;
      owl:onClass isoprops:Property ;
      owl:onProperty isoprops:hasParameterOfTheDynamicProperty ;
    ] ;
  rdfs:subClassOf [
      rdf:type owl:Restriction ;
      owl:minQualifiedCardinality 0 ;
      owl:onClass isoprops:Property ;
      owl:onProperty isoprops:isReplacedByProperty ;
    ] ;
  rdfs:subClassOf [
      rdf:type owl:Restriction ;
      owl:minQualifiedCardinality 0 ;
      owl:onClass isoprops:Property ;
      owl:onProperty isoprops:replacesProperties ;
    ] ;
  rdfs:subClassOf [
      rdf:type owl:Restriction ;
      owl:minQualifiedCardinality 0 ;
      owl:onClass isoprops:SymbolOfTheProperty ;
      owl:onProperty isoprops:hasSymbolsOfTheProperty ;
    ] ;
  rdfs:subClassOf [
      rdf:type owl:Restriction ;
      owl:minQualifiedCardinality 0 ;
      owl:onClass isoprops:TextFormatItem ;
      owl:onProperty isoprops:hasTextFormat ;
    ] ;
  rdfs:subClassOf [
      rdf:type owl:Restriction ;
      owl:minQualifiedCardinality 0 ;
      owl:onDataRange xsd:dateTime ;
      owl:onProperty isoprops:DateOfActivation ;
    ] ;
  rdfs:subClassOf [
      rdf:type owl:Restriction ;
      owl:minQualifiedCardinality 0 ;
      owl:onDataRange xsd:dateTime ;
      owl:onProperty isoprops:DateOfDeactivation ;
    ] ;
  rdfs:subClassOf [
      rdf:type owl:Restriction ;
      owl:minQualifiedCardinality 0 ;
      owl:onDataRange xsd:dateTime ;
      owl:onProperty isoprops:DateOfLastChange ;
    ] ;
  rdfs:subClassOf [
      rdf:type owl:Restriction ;
      owl:minQualifiedCardinality 0 ;
      owl:onDataRange xsd:decimal ;
      owl:onProperty isoprops:Tolerance ;
    ] ;
  rdfs:subClassOf [
      rdf:type owl:Restriction ;
      owl:minQualifiedCardinality 0 ;
      owl:onDataRange xsd:string ;
      owl:onProperty isoprops:CountryOfOrigin ;
    ] ;
  rdfs:subClassOf [
      rdf:type owl:Restriction ;
      owl:minQualifiedCardinality 0 ;
      owl:onDataRange xsd:string ;
      owl:onProperty isoprops:DeprecationExplanation ;
    ] ;
  rdfs:subClassOf [
      rdf:type owl:Restriction ;
      owl:minQualifiedCardinality 0 ;
      owl:onDataRange xsd:string ;
      owl:onProperty isoprops:DescriptionInLanguage ;
    ] ;
  rdfs:subClassOf [
      rdf:type owl:Restriction ;
      owl:minQualifiedCardinality 0 ;
      owl:onDataRange xsd:string ;
      owl:onProperty isoprops:ExampleInLanguage ;
    ] ;
  rdfs:subClassOf [
      rdf:type owl:Restriction ;
      owl:minQualifiedCardinality 0 ;
      owl:onDataRange xsd:string ;
      owl:onProperty isoprops:MethodOfMeasurement ;
    ] ;
  rdfs:subClassOf [
      rdf:type owl:Restriction ;
      owl:minQualifiedCardinality 0 ;
      owl:onDataRange xsd:string ;
      owl:onProperty isoprops:NameOfTheDefiningValues ;
    ] ;
  rdfs:subClassOf [
      rdf:type owl:Restriction ;
      owl:minQualifiedCardinality 0 ;
      owl:onDataRange xsd:string ;
      owl:onProperty isoprops:SubdivisionOfUse ;
    ] ;
  rdfs:subClassOf [
      rdf:type owl:Restriction ;
      owl:minQualifiedCardinality 0 ;
      owl:onDataRange xsd:string ;
      owl:onProperty isoprops:VisualRepresentation ;
    ] ;
  rdfs:subClassOf [
      rdf:type owl:Restriction ;
      owl:minQualifiedCardinality 0 ;
      owl:onDataRange xsd:string ;
      owl:onProperty isoprops:hasPossibleValues ;
    ] ;
  rdfs:subClassOf [
      rdf:type owl:Restriction ;
      owl:minQualifiedCardinality 1 ;
      owl:onClass isoprops:GroupOfProperties ;
      owl:onProperty isoprops:hasGroupOfProperties ;
    ] ;
  rdfs:subClassOf [
      rdf:type owl:Restriction ;
      owl:minQualifiedCardinality 1 ;
      owl:onDataRange xsd:string ;
      owl:onProperty isoprops:CountryOfUse ;
    ] ;
  rdfs:subClassOf [
      rdf:type owl:Restriction ;
      owl:minQualifiedCardinality 1 ;
      owl:onDataRange xsd:string ;
      owl:onProperty isoprops:DefinitionInLanguage ;
    ] ;
  rdfs:subClassOf [
      rdf:type owl:Restriction ;
      owl:minQualifiedCardinality 1 ;
      owl:onDataRange xsd:string ;
      owl:onProperty isoprops:NameInLanguage ;
    ] ;
  rdfs:subClassOf [
      rdf:type owl:Restriction ;
      owl:minQualifiedCardinality "1"^^xsd:nonNegativeInteger ;
      owl:onClass qudt:Unit ;
      owl:onProperty isoprops:hasUnit ;
    ] ;
  rdfs:subClassOf [
      rdf:type owl:Restriction ;
      owl:minQualifiedCardinality "1"^^xsd:nonNegativeInteger ;
      owl:onDataRange qudt:QuantityKind ;
      owl:onProperty isoprops:hasPhysicalQuantity ;
    ] ;
  rdfs:subClassOf [
      rdf:type owl:Restriction ;
      owl:onClass isoprops:BoundaryValue ;
      owl:onProperty isoprops:hasBoundary ;
      owl:qualifiedCardinality 1 ;
    ] ;
  rdfs:subClassOf [
      rdf:type owl:Restriction ;
      owl:onDataRange xsd:dateTime ;
      owl:onProperty isoprops:DateOfCreation ;
      owl:qualifiedCardinality 1 ;
    ] ;
  rdfs:subClassOf [
      rdf:type owl:Restriction ;
      owl:onDataRange xsd:dateTime ;
      owl:onProperty isoprops:DateOfRevision ;
      owl:qualifiedCardinality 1 ;
    ] ;
  rdfs:subClassOf [
      rdf:type owl:Restriction ;
      owl:onDataRange xsd:dateTime ;
      owl:onProperty isoprops:DateOfVersion ;
      owl:qualifiedCardinality 1 ;
    ] ;
  rdfs:subClassOf [
      rdf:type owl:Restriction ;
      owl:onDataRange xsd:integer ;
      owl:onProperty isoprops:RevisionNumber ;
      owl:qualifiedCardinality 1 ;
    ] ;
  rdfs:subClassOf [
      rdf:type owl:Restriction ;
      owl:onDataRange xsd:integer ;
      owl:onProperty isoprops:VersionNumber ;
      owl:qualifiedCardinality 1 ;
    ] ;
  rdfs:subClassOf [
      rdf:type owl:Restriction ;
      owl:onDataRange xsd:string ;
      owl:onProperty isoprops:GloballyUniqueIdentifier ;
      owl:qualifiedCardinality 1 ;
    ] ;
  rdfs:subClassOf [
      rdf:type owl:Restriction ;
      owl:onDataRange [
          rdf:type rdfs:Datatype ;
          owl:oneOf (
              "BOOLEAN"
              "INTEGER"
              "RATIONAL"
              "REAL"
              "COMPLEX"
              "STRING"
              "DATETIME"
            ) ;
        ] ;
      owl:onProperty isoprops:DataType ;
      owl:qualifiedCardinality "1"^^xsd:nonNegativeInteger ;
    ] ;
  rdfs:subClassOf [
      rdf:type owl:Restriction ;
      owl:onDataRange [
          rdf:type rdfs:Datatype ;
          owl:oneOf (
              "active"
              "inactive"
            ) ;
        ] ;
      owl:onProperty isoprops:Status ;
      owl:qualifiedCardinality 1 ;
    ] ;
  rdfs:subClassOf [
      rdf:type owl:Restriction ;
      owl:onDataRange [
          rdf:type rdfs:Datatype ;
          owl:oneOf (
              "yes"
              "no"
            ) ;
        ] ;
      owl:onProperty isoprops:DynamicProperty ;
      owl:qualifiedCardinality 1 ;
    ] ;
  owl:equivalentClass opm:Property ;
.
isoprops:RevisionNumber
  rdf:type owl:DatatypeProperty ;
  rdfs:comment """Diese Nummer der ueberarbeitung ermoeglicht die Verfolgung kleinerer aenderungen, z. B. neue uebersetzung, Korrekturen von Tippfehlern: wenn sich die Versionsnummer aendert, beginnt die Nummer der ueberarbeitung wieder bei 1.
Sachverstaendige entscheiden, ob eine neue Nummer der ueberarbeitung angewendet werden kann oder ob eine neue ueberarbeitung erforderlich ist."""@de-DE ;
  rdfs:comment """This revision number allows tracking of minor changes e.g. new translation, changes of typos: if the version number changes, the revision number starts again at 1
Experts decide if a new revision number can be applied or if a new revision is needed""" ;
  rdfs:domain isoprops:GroupOfProperties ;
  rdfs:domain isoprops:Property ;
  rdfs:label "Nummer der ueberarbeitung"@de-DE ;
  rdfs:label "Revision number" ;
  rdfs:range xsd:integer ;
  rdfs:subPropertyOf owl:topDataProperty ;
  skos:scopeNote "PA010/GA010" ;
  isoprops:code "PA010/GA010" ;
  isoprops:code "PA010/GA010"@de-DE ;
.
isoprops:Status
  rdf:type owl:DatatypeProperty ;
  rdfs:comment "Status des Merkmals waehrend seines Lebenszyklus"@de-DE ;
  rdfs:comment "Status of the property during its life cycle" ;
  rdfs:domain isoprops:GroupOfProperties ;
  rdfs:domain isoprops:Property ;
  rdfs:label "Status" ;
  rdfs:label "Status"@de-DE ;
  rdfs:range [
      rdf:type rdfs:Datatype ;
      owl:oneOf (
          "active"
          "inactive"
        ) ;
    ] ;
  rdfs:subPropertyOf owl:topDataProperty ;
  skos:example "active" ;
  skos:example "inactive" ;
  skos:scopeNote "PA002/GA002" ;
  isoprops:code "PA002/GA002" ;
  isoprops:code "PA002/GA002"@de-DE ;
.
isoprops:SubdivisionOfUse
  rdf:type owl:DatatypeProperty ;
  rdfs:comment "Documented geographical region of use of the group of properties" ;
  rdfs:comment "Dokumentierte geographische Region, in der das Merkmal/ die Merkmalsgruppe verwendet wird"@de-DE ;
  rdfs:domain isoprops:GroupOfProperties ;
  rdfs:domain isoprops:Property ;
  rdfs:label "Subdivision of use" ;
  rdfs:label "Unterteilung der Verwendung"@de-DE ;
  rdfs:range xsd:string ;
  rdfs:subPropertyOf owl:topDataProperty ;
  skos:scopeNote "PA025/GA020" ;
  isoprops:code "PA025/GA020" ;
  isoprops:code "PA025/GA020"@de-DE ;
.
isoprops:Symbol
  rdf:type owl:DatatypeProperty ;
  rdfs:domain isoprops:SymbolOfTheProperty ;
  rdfs:label "Symbol" ;
  rdfs:label "Symbol"@de-DE ;
  rdfs:range xsd:string ;
  rdfs:subPropertyOf owl:topDataProperty ;
  skos:scopeNote "PA022" ;
  isoprops:code "PA022" ;
  isoprops:code "PA022"@de-DE ;
.
isoprops:SymbolOfTheProperty
  rdf:type rdfs:Class ;
  rdfs:comment "Paar (Symbol des Merkmals, global eindeutiger Bezeichner der Merkmalsgruppe (Attribut GA001))"@de-DE ;
  rdfs:comment "Pair (symbol of the property, globally unique identifier of the group of properties (attribute GA001))" ;
  rdfs:label "Symbol des Merkmals in einer gegebenen Merkmalsgruppe"@de-DE ;
  rdfs:label "Symbol of the property in a given property group" ;
  rdfs:subClassOf owl:Thing ;
  rdfs:subClassOf [
      rdf:type owl:Restriction ;
      owl:onClass isoprops:GroupOfProperties ;
      owl:onProperty isoprops:hasGivenGroupOfProperties ;
      owl:qualifiedCardinality 1 ;
    ] ;
  rdfs:subClassOf [
      rdf:type owl:Restriction ;
      owl:onDataRange xsd:string ;
      owl:onProperty isoprops:Symbol ;
      owl:qualifiedCardinality 1 ;
    ] ;
  skos:scopeNote "PA022" ;
  isoprops:code "PA022" ;
  isoprops:code "PA022"@de-DE ;
.
isoprops:TextFormatItem
  rdf:type rdfs:Class ;
  rdfs:comment """Paar fuer den Texttyp (Verschluesselung, Anzahl der Zeichen)
die Verschluesselung wird nach Name der Codierungsnorm von IANA, RFC 2978 festgelegt"""@de-DE ;
  rdfs:comment """Pair for text type (encoding, number of characters)
The encoding is set according to Name of encoding standard of IANA, RFC 2978""" ;
  rdfs:label "Text format item" ;
  rdfs:label "Textformat-Item"@de-DE ;
  rdfs:subClassOf owl:Thing ;
  rdfs:subClassOf [
      rdf:type owl:Restriction ;
      owl:onDataRange xsd:integer ;
      owl:onProperty isoprops:NumberOfCharacters ;
      owl:qualifiedCardinality 1 ;
    ] ;
  rdfs:subClassOf [
      rdf:type owl:Restriction ;
      owl:onDataRange xsd:string ;
      owl:onProperty isoprops:Encoding ;
      owl:qualifiedCardinality 1 ;
    ] ;
  skos:scopeNote "PA038" ;
  isoprops:code "PA038" ;
  isoprops:code "PA038"@de-DE ;
.
isoprops:Tolerance
  rdf:type owl:DatatypeProperty ;
  rdfs:comment "For numerical values; the total amount that a specific unit is permitted to vary; it is the difference between the maximum and the minimum limits for the unit" ;
  rdfs:comment "Fuer numerische Werte; der Gesamtbetrag, um den eine be-stimmte Einheit schwanken darf; sie ist die Differenz zwischen dem Hoechstwert und dem Mindestwert fuer die Einheit"@de-DE ;
  rdfs:domain isoprops:Property ;
  rdfs:label "Tolerance" ;
  rdfs:label "Toleranz"@de-DE ;
  rdfs:range xsd:decimal ;
  rdfs:subPropertyOf owl:topDataProperty ;
  skos:scopeNote "PA036" ;
  isoprops:code "PA036" ;
  isoprops:code "PA036"@de-DE ;
.
isoprops:VersionNumber
  rdf:type owl:DatatypeProperty ;
  rdfs:comment "Diese Versionsnummer ermoeglicht die Verfolgung groesserer aenderungen. Sachverstaendige entscheiden, ob eine neue Ver-sionsnummer angewendet werden muss."@de-DE ;
  rdfs:comment "This version number allows tracking of major changes. Experts decide if a new version number must be applied" ;
  rdfs:domain isoprops:GroupOfProperties ;
  rdfs:domain isoprops:Property ;
  rdfs:label "Version number" ;
  rdfs:label "Versionsnummer"@de-DE ;
  rdfs:range xsd:integer ;
  rdfs:subPropertyOf owl:topDataProperty ;
  skos:scopeNote "PA009/GA009" ;
  isoprops:code "PA009/GA009" ;
  isoprops:code "PA009/GA009"@de-DE ;
.
isoprops:VisualRepresentation
  rdf:type owl:DatatypeProperty ;
  rdfs:comment "Bildliche Darstellung des Merkmals durch Skizzen, Fotos, Videos oder sonstige Multimedia-Objekte"@de-DE ;
  rdfs:comment "Visual representation of the group of properties through sketches, photos, videos or other multimedia objects" ;
  rdfs:domain isoprops:GroupOfProperties ;
  rdfs:domain isoprops:Property ;
  rdfs:label "Bildliche Darstellung"@de-DE ;
  rdfs:label "Visual representation" ;
  rdfs:range xsd:string ;
  rdfs:subPropertyOf owl:topDataProperty ;
  skos:scopeNote "PA023/GA018" ;
  isoprops:code "PA023/GA018" ;
  isoprops:code "PA023/GA018"@de-DE ;
.
isoprops:code
  rdf:type rdf:Property ;
  rdf:type owl:AnnotationProperty ;
  rdfs:comment "Code that can be used to identify the attribute" ;
  rdfs:comment "Code, der zur Identifizierung des Attributs verwendet werden kann"@de-DE ;
  rdfs:domain rdfs:Resource ;
  rdfs:isDefinedBy rdfs: ;
  rdfs:label "Code" ;
  rdfs:label "Code"@de-DE ;
  rdfs:range rdfs:Literal ;
.
isoprops:hasBoundary
  rdf:type owl:ObjectProperty ;
  rdfs:comment "Paar (Liste von Grenzwert-Intervallen moeglicher Werte fuer das Merkmal, Einheit)"@de-DE ;
  rdfs:comment "Pair (list of boundary intervals of possible values for the property, unit)" ;
  rdfs:domain isoprops:Property ;
  rdfs:label "Boundary values" ;
  rdfs:label "Grenzwerte"@de-DE ;
  rdfs:range isoprops:BoundaryValue ;
  rdfs:subPropertyOf owl:topObjectProperty ;
  skos:scopeNote "PA040" ;
  isoprops:code "PA040" ;
  isoprops:code "PA040"@de-DE ;
.
isoprops:hasBoundaryLimit
  rdf:type owl:ObjectProperty ;
  rdfs:comment "Einzelnes Grenzwertintervall"@de-DE ;
  rdfs:comment "Single Boundary value interval" ;
  rdfs:domain isoprops:BoundaryValue ;
  rdfs:label "Boundary value" ;
  rdfs:label "Grenzwert"@de-DE ;
  rdfs:range isoprops:BoundaryLimitMin ;
  rdfs:subPropertyOf owl:topObjectProperty ;
  skos:scopeNote "PA040" ;
  isoprops:code "PA040" ;
  isoprops:code "PA040"@de-DE ;
.
isoprops:hasConnectedProperty
  rdf:type owl:ObjectProperty ;
  rdfs:comment "List of the globally unique identifier of the connected properties (attribute PA001); the value of one property is related to the values of the other ones. For example, a sound absorption coefficient is given for a specific frequency, in this case sound absorption and frequency are connected properties" ;
  rdfs:comment "Liste der global eindeutigen Bezeichner der verbundenen Merkmale (Attribut PA001); der Wert eines Merkmals steht zu den Werten der anderen in einer Beziehung. Beispielsweise ist ein Schallabsorptionsgrad fuer eine bestimmte Frequenz gegeben, in diesem Fall sind Schallabsorp-tionsgrad und Frequenz ver-bundene Merkmale."@de-DE ;
  rdfs:domain isoprops:Property ;
  rdfs:label "Connected properties" ;
  rdfs:label "Verbundene Merkmale"@de-DE ;
  rdfs:range isoprops:Property ;
  rdfs:subPropertyOf owl:topObjectProperty ;
  skos:scopeNote "PA020" ;
  isoprops:code "PA020" ;
  isoprops:code "PA020"@de-DE ;
.
isoprops:hasDefiningValue
  rdf:type owl:ObjectProperty ;
  rdfs:comment "Im Falle eines Feldes liefert dieses Attribut die definierenden Werte, sofern zutreffend, der Datentyp wird durch das Attribut PA030 angegeben"@de-DE ;
  rdfs:comment "In case of an array, this attribute provides the defining values when applicable, the datatype is given by the attribute PA030" ;
  rdfs:domain isoprops:Property ;
  rdfs:label "Definierende Werte"@de-DE ;
  rdfs:label "Defining values" ;
  rdfs:range isoprops:DefiningValuesList ;
  rdfs:subPropertyOf owl:topObjectProperty ;
  skos:scopeNote "PA035" ;
  isoprops:code "PA035" ;
  isoprops:code "PA035"@de-DE ;
.
isoprops:hasDefiningValueItem
  rdf:type owl:ObjectProperty ;
  rdfs:comment "Contains a defining value of an array" ;
  rdfs:comment "Enthaelt einen definierenden Wert eines Arrays"@de-DE ;
  rdfs:domain isoprops:DefiningValuesList ;
  rdfs:label "Definierender Wert"@de-DE ;
  rdfs:label "Defining value" ;
  rdfs:range isoprops:DefiningValueItem ;
  rdfs:subPropertyOf owl:topObjectProperty ;
  skos:scopeNote "PA035" ;
  isoprops:code "PA035" ;
  isoprops:code "PA035"@de-DE ;
.
isoprops:hasDictionaryReferenceDocument
  rdf:type owl:ObjectProperty ;
  rdfs:domain isoprops:DictionarySubset ;
  rdfs:label "has relation to a reference document" ;
  rdfs:label "hat den Verweis auf ein Referenzdokument"@de-DE ;
  rdfs:range isoprops:DictionaryReferenceDocument ;
  rdfs:subPropertyOf dcat:distribution ;
.
isoprops:hasDictionarySubset
  rdf:type owl:ObjectProperty ;
  rdfs:domain isoprops:Dictionary ;
  rdfs:label "has dictionary subset" ;
  rdfs:label "hat Teilmenge eines Katalogs"@de-DE ;
  rdfs:range isoprops:DictionarySubset ;
  rdfs:subPropertyOf dcat:dataset ;
.
isoprops:hasDigitalFormat
  rdf:type owl:ObjectProperty ;
  rdfs:comment """Paar fuer den digitalen Texttyp (Praezision, Masseinheit)
Praezision ist die Anzahl signifikanter Stellen"""@de-DE ;
  rdfs:comment """Pair for digital text type (precision, unit)
Precision is the number of significant digits""" ;
  rdfs:domain isoprops:Property ;
  rdfs:label "Digital format" ;
  rdfs:label "Digitales Format"@de-DE ;
  rdfs:range isoprops:DigitalFormatItem ;
  rdfs:subPropertyOf owl:topObjectProperty ;
  skos:scopeNote "PA037" ;
  isoprops:code "PA037" ;
  isoprops:code "PA037"@de-DE ;
.
isoprops:hasExternalDictionary
  rdf:type owl:ObjectProperty ;
  rdfs:label "has external dictionary" ;
  rdfs:subPropertyOf owl:topObjectProperty ;
  owl:equivalentProperty <http://inf.bi.rub.de/ontology/dt#hasExternalDictionary> ;
.
isoprops:hasExternalDictionaryProperty
  rdf:type owl:ObjectProperty ;
  rdfs:label "has external dictionary property" ;
  rdfs:subPropertyOf owl:topObjectProperty ;
  owl:equivalentProperty <http://inf.bi.rub.de/ontology/dt#hasExternalDictionaryProperty> ;
.
isoprops:hasExternalDictionaryReference
  rdf:type owl:ObjectProperty ;
  rdfs:comment """List of pairs (property internal identifier, corresponding data dictionary identifier)
This attribute should be used for compatibility between already existing properties""" ;
  rdfs:comment """Liste von Paaren (interner Merk-malsbezeichner, entsprechender Datenkatalog-Bezeichner)
dieses Attribut sollte fuer die Vertraeglichkeit zwischen bereits vorhandenen Merkmalen verwendet werden"""@de-DE ;
  rdfs:domain isoprops:GroupOfProperties ;
  rdfs:domain isoprops:Property ;
  rdfs:label "has External Dictionary Reference" ;
  rdfs:label "hat externe Dictionary Referenz"@de-DE ;
  rdfs:range isoprops:ExternalDictionaryReference ;
  rdfs:subPropertyOf owl:topObjectProperty ;
  skos:scopeNote "GA014" ;
  skos:scopeNote "PA014" ;
  isoprops:code "GA014" ;
  isoprops:code "GA014"@de-DE ;
  isoprops:code "PA014" ;
  isoprops:code "PA014"@de-DE ;
.
isoprops:hasGivenGroupOfProperties
  rdf:type owl:ObjectProperty ;
  rdfs:comment "Global eindeutiger Bezeichner einer Merkmalsgruppe (Attribut GA001) fuer das dem Merkmal zugeordnetem Symbol"@de-DE ;
  rdfs:comment "Globally unique identifier of a group of properties (attribute GA001) for the symbol assigned to the property." ;
  rdfs:domain isoprops:Property ;
  rdfs:label "Gegebene Merkmalsgruppe"@de-DE ;
  rdfs:label "Given group of properties" ;
  rdfs:range isoprops:GroupOfProperties ;
  rdfs:subPropertyOf owl:topObjectProperty ;
  skos:scopeNote "PA022" ;
  isoprops:code "PA022" ;
  isoprops:code "PA022"@de-DE ;
.
isoprops:hasGroupOfProperties
  rdf:type owl:ObjectProperty ;
  rdfs:comment "List of globally unique identifiers of groups of properties (attribute GA001) to which the property is attached" ;
  rdfs:comment "Liste von global eindeutigen Bezeichnern von Merkmalsgruppen (Attribut GA001), denen das Merkmal angehoert"@de-DE ;
  rdfs:domain isoprops:Property ;
  rdfs:label "Group(s) of properties" ;
  rdfs:label "Merkmalsgruppe(n)"@de-DE ;
  rdfs:range isoprops:GroupOfProperties ;
  rdfs:subPropertyOf owl:topObjectProperty ;
  skos:scopeNote "PA021" ;
  isoprops:code "PA021" ;
  isoprops:code "PA021"@de-DE ;
.
isoprops:hasParameterOfTheDynamicProperty
  rdf:type owl:ObjectProperty ;
  rdfs:comment "List of GUIDS of properties which are parameters of the function for a dynamic property" ;
  rdfs:comment "Liste von GUIDs von Merkmalen, welche Parameter der Funktion fuer ein dynamisches Merkmal sind"@de-DE ;
  rdfs:domain isoprops:Property ;
  rdfs:label "Parameter des dynamischen Merkmals"@de-DE ;
  rdfs:label "Parameters of the dynamic property" ;
  rdfs:range isoprops:Property ;
  rdfs:subPropertyOf owl:topObjectProperty ;
  skos:scopeNote "PA032" ;
  isoprops:code "GA032"@de-DE ;
  isoprops:code "PA032" ;
.
isoprops:hasParentGroupOfProperties
  rdf:type owl:ObjectProperty ;
  rdfs:comment """Enables a sub-group to be linked to a parent group via their globally unique identifiers (attribute GA001)
Any property attached to a group is inherited by the sub-group(s)""" ;
  rdfs:comment """Ermoeglicht die Ver-knuepfung einer Unter-gruppe mit einer ueber-geordneten Gruppe ueber ihre global ein-deutigen Bezeichner (Attribut GA001)
jedes einer Gruppe zugehoerige Merkmal wird von der/den Untergruppe(n) uebernommen"""@de-DE ;
  rdfs:domain isoprops:GroupOfProperties ;
  rdfs:label "Parent group of properties" ;
  rdfs:label "uebergeordnete Merkmalsgruppe"@de-DE ;
  rdfs:range isoprops:GroupOfProperties ;
  rdfs:subPropertyOf owl:topObjectProperty ;
  skos:scopeNote "GA023" ;
  isoprops:code "GA023" ;
  isoprops:code "GA023"@de-DE ;
.
isoprops:hasPhysicalQuantity
  rdf:type owl:ObjectProperty ;
  rdfs:comment """List of pairs (physical quantity | language)
Physical quantities are expressed in International System (SI) units
Non-physical quantities such as text are expressed with the value \"without\" --> http://qudt.org/vocab/quantitykind/Dimensionless
This is equivalent to a measure in ISO 16739-1 and ISO 10303
Only one physical quantity can be attached to a property. This attribute is used to provide the quantity in plain text with all the needed translations""" ;
  rdfs:comment """Liste von Paaren (physikalische Groesse | Sprache)
Physikalische Groessen werden in Einheiten des Internationalen Einheitensystems (SI) angegeben
nicht physikalische Groessen wie z. B. Text werden mit dem Wert \"ohne\" angegeben --> http://qudt.org/vocab/quantitykind/Dimensionless
dies ist gleichbedeutend mit einem Mass in ISO 16739-1 und ISO 10303
nur eine physikalische Groesse kann einem Merkmal zugeordnet werden. Dieses Attribut wird ver-wendet, um die Groesse in Klartext mit allen benoetigten ueberset-zungen bereitzustellen."""@de-DE ;
  rdfs:domain isoprops:Property ;
  rdfs:label "Physical quantity" ;
  rdfs:label "Physikalische Groesse"@de-DE ;
  rdfs:range qudt:QuantityKind ;
  rdfs:seeAlso <http://qudt.org/vocab/quantitykind> ;
  rdfs:subPropertyOf owl:topObjectProperty ;
  skos:scopeNote "PA027" ;
  isoprops:code "PA027" ;
  isoprops:code "PA027"@de-DE ;
.
isoprops:hasPossibleValues
  rdf:type owl:ObjectProperty ;
  rdfs:comment """List of pairs (possible value for the property and language)
Values can be string or numbers""" ;
  rdfs:comment """Liste von Paaren (moeglicher Wert fuer das Merkmal und Sprache)
Werte koennen String oder Zahlen sein"""@de-DE ;
  rdfs:domain isoprops:Property ;
  rdfs:label "List of possible values in language N" ;
  rdfs:label "Liste moeglicher Werte in Sprache N"@de-DE ;
  rdfs:range isoprops:PossibleValues ;
  rdfs:subPropertyOf owl:topObjectProperty ;
  skos:scopeNote "PA039" ;
  isoprops:code "PA039" ;
  isoprops:code "PA039"@de-DE ;
.
isoprops:hasProperty
  rdf:type owl:ObjectProperty ;
  rdfs:comment "Attaches a property to a feature of interest (FOI)" ;
  rdfs:comment "Fuegt ein Merkmal zu einem Feature of Interest (FOI) hinzu"@de-DE ;
  rdfs:label "has property" ;
  rdfs:label "hat Merkmal"@de-DE ;
  rdfs:range isoprops:AssignedProperty ;
  rdfs:subPropertyOf owl:topObjectProperty ;
.
isoprops:hasPropertyGroupReference
  rdf:type owl:ObjectProperty ;
  rdfs:comment "Attaches a property group reference to a isoprops:ReferenceDocument" ;
  rdfs:comment "Fuegt eine Merkmalsgruppe (oberstes in der Hierarchie) zu einer isoprops:ReferenceDocument hinzu"@de-DE ;
  rdfs:domain isoprops:ReferenceDocument ;
  rdfs:label "has property group reference" ;
  rdfs:label "hat Merkmalsgruppenreferenz"@de-DE ;
  rdfs:range isoprops:GroupOfProperties ;
  rdfs:subPropertyOf owl:topObjectProperty ;
  rdfs:subPropertyOf dcat:distribution ;
.
isoprops:hasPropertyReference
  rdf:type owl:ObjectProperty ;
  rdfs:comment "Attaches a property reference to a property assignment" ;
  rdfs:comment "Fuegt ein Merkmal zu einer Merkmalszuweisung hinzu"@de-DE ;
  rdfs:domain isoprops:AssignedProperty ;
  rdfs:label "has Property Reference" ;
  rdfs:label "hat Merkmalreferenz"@de-DE ;
  rdfs:range isoprops:Property ;
  rdfs:subPropertyOf owl:topObjectProperty ;
.
isoprops:hasRelationOfTheGroupOfPropertiesIdentifiersInTheInterconnectedDataDictionaries
  rdf:type owl:ObjectProperty ;
  rdfs:comment """List of pairs (group of properties internal identifier, corresponding data dictionary identifier)
This attribute should be used for compatibility between already existing groups of properties""" ;
  rdfs:comment """Liste von Paaren (inter-ner Bezeichner der Merkmalsgruppe, ent-sprechender Daten-katalog-Bezeichner)
dieses Attribut sollte fuer die Kompatibilitaet zwischen bereits vorhandenen Merk-malsgruppen verwen-det werden"""@de-DE ;
  rdfs:domain isoprops:GroupOfProperties ;
  rdfs:label "Beziehung der Bezeichner der Merkmalsgruppe in den miteinander verbundenen Datenkatalogen"@de-DE ;
  rdfs:label "Relations of the group of properties identifiers in the interconnected data dictionaries" ;
  rdfs:subPropertyOf owl:topObjectProperty ;
  skos:scopeNote "GA014" ;
  isoprops:code "GA014" ;
  isoprops:code "GA014"@de-DE ;
.
isoprops:hasSymbolsOfTheProperty
  rdf:type owl:ObjectProperty ;
  rdfs:comment "List of pairs (symbol of the property, globally unique identifier of the group of properties (attribute GA001))" ;
  rdfs:comment "Liste von Paaren (Symbol des Merkmals, global eindeutiger Bezeichner der Merkmalsgruppe (Attribut GA001))"@de-DE ;
  rdfs:domain isoprops:Property ;
  rdfs:label "Symbole des Merkmals in einer gegebenen Merk-malsgruppe"@de-DE ;
  rdfs:label "Symbols of the property in a given property group" ;
  rdfs:range isoprops:SymbolOfTheProperty ;
  rdfs:subPropertyOf owl:topObjectProperty ;
  skos:scopeNote "PA022" ;
  isoprops:code "PA022" ;
  isoprops:code "PA022"@de-DE ;
.
isoprops:hasTextFormat
  rdf:type owl:ObjectProperty ;
  rdfs:comment """Paar fuer den Texttyp (Verschluesselung, Anzahl der Zeichen)
die Verschluesselung wird nach Name der Codierungsnorm von IANA, RFC 2978 festgelegt"""@de-DE ;
  rdfs:comment """Pair for text type (encoding, number of characters)
The encoding is set according to Name of encoding standard of IANA, RFC 2978""" ;
  rdfs:domain isoprops:Property ;
  rdfs:label "Text format" ;
  rdfs:label "Textformat"@de-DE ;
  rdfs:range isoprops:TextFormatItem ;
  rdfs:subPropertyOf owl:topObjectProperty ;
  skos:scopeNote "PA038" ;
  isoprops:code "PA038" ;
  isoprops:code "PA038"@de-DE ;
.
isoprops:hasUnit
  rdf:type owl:ObjectProperty ;
  rdfs:comment """A unit to represent a scale that enables a value to be measured
It is possible to use this attribute to explain there is no unit attached to the property by using unitless --> http://qudt.org/vocab/unit/UNITLESS""" ;
  rdfs:comment """Eine Einheit zur Darstellung einer Skala, die es ermoeglicht, einen Wert zu messen
es ist moeglich, dieses Attribut zu verwenden, um zu erlaeutern, dass dem Merkmal keine Einheit zugeordnet ist, indem einheitslos verwendet wird --> http://qudt.org/vocab/unit/UNITLESS"""@de-DE ;
  rdfs:domain isoprops:BoundaryLimitMax ;
  rdfs:domain isoprops:BoundaryLimitMin ;
  rdfs:domain isoprops:Property ;
  rdfs:label "has unit" ;
  rdfs:label "hat Einheit"@de-DE ;
  rdfs:range qudt:Unit ;
  rdfs:seeAlso unit:UNITLESS ;
  rdfs:subPropertyOf owl:topObjectProperty ;
  skos:scopeNote "PA033" ;
  isoprops:code "PA033" ;
  isoprops:code "PA033"@de-DE ;
.
isoprops:isReplacedByGroupOfProperties
  rdf:type owl:ObjectProperty ;
  rdfs:comment "List of globally unique identifiers of the replacing groups of properties" ;
  rdfs:comment "Liste von globalen Bezeichnern fuer die ersetzenden Merkmalsgruppen"@de-DE ;
  rdfs:domain isoprops:GroupOfProperties ;
  rdfs:label "List of replacing groups of properties" ;
  rdfs:label "Liste ersetzender Merkmalsgruppen"@de-DE ;
  rdfs:range isoprops:GroupOfProperties ;
  rdfs:subPropertyOf owl:topObjectProperty ;
  owl:inverseOf isoprops:replacesGroupOfProperties ;
  skos:scopeNote "GA012" ;
  isoprops:code "GA012" ;
  isoprops:code "GA012"@de-DE ;
.
isoprops:isReplacedByProperty
  rdf:type owl:ObjectProperty ;
  rdfs:comment "Globally unique identifier (attribute PA001) of the replacing property (or properties)" ;
  rdfs:comment "global eindeutiger Bezeichner (Attribut PA001) des ersetzenden Merkmals (oder der Merkmale)"@de-DE ;
  rdfs:domain isoprops:Property ;
  rdfs:label "List of replacing properties" ;
  rdfs:label "Liste ersetzender Merkmale"@de-DE ;
  rdfs:range isoprops:Property ;
  rdfs:subPropertyOf owl:topObjectProperty ;
  owl:inverseOf isoprops:replacesProperties ;
  skos:scopeNote "PA012" ;
  isoprops:code "PA012" ;
  isoprops:code "PA012"@de-DE ;
.
isoprops:replacesGroupOfProperties
  rdf:type owl:ObjectProperty ;
  rdfs:comment "List of globally unique identifiers of the replaced groups of properties" ;
  rdfs:comment "Liste von globalen Bezeichnern fuer die ersetzten Merk-malsgruppen"@de-DE ;
  rdfs:domain isoprops:GroupOfProperties ;
  rdfs:label "List of replaced groups of properties" ;
  rdfs:label "Liste ersetzter Merkmalsgruppen"@de-DE ;
  rdfs:range isoprops:GroupOfProperties ;
  rdfs:subPropertyOf owl:topObjectProperty ;
  owl:inverseOf isoprops:isReplacedByGroupOfProperties ;
  skos:scopeNote "GA011" ;
  isoprops:code "GA011" ;
  isoprops:code "GA011"@de-DE ;
.
isoprops:replacesProperties
  rdf:type owl:ObjectProperty ;
  rdfs:comment "Global eindeutiger Bezeichner des ersetzten Merkmals (oder der Merkmale)"@de-DE ;
  rdfs:comment "Globally unique identifier of the replaced property (or properties)" ;
  rdfs:domain isoprops:Property ;
  rdfs:label "List of replaced properties" ;
  rdfs:label "Liste ersetzter Merkmale"@de-DE ;
  rdfs:range isoprops:Property ;
  rdfs:subPropertyOf owl:topObjectProperty ;
  owl:inverseOf isoprops:isReplacedByProperty ;
  skos:scopeNote "PA011" ;
  isoprops:code "PA011" ;
  isoprops:code "PA011"@de-DE ;
.
