<?xml version="1.0"?>
<rdf:RDF
    xmlns:Container="https://standards.iso.org/iso/21597/-1/ed-1/en/Container#"
    xmlns:rdf="http://www.w3.org/1999/02/22-rdf-syntax-ns#"
    xmlns:schema="https://schema.org/"
    xmlns:vs="http://www.w3.org/2003/06/sw-vocab-status/ns#"
    xmlns:icdd4loin="https://w3id.org/loin/v2/icdd#"
    xmlns:Linkset="https://standards.iso.org/iso/21597/-1/ed-1/en/Linkset#"
    xmlns:foaf="http://xmlns.com/foaf/0.1#"
    xmlns:rdfs="http://www.w3.org/2000/01/rdf-schema#"
    xmlns:dc="http://purl.org/dc/terms/"
    xmlns:dt="https://w3id.org/dt#"
    xmlns:owl="http://www.w3.org/2002/07/owl#"
    xmlns:ids4loin="https://w3id.org/loin/v2/ids#"
    xmlns:loin="https://w3id.org/loin#"
    xmlns:j.0="http://www.w3.org/2004/02/skos/core#"
    xmlns:sh="http://www.w3.org/ns/shacl#"
    xmlns:vann="http://purl.org/vocab/vann/"
    xmlns:xsd="http://www.w3.org/2001/XMLSchema#"
  xml:base="https://w3id.org/loin" > 
  <rdf:Description rdf:about="#LevelOfInformationNeed">
    <rdfs:subClassOf rdf:nodeID="A0"/>
    <rdfs:subClassOf rdf:resource="http://www.w3.org/2002/07/owl#Thing"/>
    <rdfs:label xml:lang="en">Level Of Information Need</rdfs:label>
    <rdfs:comment xml:lang="en">Level of Information Need as defined by ISO 7817</rdfs:comment>
    <rdf:type rdf:resource="http://www.w3.org/2002/07/owl#Class"/>
  </rdf:Description>
  <rdf:Description rdf:nodeID="A1">
    <rdf:rest rdf:nodeID="A2"/>
    <rdf:first>L2</rdf:first>
  </rdf:Description>
  <rdf:Description rdf:nodeID="A3">
    <rdf:rest rdf:nodeID="A4"/>
    <rdf:first>D1</rdf:first>
  </rdf:Description>
  <rdf:Description rdf:about="#Enumeration">
    <vs:term_status>stable</vs:term_status>
    <rdfs:label xml:lang="en">Enumeration restriction</rdfs:label>
    <rdfs:comment xml:lang="en">Enumeration restriction specifies that the value must be one of a list of allowed values. It is defined by complex restriction of IDS. In this ontology, it is defined as a restriction type, which specifies the restriction formulation.</rdfs:comment>
    <rdf:type rdf:resource="https://w3id.org/loin/v2/ids#RestrictionType"/>
  </rdf:Description>
  <rdf:Description rdf:nodeID="A2">
    <rdf:rest rdf:nodeID="A5"/>
    <rdf:first>L3</rdf:first>
  </rdf:Description>
  <rdf:Description rdf:about="#Required_For_Approval">
    <vs:term_status>stable</vs:term_status>
    <rdfs:label xml:lang="en">document required for approval</rdfs:label>
    <rdfs:comment xml:lang="en">The document required by deliverer is for getting approval</rdfs:comment>
    <rdf:type rdf:resource="#DocumentPurpose"/>
  </rdf:Description>
  <rdf:Description rdf:about="#Photograph">
    <vs:term_status>stable</vs:term_status>
    <rdfs:label>Photograph</rdfs:label>
    <rdfs:comment xml:lang="en">Documents such as records of work done, records of existing conditions according to notes of BS EN 17412-1 (2020)</rdfs:comment>
    <rdf:type rdf:resource="#DocumentContent"/>
  </rdf:Description>
  <rdf:Description rdf:nodeID="A6">
    <owl:onProperty rdf:resource="https://w3id.org/loin/v2/ids#restrictionFormulation"/>
    <owl:cardinality rdf:datatype="http://www.w3.org/2001/XMLSchema#nonNegativeInteger">1</owl:cardinality>
    <rdf:type rdf:resource="http://www.w3.org/2002/07/owl#Restriction"/>
  </rdf:Description>
  <rdf:Description rdf:nodeID="A7">
    <owl:onProperty rdf:resource="https://w3id.org/loin/v2/ids#restrictionFormulation"/>
    <owl:cardinality rdf:datatype="http://www.w3.org/2001/XMLSchema#nonNegativeInteger">1</owl:cardinality>
    <rdf:type rdf:resource="http://www.w3.org/2002/07/owl#Restriction"/>
  </rdf:Description>
  <rdf:Description rdf:about="https://w3id.org/loin/v2/ids#hasRestrictionType">
    <vs:term_status>stable</vs:term_status>
    <rdfs:range rdf:resource="https://w3id.org/loin/v2/ids#RestrictionType"/>
    <rdfs:label xml:lang="en">has restriction type</rdfs:label>
    <rdfs:domain rdf:resource="https://w3id.org/loin/v2/ids#FacetParameter"/>
    <rdfs:comment xml:lang="en">relates the restriction type with the facet parameter in IDS data definition</rdfs:comment>
    <rdf:type rdf:resource="http://www.w3.org/2002/07/owl#ObjectProperty"/>
  </rdf:Description>
  <rdf:Description rdf:about="https://w3id.org/loin/v2/icdd#isRelatedToLinksetIdentifier">
    <vs:term_status>stable</vs:term_status>
    <rdfs:range rdf:resource="https://standards.iso.org/iso/21597/-1/ed-1/en/Linkset#Identifier"/>
    <rdfs:label xml:lang="en">is related to linkset identifier</rdfs:label>
    <rdfs:domain rdf:resource="#IdentifierType"/>
    <rdfs:comment xml:lang="en">The object property is an extension with ICDD. It relates the identifier type defined by BS EN 17412-1(2020) with linkset identifier</rdfs:comment>
    <rdf:type rdf:resource="http://www.w3.org/2002/07/owl#ObjectProperty"/>
  </rdf:Description>
  <rdf:Description rdf:about="#Dimensionality">
    <vs:term_status>stable</vs:term_status>
    <rdfs:subClassOf rdf:nodeID="A8"/>
    <rdfs:subClassOf rdf:resource="#GeometrySpecification"/>
    <rdfs:label xml:lang="en">Dimensionality</rdfs:label>
    <rdfs:comment xml:lang="en">Dimensionality as a geometrical information specification for information need according to ISO 7817-3</rdfs:comment>
    <rdf:type rdf:resource="http://www.w3.org/2002/07/owl#Class"/>
  </rdf:Description>
  <rdf:Description rdf:nodeID="A9">
    <owl:onProperty rdf:resource="https://w3id.org/loin/v2/icdd#isRelatedToContainerLinkset"/>
    <owl:maxCardinality rdf:datatype="http://www.w3.org/2001/XMLSchema#nonNegativeInteger">1</owl:maxCardinality>
    <rdf:type rdf:resource="http://www.w3.org/2002/07/owl#Restriction"/>
  </rdf:Description>
  <rdf:Description rdf:about="https://w3id.org/loin/v2/ids#PropertyName">
    <vs:term_status>stable</vs:term_status>
    <rdfs:subClassOf rdf:nodeID="A10"/>
    <rdfs:subClassOf rdf:nodeID="A6"/>
    <rdfs:subClassOf rdf:resource="https://w3id.org/loin/v2/ids#FacetParameter"/>
    <rdfs:label xml:lang="en">Property name</rdfs:label>
    <rdfs:comment xml:lang="en">Property name must be a valid name from the IFC schema, or any custom text value according to IDS stan developed by buildingSMART International</rdfs:comment>
    <rdf:type rdf:resource="http://www.w3.org/2002/07/owl#Class"/>
  </rdf:Description>
  <rdf:Description rdf:nodeID="A4">
    <rdf:rest rdf:nodeID="A11"/>
    <rdf:first>D2</rdf:first>
  </rdf:Description>
  <rdf:Description rdf:about="#hasGroupOfProperties">
    <owl:equivalentProperty rdf:resource="https://w3id.org/tempo#hasSetOfProperties"/>
    <rdfs:subPropertyOf rdf:resource="http://www.w3.org/2002/07/owl#topObjectProperty"/>
    <rdfs:range rdf:resource="https://w3id.org/tempo#GroupOfProperties"/>
    <rdfs:label xml:lang="en">The object property relates the alphanumerical information with the set of properties  according to ISO 7817</rdfs:label>
    <rdfs:domain rdf:resource="#AlphanumericalInformation"/>
    <rdf:type rdf:resource="http://www.w3.org/2002/07/owl#ObjectProperty"/>
  </rdf:Description>
  <rdf:Description rdf:about="#informationDeliveryMilestone">
    <rdfs:subPropertyOf rdf:resource="http://www.w3.org/2002/07/owl#topDataProperty"/>
    <rdfs:range rdf:resource="http://www.w3.org/2001/XMLSchema#string"/>
    <rdfs:label xml:lang="en">Information delivery milestone</rdfs:label>
    <rdf:type rdf:resource="http://www.w3.org/2002/07/owl#DatatypeProperty"/>
  </rdf:Description>
  <rdf:Description rdf:nodeID="A12">
    <schema:memberOf rdf:nodeID="A13"/>
    <schema:name>Philipp Hagedorn</schema:name>
    <schema:identifier rdf:resource="https://orcid.org/0000-0002-6249-243X"/>
    <rdf:type rdf:resource="https://schema.org/Person"/>
    <schema:email rdf:resource="mailto:philipp.hagedorn-n6v@rub.de"/>
  </rdf:Description>
  <rdf:Description rdf:nodeID="A14">
    <owl:onProperty rdf:resource="#requested"/>
    <owl:cardinality rdf:datatype="http://www.w3.org/2001/XMLSchema#nonNegativeInteger">1</owl:cardinality>
    <rdf:type rdf:resource="http://www.w3.org/2002/07/owl#Restriction"/>
  </rdf:Description>
  <rdf:Description rdf:nodeID="A15">
    <owl:onProperty rdf:resource="https://w3id.org/loin/v2/ids#hasRequirement"/>
    <owl:minCardinality rdf:datatype="http://www.w3.org/2001/XMLSchema#nonNegativeInteger">1</owl:minCardinality>
    <rdf:type rdf:resource="http://www.w3.org/2002/07/owl#Restriction"/>
  </rdf:Description>
  <rdf:Description rdf:about="#absolute">
    <vs:term_status>stable</vs:term_status>
    <rdfs:label xml:lang="en">Absolute location</rdfs:label>
    <rdfs:comment xml:lang="en">An example of location according to notes of geometrical information specification for information need in BS EN 17412-1 (2020)</rdfs:comment>
    <rdf:type rdf:resource="#Location"/>
  </rdf:Description>
  <rdf:Description rdf:about="#EngineeringPrinciple">
    <vs:term_status>stable</vs:term_status>
    <rdfs:label xml:lang="en">Engineering principle</rdfs:label>
    <rdfs:comment xml:lang="en">An example of breakdown structure type according to BS EN 17412-1 (2020)</rdfs:comment>
    <rdf:type rdf:resource="#BreakdownStructureType"/>
  </rdf:Description>
  <rdf:Description rdf:about="https://w3id.org/loin/v2/ids#FacetParameter">
    <vs:term_status>stable</vs:term_status>
    <rdfs:subClassOf rdf:resource="http://www.w3.org/2000/01/rdf-schema#Resource"/>
    <rdfs:label xml:lang="en">IDS facet parameter</rdfs:label>
    <rdfs:comment xml:lang="en">IDS facet parameter is used to specify a facet definition according to IDS standard developed by buildingSMART International</rdfs:comment>
    <rdf:type rdf:resource="http://www.w3.org/2002/07/owl#Class"/>
  </rdf:Description>
  <rdf:Description rdf:about="https://w3id.org/loin/v2/icdd#isRelatedToContainerDocument">
    <vs:term_status>stable</vs:term_status>
    <rdfs:range rdf:resource="https://standards.iso.org/iso/21597/-1/ed-1/en/Container#Document"/>
    <rdfs:label xml:lang="en">is related to container document</rdfs:label>
    <rdfs:domain rdf:resource="#RequiredDocument"/>
    <rdfs:comment xml:lang="en">The object property is an extension with ICDD. It relates documents defined by BS EN 17412-1(2020) with container documents</rdfs:comment>
    <rdf:type rdf:resource="http://www.w3.org/2002/07/owl#SymmetricProperty"/>
    <rdf:type rdf:resource="http://www.w3.org/2002/07/owl#ObjectProperty"/>
  </rdf:Description>
  <rdf:Description rdf:nodeID="A16">
    <owl:oneOf rdf:nodeID="A17"/>
    <rdf:type rdf:resource="http://www.w3.org/2000/01/rdf-schema#Datatype"/>
  </rdf:Description>
  <rdf:Description rdf:nodeID="A18">
    <rdf:rest rdf:nodeID="A19"/>
    <rdf:first>D2</rdf:first>
  </rdf:Description>
  <rdf:Description rdf:nodeID="A20">
    <rdf:rest rdf:resource="http://www.w3.org/1999/02/22-rdf-syntax-ns#nil"/>
    <rdf:first>ParametricGeometry</rdf:first>
  </rdf:Description>
  <rdf:Description rdf:about="#hasAgent">
    <vs:term_status>stable</vs:term_status>
    <rdfs:subPropertyOf rdf:resource="http://www.w3.org/2002/07/owl#topObjectProperty"/>
    <rdfs:label xml:lang="en">has agent</rdfs:label>
    <rdfs:domain rdf:resource="#Actor"/>
    <rdfs:comment xml:lang="en">Information of the information delivery actor defined by foaf ontology mit class foaf:Agent</rdfs:comment>
    <rdf:type rdf:resource="http://www.w3.org/2002/07/owl#ObjectProperty"/>
  </rdf:Description>
  <rdf:Description rdf:nodeID="A21">
    <owl:onProperty rdf:resource="#sendingActor"/>
    <owl:onDataRange rdf:resource="http://www.w3.org/2001/XMLSchema#string"/>
    <owl:minQualifiedCardinality rdf:datatype="http://www.w3.org/2001/XMLSchema#nonNegativeInteger">0</owl:minQualifiedCardinality>
    <rdf:type rdf:resource="http://www.w3.org/2002/07/owl#Restriction"/>
  </rdf:Description>
  <rdf:Description rdf:nodeID="A22">
    <owl:onProperty rdf:resource="https://w3id.org/loin/v2/ids#hasRestrictionType"/>
    <owl:cardinality rdf:datatype="http://www.w3.org/2001/XMLSchema#nonNegativeInteger">1</owl:cardinality>
    <rdf:type rdf:resource="http://www.w3.org/2002/07/owl#Restriction"/>
  </rdf:Description>
  <rdf:Description rdf:about="#Documentation">
    <vs:term_status>stable</vs:term_status>
    <rdfs:subClassOf rdf:nodeID="A23"/>
    <rdfs:subClassOf rdf:nodeID="A24"/>
    <rdfs:subClassOf rdf:nodeID="A25"/>
    <rdfs:subClassOf rdf:nodeID="A26"/>
    <rdfs:subClassOf rdf:resource="#Information"/>
    <rdfs:label xml:lang="en">Documentation</rdfs:label>
    <rdfs:comment xml:lang="en">Documentation is a term for specifying the information need according to ISO 7817-3</rdfs:comment>
    <rdf:type rdf:resource="http://www.w3.org/2002/07/owl#Class"/>
  </rdf:Description>
  <rdf:Description rdf:nodeID="A27">
    <owl:onProperty rdf:resource="#requested"/>
    <owl:cardinality rdf:datatype="http://www.w3.org/2001/XMLSchema#nonNegativeInteger">1</owl:cardinality>
    <rdf:type rdf:resource="http://www.w3.org/2002/07/owl#Restriction"/>
  </rdf:Description>
  <rdf:Description rdf:nodeID="A28">
    <rdf:rest rdf:nodeID="A29"/>
    <rdf:first>MaterialColor</rdf:first>
  </rdf:Description>
  <rdf:Description rdf:about="#one-dimensional">
    <vs:term_status>stable</vs:term_status>
    <rdfs:label xml:lang="en">one-dimensional</rdfs:label>
    <rdfs:comment xml:lang="en">one-dimensional, an example of dimensionality according to notes of geometrical information specification for information need in BS EN 17412-1 (2020)</rdfs:comment>
    <rdf:type rdf:resource="#Dimensionality"/>
  </rdf:Description>
  <rdf:Description rdf:about="#hasAppearance">
    <vs:term_status>stable</vs:term_status>
    <rdfs:subPropertyOf rdf:resource="http://www.w3.org/2002/07/owl#topDataProperty"/>
    <rdfs:range rdf:nodeID="A30"/>
    <rdfs:label xml:lang="en">has appearance</rdfs:label>
    <rdfs:domain rdf:resource="#Appearance"/>
    <rdf:type rdf:resource="http://www.w3.org/2002/07/owl#DatatypeProperty"/>
  </rdf:Description>
  <rdf:Description rdf:nodeID="A31">
    <owl:onProperty rdf:resource="#value"/>
    <owl:cardinality rdf:datatype="http://www.w3.org/2001/XMLSchema#nonNegativeInteger">1</owl:cardinality>
    <rdf:type rdf:resource="http://www.w3.org/2002/07/owl#Restriction"/>
  </rdf:Description>
  <rdf:Description rdf:nodeID="A32">
    <owl:onProperty rdf:resource="https://w3id.org/loin/v2/ids#belongsToPset"/>
    <owl:cardinality rdf:datatype="http://www.w3.org/2001/XMLSchema#nonNegativeInteger">1</owl:cardinality>
    <rdf:type rdf:resource="http://www.w3.org/2002/07/owl#Restriction"/>
  </rdf:Description>
  <rdf:Description rdf:nodeID="A33">
    <owl:onProperty rdf:resource="#sendingActor"/>
    <owl:onDataRange rdf:resource="http://www.w3.org/2001/XMLSchema#string"/>
    <owl:maxQualifiedCardinality rdf:datatype="http://www.w3.org/2001/XMLSchema#nonNegativeInteger">1</owl:maxQualifiedCardinality>
    <rdf:type rdf:resource="http://www.w3.org/2002/07/owl#Restriction"/>
  </rdf:Description>
  <rdf:Description rdf:nodeID="A34">
    <rdf:rest rdf:nodeID="A18"/>
    <rdf:first>D1</rdf:first>
  </rdf:Description>
  <rdf:Description rdf:nodeID="A35">
    <owl:someValuesFrom rdf:resource="#DocumentContent"/>
    <owl:onProperty rdf:resource="#hasDocumentSpecification"/>
    <rdf:type rdf:resource="http://www.w3.org/2002/07/owl#Restriction"/>
  </rdf:Description>
  <rdf:Description rdf:about="https://w3id.org/loin/v2/icdd#isRelatedToContainerDescription">
    <vs:term_status>stable</vs:term_status>
    <rdfs:range rdf:resource="https://standards.iso.org/iso/21597/-1/ed-1/en/Container#ContainerDescription"/>
    <rdfs:label xml:lang="en">is related to container description</rdfs:label>
    <rdfs:domain rdf:resource="#Purpose"/>
    <rdfs:comment xml:lang="en">The object property is an extension with ICDD. It relates the information delivery milestone defined by BS EN 17412-1(2020) with container description</rdfs:comment>
    <rdf:type rdf:resource="http://www.w3.org/2002/07/owl#ObjectProperty"/>
  </rdf:Description>
  <rdf:Description rdf:about="https://w3id.org/loin/v2/ids#hasPredefinedType">
    <vs:term_status>stable</vs:term_status>
    <rdfs:range rdf:resource="https://w3id.org/loin/v2/ids#PredefinedType"/>
    <rdfs:label xml:lang="en">has predefined type</rdfs:label>
    <rdfs:domain rdf:resource="https://w3id.org/loin/v2/ids#Entity"/>
    <rdfs:comment xml:lang="en">The object property relates a predefined type with the facet entity according to IDS definition</rdfs:comment>
    <rdf:type rdf:resource="http://www.w3.org/2002/07/owl#ObjectProperty"/>
  </rdf:Description>
  <rdf:Description rdf:nodeID="A36">
    <owl:someValuesFrom rdf:resource="#Appearance"/>
    <owl:onProperty rdf:resource="#hasGeometrySpecification"/>
    <rdf:type rdf:resource="http://www.w3.org/2002/07/owl#Restriction"/>
  </rdf:Description>
  <rdf:Description rdf:about="#Report">
    <vs:term_status>stable</vs:term_status>
    <rdfs:label>Report</rdfs:label>
    <rdfs:comment xml:lang="en">Documents such as geotechnical reports, reports of existing building conditions, soil surveys, pre calculations according to notes of BS EN 17412-1 (2020)</rdfs:comment>
    <rdf:type rdf:resource="#DocumentContent"/>
  </rdf:Description>
  <rdf:Description rdf:nodeID="A37">
    <owl:onProperty rdf:resource="https://w3id.org/loin/v2/ids#hasAttributeName"/>
    <owl:cardinality rdf:datatype="http://www.w3.org/2001/XMLSchema#nonNegativeInteger">1</owl:cardinality>
    <rdf:type rdf:resource="http://www.w3.org/2002/07/owl#Restriction"/>
  </rdf:Description>
  <rdf:Description rdf:nodeID="A19">
    <rdf:rest rdf:resource="http://www.w3.org/1999/02/22-rdf-syntax-ns#nil"/>
    <rdf:first>D3</rdf:first>
  </rdf:Description>
  <rdf:Description rdf:about="#TypeName">
    <vs:term_status>stable</vs:term_status>
    <rdfs:label xml:lang="en">Type name of an item in a breakdown structure</rdfs:label>
    <rdfs:comment xml:lang="en">Type name, an identifier type in a breakdown structure according to notes of BS EN 17412-1 (2020)</rdfs:comment>
    <rdf:type rdf:resource="#IdentifierType"/>
  </rdf:Description>
  <rdf:Description rdf:about="#Codification">
    <vs:term_status>stable</vs:term_status>
    <rdfs:label xml:lang="en">Codification of an item in a breakdown structure</rdfs:label>
    <rdfs:comment xml:lang="en">An example of identifier type from a breakdown structure according to BS EN 17412-1 (2020)</rdfs:comment>
    <rdf:type rdf:resource="#IdentifierType"/>
  </rdf:Description>
  <rdf:Description rdf:nodeID="A5">
    <rdf:rest rdf:nodeID="A38"/>
    <rdf:first>L4</rdf:first>
  </rdf:Description>
  <rdf:Description rdf:nodeID="A39">
    <owl:onProperty rdf:resource="#hasDescriptionInLanguage"/>
    <owl:onDataRange rdf:resource="http://www.w3.org/1999/02/22-rdf-syntax-ns#langString"/>
    <owl:maxQualifiedCardinality rdf:datatype="http://www.w3.org/2001/XMLSchema#nonNegativeInteger">1</owl:maxQualifiedCardinality>
    <rdf:type rdf:resource="http://www.w3.org/2002/07/owl#Restriction"/>
  </rdf:Description>
  <rdf:Description rdf:nodeID="A40">
    <rdf:type rdf:resource="https://schema.org/Organization"/>
    <schema:name>Ruhr University Bochum, Germany</schema:name>
  </rdf:Description>
  <rdf:Description rdf:about="">
    <rdfs:comment>The Level of Information Need (LOIN) Ontology is defined for specifying information requirements for delivery of data in a buildings' life cycle. The LOIN ontology is based on the standard BS EN 17412-1 (2020). Furthermore, it is extended with vocabulary for connecing Information Delivery Specifications (IDS) and Information containers for linked document delivery (ICDD) as per ISO 21597-1 (2020). 

The namespace for LOIN terms is [https://w3id.org/loin](https://w3id.org/loin)

The preferred prefix for the LOIN Ontology namespace is `loin`.

## Ontology Overview 
![LOIN Ontology](figures/OntologyOverview.svg "Ontology")

</rdfs:comment>
    <dc:license rdf:resource="https://creativecommons.org/licenses/by/4.0/"/>
    <dc:publisher rdf:nodeID="A41"/>
    <dc:creator rdf:nodeID="A12"/>
    <dc:contributor rdf:nodeID="A42"/>
    <dc:modified rdf:datatype="http://www.w3.org/2001/XMLSchema#date">2025-01-15</dc:modified>
    <rdf:type rdf:resource="http://www.w3.org/2002/07/owl#Ontology"/>
    <vann:preferredNamespacePrefix>loin</vann:preferredNamespacePrefix>
    <j.0:historyNote>v3.0: Adjustments due to the update of the IR Ontology Network
v2.0: Updated and aligned within the IR-Ontology Network
v1.0: Creation of LOIN Ontology</j.0:historyNote>
    <dc:issued rdf:datatype="http://www.w3.org/2001/XMLSchema#date">2024-03-15</dc:issued>
    <dc:source rdf:resource="https://linkedbuildingdata.net/ldac2024/files/papers/LDAC2024_Camera_8.pdf"/>
    <dc:title xml:lang="en">Level of Information Need (LOIN) Ontology</dc:title>
    <owl:imports rdf:resource="https://w3id.org/tempo"/>
    <dc:created rdf:datatype="http://www.w3.org/2001/XMLSchema#date">2023-01-30</dc:created>
    <dc:creator rdf:nodeID="A43"/>
    <owl:versionInfo>3.0</owl:versionInfo>
    <dc:rights>Copyright 2023 by Chair of Computing in Engineering, Ruhr University Bochum</dc:rights>
    <vann:preferredNamespaceUri>https://w3id.org/loin#</vann:preferredNamespaceUri>
  </rdf:Description>
  <rdf:Description rdf:about="#FederationStrategy">
    <vs:term_status>stable</vs:term_status>
    <rdfs:label xml:lang="en">Federation strategy</rdfs:label>
    <rdfs:comment xml:lang="en">An example of breakdown structure type according to BS EN 17412-1 (2020)</rdfs:comment>
    <rdf:type rdf:resource="#BreakdownStructureType"/>
  </rdf:Description>
  <rdf:Description rdf:about="#Length">
    <vs:term_status>stable</vs:term_status>
    <rdfs:label xml:lang="en">Length restriction</rdfs:label>
    <rdfs:comment xml:lang="en">Length restriction specifies the exact number of characters allowed in a value. It is defined by complex restriction of IDS. In this ontology, it is defined as a restriction type, which specifies the restriction formulation.</rdfs:comment>
    <rdf:type rdf:resource="https://w3id.org/loin/v2/ids#RestrictionType"/>
  </rdf:Description>
  <rdf:Description rdf:about="#BreakdownStructureType">
    <vs:term_status>stable</vs:term_status>
    <rdfs:subClassOf rdf:resource="http://www.w3.org/2002/07/owl#Thing"/>
    <rdfs:label xml:lang="en">Breakdown structure type</rdfs:label>
    <rdfs:comment xml:lang="en">Breakdown structure type is a term to specify the structure according to BS EN 17412-1 (2020)</rdfs:comment>
    <rdf:type rdf:resource="http://www.w3.org/2002/07/owl#Class"/>
  </rdf:Description>
  <rdf:Description rdf:about="#hasObjectType">
    <rdfs:subPropertyOf rdf:resource="http://www.w3.org/2002/07/owl#topObjectProperty"/>
    <rdfs:range rdf:resource="https://w3id.org/tempo#ObjectType"/>
    <rdfs:label xml:lang="en">has object type</rdfs:label>
    <rdfs:domain rdf:resource="#SpecificationPerObjectType"/>
    <rdfs:comment xml:lang="en">The object property relates the specification per object type with the object type</rdfs:comment>
    <rdf:type rdf:resource="http://www.w3.org/2002/07/owl#ObjectProperty"/>
  </rdf:Description>
  <rdf:Description rdf:about="#realistic">
    <vs:term_status>stable</vs:term_status>
    <rdfs:label xml:lang="en">realistic</rdfs:label>
    <rdfs:comment xml:lang="en">realistic, an example of appearance according to notes of geometrical information specification for information need in BS EN 17412-1 (2020)</rdfs:comment>
    <rdf:type rdf:resource="#Appearance"/>
  </rdf:Description>
  <rdf:Description rdf:about="#constructive">
    <vs:term_status>stable</vs:term_status>
    <rdfs:label xml:lang="en">constructive</rdfs:label>
    <rdfs:comment xml:lang="en">An example of parametric behaviour according to notes of geometrical information specification for information need in BS EN 17412-1 (2020)</rdfs:comment>
    <rdf:type rdf:resource="#ParametricBehaviour"/>
  </rdf:Description>
  <rdf:Description rdf:nodeID="A44">
    <owl:onProperty rdf:resource="#hasIdentifierType"/>
    <owl:cardinality rdf:datatype="http://www.w3.org/2001/XMLSchema#nonNegativeInteger">1</owl:cardinality>
    <rdf:type rdf:resource="http://www.w3.org/2002/07/owl#Restriction"/>
  </rdf:Description>
  <rdf:Description rdf:nodeID="A45">
    <rdf:rest rdf:resource="http://www.w3.org/1999/02/22-rdf-syntax-ns#nil"/>
    <rdf:first>Prohibited</rdf:first>
  </rdf:Description>
  <rdf:Description rdf:about="#Location">
    <vs:term_status>stable</vs:term_status>
    <rdfs:subClassOf rdf:nodeID="A46"/>
    <rdfs:subClassOf rdf:resource="#GeometrySpecification"/>
    <rdfs:label xml:lang="en">Location</rdfs:label>
    <rdfs:comment xml:lang="en">Location as a geometrical information specification for information need according to ISO 7817-3</rdfs:comment>
    <rdf:type rdf:resource="http://www.w3.org/2002/07/owl#Class"/>
  </rdf:Description>
  <rdf:Description rdf:about="#hasNameInLanguage">
    <rdfs:subPropertyOf rdf:resource="http://www.w3.org/2002/07/owl#topDataProperty"/>
    <rdfs:range rdf:resource="http://www.w3.org/1999/02/22-rdf-syntax-ns#langString"/>
    <rdfs:label xml:lang="en">Site plan</rdfs:label>
    <rdfs:label xml:lang="de">Lageplan</rdfs:label>
    <rdf:type rdf:resource="http://www.w3.org/2002/07/owl#DatatypeProperty"/>
  </rdf:Description>
  <rdf:Description rdf:about="https://w3id.org/loin/v2/ids#PsetName">
    <vs:term_status>stable</vs:term_status>
    <rdfs:subClassOf rdf:nodeID="A47"/>
    <rdfs:subClassOf rdf:nodeID="A48"/>
    <rdfs:subClassOf rdf:resource="https://w3id.org/loin/v2/ids#FacetParameter"/>
    <rdfs:label xml:lang="en">Property set name</rdfs:label>
    <rdfs:comment xml:lang="en">Property set name must be a valid name from the IFC schema, or any custom text value according to IDS standard developed by buildingSMART International</rdfs:comment>
    <rdf:type rdf:resource="http://www.w3.org/2002/07/owl#Class"/>
  </rdf:Description>
  <rdf:Description rdf:nodeID="A49">
    <owl:oneOf rdf:nodeID="A50"/>
    <rdf:type rdf:resource="http://www.w3.org/2000/01/rdf-schema#Datatype"/>
  </rdf:Description>
  <rdf:Description rdf:nodeID="A17">
    <rdf:rest rdf:nodeID="A51"/>
    <rdf:first>ExplicitGeometry</rdf:first>
  </rdf:Description>
  <rdf:Description rdf:nodeID="A52">
    <rdf:rest rdf:nodeID="A20"/>
    <rdf:first>ConstructiveGeometry</rdf:first>
  </rdf:Description>
  <rdf:Description rdf:about="#real-world">
    <vs:term_status>stable</vs:term_status>
    <rdfs:label xml:lang="en">real-world</rdfs:label>
    <rdfs:comment xml:lang="en">Real-world, an example of appearance according to notes of geometrical information specification for information need in BS EN 17412-1 (2020)</rdfs:comment>
    <rdf:type rdf:resource="#Appearance"/>
  </rdf:Description>
  <rdf:Description rdf:about="#hasDocumentation">
    <vs:term_status>stable</vs:term_status>
    <rdfs:subPropertyOf rdf:resource="#hasInformation"/>
    <rdfs:range rdf:resource="#Documentation"/>
    <rdfs:label xml:lang="en">has documentation</rdfs:label>
    <rdfs:domain rdf:resource="#SpecificationPerObjectType"/>
    <rdfs:comment xml:lang="en">The object property relates the documentation with a LOIN object according to ISO 7817-3</rdfs:comment>
    <rdf:type rdf:resource="http://www.w3.org/2002/07/owl#ObjectProperty"/>
  </rdf:Description>
  <rdf:Description rdf:nodeID="A53">
    <owl:onProperty rdf:resource="#hasQuantityKind"/>
    <owl:minCardinality rdf:datatype="http://www.w3.org/2001/XMLSchema#nonNegativeInteger">0</owl:minCardinality>
    <rdf:type rdf:resource="http://www.w3.org/2002/07/owl#Restriction"/>
  </rdf:Description>
  <rdf:Description rdf:nodeID="A54">
    <owl:qualifiedCardinality rdf:datatype="http://www.w3.org/2001/XMLSchema#nonNegativeInteger">1</owl:qualifiedCardinality>
    <owl:onProperty rdf:resource="#hasDetail"/>
    <owl:onDataRange rdf:nodeID="A55"/>
    <rdf:type rdf:resource="http://www.w3.org/2002/07/owl#Restriction"/>
  </rdf:Description>
  <rdf:Description rdf:about="#Name">
    <vs:term_status>stable</vs:term_status>
    <rdfs:label xml:lang="en">Name of an item in a breakdown structure</rdfs:label>
    <rdfs:comment xml:lang="en">Name, an identifier type in a breakdown structure according to notes of BS EN 17412-1 (2020)</rdfs:comment>
    <rdf:type rdf:resource="#IdentifierType"/>
  </rdf:Description>
  <rdf:Description rdf:about="#hasBreakdownStructure">
    <vs:term_status>stable</vs:term_status>
    <rdfs:subPropertyOf rdf:resource="http://www.w3.org/2002/07/owl#topObjectProperty"/>
    <rdfs:range rdf:resource="#BreakdownStructure"/>
    <rdfs:label xml:lang="en">has breakdown structure</rdfs:label>
    <rdfs:domain rdf:resource="#Identification"/>
    <rdfs:comment xml:lang="en">The object property relates the identification with a breakdown structure according to BS EN 17412-1 (2020)</rdfs:comment>
    <rdf:type rdf:resource="http://www.w3.org/2002/07/owl#ObjectProperty"/>
  </rdf:Description>
  <rdf:Description rdf:nodeID="A56">
    <owl:oneOf rdf:nodeID="A57"/>
    <rdf:type rdf:resource="http://www.w3.org/2000/01/rdf-schema#Datatype"/>
  </rdf:Description>
  <rdf:Description rdf:about="#hasReferenceDocument">
    <owl:equivalentProperty rdf:resource="https://w3id.org/tempo#hasReferenceDocument"/>
    <rdfs:subPropertyOf rdf:resource="http://www.w3.org/2002/07/owl#topObjectProperty"/>
    <rdfs:range rdf:resource="https://w3id.org/tempo#ReferenceDocument"/>
    <rdfs:label>has reference document</rdfs:label>
    <rdfs:domain rdf:resource="#AlphanumericalInformation"/>
    <rdfs:comment xml:lang="en">The object property relates the alphanumerical information with the reference document according to ISO 7817-3</rdfs:comment>
    <rdf:type rdf:resource="http://www.w3.org/2002/07/owl#ObjectProperty"/>
  </rdf:Description>
  <rdf:Description rdf:nodeID="A58">
    <owl:onProperty rdf:resource="#hasGroupOfProperties"/>
    <owl:minCardinality rdf:datatype="http://www.w3.org/2001/XMLSchema#nonNegativeInteger">0</owl:minCardinality>
    <rdf:type rdf:resource="http://www.w3.org/2002/07/owl#Restriction"/>
  </rdf:Description>
  <rdf:Description rdf:nodeID="A59">
    <owl:onProperty rdf:resource="#hasReferenceDocument"/>
    <owl:minCardinality rdf:datatype="http://www.w3.org/2001/XMLSchema#nonNegativeInteger">0</owl:minCardinality>
    <rdf:type rdf:resource="http://www.w3.org/2002/07/owl#Restriction"/>
  </rdf:Description>
  <rdf:Description rdf:nodeID="A60">
    <owl:onProperty rdf:resource="#receivingActor"/>
    <owl:onDataRange rdf:resource="http://www.w3.org/2001/XMLSchema#string"/>
    <owl:minQualifiedCardinality rdf:datatype="http://www.w3.org/2001/XMLSchema#nonNegativeInteger">0</owl:minQualifiedCardinality>
    <rdf:type rdf:resource="http://www.w3.org/2002/07/owl#Restriction"/>
  </rdf:Description>
  <rdf:Description rdf:about="https://w3id.org/loin/v2/ids#EntityName">
    <vs:term_status>stable</vs:term_status>
    <rdfs:subClassOf rdf:nodeID="A61"/>
    <rdfs:subClassOf rdf:nodeID="A22"/>
    <rdfs:subClassOf rdf:resource="https://w3id.org/loin/v2/ids#FacetParameter"/>
    <rdfs:label xml:lang="en">Entity name</rdfs:label>
    <rdfs:comment xml:lang="en">Entity name must be a valid IFC class from the IFC schema according to IDS developed by buildingSMART International. Example EntityName = "IFCWALL"</rdfs:comment>
    <rdf:type rdf:resource="http://www.w3.org/2002/07/owl#Class"/>
  </rdf:Description>
  <rdf:Description rdf:nodeID="A62">
    <rdf:rest rdf:nodeID="A63"/>
    <rdf:first>NoColor</rdf:first>
  </rdf:Description>
  <rdf:Description rdf:about="#symbolic">
    <vs:term_status>stable</vs:term_status>
    <rdfs:label xml:lang="en">symbolic</rdfs:label>
    <rdfs:comment xml:lang="en">symbolic, an example of appearance according to notes of geometrical information specification for information need in BS EN 17412-1 (2020)</rdfs:comment>
    <rdf:type rdf:resource="#Appearance"/>
  </rdf:Description>
  <rdf:Description rdf:about="#explicit">
    <vs:term_status>stable</vs:term_status>
    <rdfs:label xml:lang="en">explicit</rdfs:label>
    <rdfs:comment xml:lang="en">Explicit, an example of parametric behaviour according to notes of geometrical information specification for information need in BS EN 17412-1 (2020)</rdfs:comment>
    <rdf:type rdf:resource="#ParametricBehaviour"/>
  </rdf:Description>
  <rdf:Description rdf:nodeID="A64">
    <owl:unionOf rdf:nodeID="A65"/>
    <rdf:type rdf:resource="http://www.w3.org/2002/07/owl#Class"/>
  </rdf:Description>
  <rdf:Description rdf:about="#ClassificationSystem">
    <vs:term_status>stable</vs:term_status>
    <rdfs:label xml:lang="en">Classification system</rdfs:label>
    <rdfs:comment xml:lang="en">An example of breakdown structure type according to BS EN 17412-1 (2020)</rdfs:comment>
    <rdf:type rdf:resource="#BreakdownStructureType"/>
  </rdf:Description>
  <rdf:Description rdf:about="#Specification">
    <rdfs:subClassOf rdf:nodeID="A39"/>
    <rdf:type rdf:resource="http://www.w3.org/2002/07/owl#Class"/>
    <rdfs:label xml:lang="en">has Reference Type</rdfs:label>
    <rdfs:subClassOf rdf:nodeID="A66"/>
    <rdfs:subClassOf rdf:nodeID="A67"/>
    <rdfs:subClassOf rdf:resource="http://www.w3.org/2002/07/owl#Thing"/>
    <rdfs:subClassOf rdf:nodeID="A68"/>
    <rdfs:subClassOf rdf:nodeID="A69"/>
    <rdfs:subClassOf rdf:nodeID="A70"/>
    <rdfs:subClassOf rdf:nodeID="A71"/>
    <rdfs:subClassOf rdf:nodeID="A72"/>
  </rdf:Description>
  <rdf:Description rdf:nodeID="A73">
    <owl:onProperty rdf:resource="https://w3id.org/loin/v2/ids#restrictionFormulation"/>
    <owl:cardinality rdf:datatype="http://www.w3.org/2001/XMLSchema#nonNegativeInteger">1</owl:cardinality>
    <rdf:type rdf:resource="http://www.w3.org/2002/07/owl#Restriction"/>
  </rdf:Description>
  <rdf:Description rdf:about="https://w3id.org/loin/v2/ids#AttributeName">
    <vs:term_status>stable</vs:term_status>
    <rdfs:subClassOf rdf:nodeID="A74"/>
    <rdfs:subClassOf rdf:nodeID="A75"/>
    <rdfs:subClassOf rdf:resource="https://w3id.org/loin/v2/ids#FacetParameter"/>
    <rdfs:label xml:lang="en">Attribute name</rdfs:label>
    <rdfs:comment xml:lang="en">Attribute name must be a valid attribute name from the IFC schema according to the definition of IDS developed by buildingSMART International. Example AttributeName = "Description"</rdfs:comment>
    <rdf:type rdf:resource="http://www.w3.org/2002/07/owl#Class"/>
  </rdf:Description>
  <rdf:Description rdf:about="https://w3id.org/loin/v2/ids#IFCDataType">
    <vs:term_status>stable</vs:term_status>
    <rdfs:subClassOf rdf:nodeID="A7"/>
    <rdfs:subClassOf rdf:nodeID="A76"/>
    <rdfs:subClassOf rdf:resource="https://w3id.org/loin/v2/ids#FacetParameter"/>
    <rdfs:label xml:lang="en">IFC data type</rdfs:label>
    <rdfs:comment xml:lang="en">IFC data type must be a valid predefined type from the IFC schema according to IDS standard developed by buildingSMART International</rdfs:comment>
    <rdf:type rdf:resource="http://www.w3.org/2002/07/owl#Class"/>
  </rdf:Description>
  <rdf:Description rdf:about="https://w3id.org/loin/v2/ids#hasIFCDataType">
    <vs:term_status>stable</vs:term_status>
    <rdfs:range rdf:resource="https://w3id.org/loin/v2/ids#IFCDataType"/>
    <rdfs:label xml:lang="en">has IFC data type</rdfs:label>
    <rdfs:domain rdf:resource="https://w3id.org/loin/v2/ids#Property"/>
    <rdfs:comment xml:lang="en">The object property relates the IFC data type with the facet property according to IDS definition</rdfs:comment>
    <rdf:type rdf:resource="http://www.w3.org/2002/07/owl#ObjectProperty"/>
  </rdf:Description>
  <rdf:Description rdf:about="https://w3id.org/loin/v2/ids#hasRequirement">
    <vs:term_status>stable</vs:term_status>
    <rdfs:range rdf:resource="https://w3id.org/loin/v2/ids#FacetDefinition"/>
    <rdfs:label xml:lang="en">has requirement</rdfs:label>
    <rdfs:domain rdf:resource="https://w3id.org/loin/v2/ids#DataDefinition"/>
    <rdfs:comment xml:lang="en">The object property relates the requirements with the IDS data definition</rdfs:comment>
    <rdf:type rdf:resource="http://www.w3.org/2002/07/owl#ObjectProperty"/>
  </rdf:Description>
  <rdf:Description rdf:about="https://w3id.org/loin/v2/ids#Attribute">
    <vs:term_status>stable</vs:term_status>
    <rdfs:subClassOf rdf:nodeID="A37"/>
    <rdfs:subClassOf rdf:resource="https://w3id.org/loin/v2/ids#FacetDefinition"/>
    <rdfs:label xml:lang="en">Attribute of IDS</rdfs:label>
    <rdfs:comment xml:lang="en">Attribute is a facet of Information Delivery Specification (IDS), a standard developed by buildingSMART International</rdfs:comment>
    <rdf:type rdf:resource="http://www.w3.org/2002/07/owl#Class"/>
  </rdf:Description>
  <rdf:Description rdf:about="#hasGeometrySpecification">
    <vs:term_status>stable</vs:term_status>
    <rdfs:subPropertyOf rdf:resource="http://www.w3.org/2002/07/owl#topObjectProperty"/>
    <rdfs:range rdf:resource="#GeometrySpecification"/>
    <rdfs:label xml:lang="en">has geometrical specification</rdfs:label>
    <rdfs:domain rdf:resource="#GeometricalInformation"/>
    <rdfs:comment>["Appearance",&#xD;
"Detail",&#xD;
"Dimensionality",&#xD;
"Location",&#xD;
"ParametricBehaviour"]</rdfs:comment>
    <rdfs:comment xml:lang="en">The object property relates the specific aspects with geometrical information according to ISO 7817-3</rdfs:comment>
    <rdf:type rdf:resource="http://www.w3.org/2002/07/owl#ObjectProperty"/>
  </rdf:Description>
  <rdf:Description rdf:nodeID="A77">
    <rdf:rest rdf:nodeID="A78"/>
    <rdf:first>Absolute</rdf:first>
  </rdf:Description>
  <rdf:Description rdf:nodeID="A79">
    <owl:onProperty rdf:resource="https://w3id.org/loin/v2/ids#hasRestrictionType"/>
    <owl:cardinality rdf:datatype="http://www.w3.org/2001/XMLSchema#nonNegativeInteger">1</owl:cardinality>
    <rdf:type rdf:resource="http://www.w3.org/2002/07/owl#Restriction"/>
  </rdf:Description>
  <rdf:Description rdf:about="#hasIdentifierType">
    <rdfs:subPropertyOf rdf:resource="http://www.w3.org/2002/07/owl#topObjectProperty"/>
    <rdfs:range rdf:resource="#IdentifierType"/>
    <rdfs:label xml:lang="en">has identifier type</rdfs:label>
    <rdfs:domain rdf:resource="#Identifier"/>
    <rdfs:comment xml:lang="en">The object property relates an identifier of breakdown structure with a specific type according to BS EN 17412-1 (2020)</rdfs:comment>
    <rdf:type rdf:resource="http://www.w3.org/2002/07/owl#ObjectProperty"/>
  </rdf:Description>
  <rdf:Description rdf:nodeID="A80">
    <rdf:rest rdf:resource="http://www.w3.org/1999/02/22-rdf-syntax-ns#nil"/>
    <rdf:first>Textures</rdf:first>
  </rdf:Description>
  <rdf:Description rdf:about="#detailed">
    <vs:term_status>stable</vs:term_status>
    <rdfs:label xml:lang="en">detailed</rdfs:label>
    <rdfs:comment xml:lang="en">Detail, an example of detail aspect according to notes of geometrical information specification for information need in BS EN 17412-1 (2020)</rdfs:comment>
    <rdf:type rdf:resource="#Detail"/>
  </rdf:Description>
  <rdf:Description rdf:nodeID="A81">
    <rdf:rest rdf:nodeID="A82"/>
    <rdf:first>L2</rdf:first>
  </rdf:Description>
  <rdf:Description rdf:nodeID="A47">
    <owl:onProperty rdf:resource="https://w3id.org/loin/v2/ids#restrictionFormulation"/>
    <owl:cardinality rdf:datatype="http://www.w3.org/2001/XMLSchema#nonNegativeInteger">1</owl:cardinality>
    <rdf:type rdf:resource="http://www.w3.org/2002/07/owl#Restriction"/>
  </rdf:Description>
  <rdf:Description rdf:about="#Numbering">
    <vs:term_status>stable</vs:term_status>
    <rdfs:label>Numbering of an item in a breakdown structure</rdfs:label>
    <rdfs:comment xml:lang="en">Numbering, an identifier type in a breakdown structure according to notes of BS EN 17412-1 (2020)</rdfs:comment>
    <rdf:type rdf:resource="#IdentifierType"/>
  </rdf:Description>
  <rdf:Description rdf:about="#coordination">
    <vs:term_status>stable</vs:term_status>
    <rdfs:label xml:lang="en">Coordination</rdfs:label>
    <rdfs:comment xml:lang="en">coordination, an example of IDM purpose from BS EN 17412-1 (2020) - Annex B</rdfs:comment>
    <rdf:type rdf:resource="#Purpose"/>
  </rdf:Description>
  <rdf:Description rdf:nodeID="A83">
    <schema:name>Ruhr University Bochum</schema:name>
    <schema:identifier rdf:resource="https://www.inf.bi.ruhr-uni-bochum.de/iib/lehrstuhl/mitarbeiter/liu_liu.html.en"/>
  </rdf:Description>
  <rdf:Description rdf:about="#Spatial">
    <vs:term_status>stable</vs:term_status>
    <rdfs:label xml:lang="en">Spatial structure</rdfs:label>
    <rdfs:comment xml:lang="en">An example of breakdown structure type according to BS EN 17412-1 (2020)</rdfs:comment>
    <rdf:type rdf:resource="#BreakdownStructureType"/>
  </rdf:Description>
  <rdf:Description rdf:about="#hasIdentifier">
    <vs:term_status>stable</vs:term_status>
    <rdfs:subPropertyOf rdf:resource="http://www.w3.org/2002/07/owl#topObjectProperty"/>
    <rdfs:range rdf:resource="#Identifier"/>
    <rdfs:label xml:lang="en">has identifier</rdfs:label>
    <rdfs:domain rdf:resource="#BreakdownStructure"/>
    <rdfs:comment xml:lang="en">The object property relates a breakdown structure with its identifier according to BS EN 17412-1 (2020)</rdfs:comment>
    <rdf:type rdf:resource="http://www.w3.org/2002/07/owl#ObjectProperty"/>
  </rdf:Description>
  <rdf:Description rdf:about="#hasProperty">
    <owl:equivalentProperty rdf:resource="https://w3id.org/tempo#hasProperty"/>
    <rdfs:subPropertyOf rdf:resource="http://www.w3.org/2002/07/owl#topObjectProperty"/>
    <rdfs:range rdf:resource="https://w3id.org/tempo#Property"/>
    <rdfs:range rdf:resource="https://w3id.org/isoprops#Property"/>
    <rdfs:label xml:lang="en">The object property relates the data template with the properties</rdfs:label>
    <rdfs:domain rdf:resource="https://w3id.org/tempo#DataTemplate"/>
    <rdf:type rdf:resource="http://www.w3.org/2002/07/owl#ObjectProperty"/>
  </rdf:Description>
  <rdf:Description rdf:nodeID="A84">
    <owl:onProperty rdf:resource="#purpose"/>
    <owl:onDataRange rdf:resource="http://www.w3.org/2001/XMLSchema#string"/>
    <owl:minQualifiedCardinality rdf:datatype="http://www.w3.org/2001/XMLSchema#nonNegativeInteger">0</owl:minQualifiedCardinality>
    <rdf:type rdf:resource="http://www.w3.org/2002/07/owl#Restriction"/>
  </rdf:Description>
  <rdf:Description rdf:about="https://w3id.org/dt#isDataTemplateFor">
    <owl:inverseOf rdf:resource="#hasDataTemplate"/>
  </rdf:Description>
  <rdf:Description rdf:nodeID="A85">
    <owl:onProperty rdf:resource="https://w3id.org/tempo#conceptGUID"/>
    <owl:onDataRange rdf:resource="https://w3id.org/tempo#GUIDType"/>
    <owl:minQualifiedCardinality rdf:datatype="http://www.w3.org/2001/XMLSchema#nonNegativeInteger">0</owl:minQualifiedCardinality>
    <rdf:type rdf:resource="http://www.w3.org/2002/07/owl#Restriction"/>
  </rdf:Description>
  <rdf:Description rdf:nodeID="A78">
    <rdf:rest rdf:resource="http://www.w3.org/1999/02/22-rdf-syntax-ns#nil"/>
    <rdf:first>Relative</rdf:first>
  </rdf:Description>
  <rdf:Description rdf:about="#visualization">
    <vs:term_status>stable</vs:term_status>
    <rdfs:label>Visualization</rdfs:label>
    <rdfs:comment xml:lang="en">Visualization, an example of IDM purpose from BS EN 17412-1 (2020) - Annex B</rdfs:comment>
    <rdf:type rdf:resource="#Purpose"/>
  </rdf:Description>
  <rdf:Description rdf:nodeID="A86">
    <owl:onProperty rdf:resource="#hasIdentifier"/>
    <owl:cardinality rdf:datatype="http://www.w3.org/2001/XMLSchema#nonNegativeInteger">1</owl:cardinality>
    <rdf:type rdf:resource="http://www.w3.org/2002/07/owl#Restriction"/>
  </rdf:Description>
  <rdf:Description rdf:about="https://w3id.org/loin/v2/ids#Classification">
    <vs:term_status>stable</vs:term_status>
    <owl:equivalentClass rdf:resource="#Identification"/>
    <rdfs:subClassOf rdf:resource="https://w3id.org/loin/v2/ids#FacetDefinition"/>
    <rdfs:label xml:lang="en">Classification of IDS</rdfs:label>
    <rdfs:comment xml:lang="en">Classification is is a facet of Information Delivery Specification (IDS), a standard developed by buildingSMART International. In this ontology, it is defined as an equivalent class of Indentification according to BS EN 17412-1</rdfs:comment>
    <rdf:type rdf:resource="http://www.w3.org/2002/07/owl#Class"/>
  </rdf:Description>
  <rdf:Description rdf:nodeID="A87">
    <owl:onProperty rdf:resource="https://w3id.org/loin/v2/icdd#isRelatedToContainerDocument"/>
    <owl:maxCardinality rdf:datatype="http://www.w3.org/2001/XMLSchema#nonNegativeInteger">1</owl:maxCardinality>
    <rdf:type rdf:resource="http://www.w3.org/2002/07/owl#Restriction"/>
  </rdf:Description>
  <rdf:Description rdf:nodeID="A88">
    <owl:onProperty rdf:resource="#specifiedByIdentifier"/>
    <owl:minCardinality rdf:datatype="http://www.w3.org/2001/XMLSchema#nonNegativeInteger">1</owl:minCardinality>
    <rdf:type rdf:resource="http://www.w3.org/2002/07/owl#Restriction"/>
  </rdf:Description>
  <rdf:Description rdf:about="#hasSpecificationPerObjectType">
    <vs:term_status>stable</vs:term_status>
    <rdfs:subPropertyOf rdf:resource="http://www.w3.org/2002/07/owl#topObjectProperty"/>
    <rdfs:range rdf:resource="#SpecificationPerObjectType"/>
    <rdfs:label xml:lang="en">has specification per object type</rdfs:label>
    <rdfs:domain rdf:resource="#Specification"/>
    <rdfs:comment xml:lang="en">The object property relates the specification with the specification per object type according to ISO 7817</rdfs:comment>
    <rdf:type rdf:resource="http://www.w3.org/2002/07/owl#ObjectProperty"/>
  </rdf:Description>
  <rdf:Description rdf:about="#Information">
    <rdfs:subClassOf rdf:resource="http://www.w3.org/2002/07/owl#Thing"/>
    <rdfs:label xml:lang="en">Information</rdfs:label>
    <rdfs:comment xml:lang="en">Proxy class for the three information specifications Alphanumerical Information, Geometrical Information, and Documentation</rdfs:comment>
    <rdf:type rdf:resource="http://www.w3.org/2000/01/rdf-schema#Class"/>
  </rdf:Description>
  <rdf:Description rdf:about="#BreakdownStructure">
    <vs:term_status>stable</vs:term_status>
    <rdfs:subClassOf rdf:nodeID="A86"/>
    <rdfs:subClassOf rdf:resource="http://www.w3.org/2002/07/owl#Thing"/>
    <rdfs:label xml:lang="en">Breakdown structure</rdfs:label>
    <rdfs:comment xml:lang="en">Breakdown structure is a term for positioning the object in a structure according to BS EN 17412-1 (2020)</rdfs:comment>
    <rdf:type rdf:resource="http://www.w3.org/2002/07/owl#Class"/>
  </rdf:Description>
  <rdf:Description rdf:nodeID="A82">
    <rdf:rest rdf:nodeID="A89"/>
    <rdf:first>L3</rdf:first>
  </rdf:Description>
  <rdf:Description rdf:nodeID="A90">
    <owl:onProperty rdf:resource="#receivingActor"/>
    <owl:onDataRange rdf:resource="http://www.w3.org/2001/XMLSchema#string"/>
    <owl:maxQualifiedCardinality rdf:datatype="http://www.w3.org/2001/XMLSchema#nonNegativeInteger">1</owl:maxQualifiedCardinality>
    <rdf:type rdf:resource="http://www.w3.org/2002/07/owl#Restriction"/>
  </rdf:Description>
  <rdf:Description rdf:nodeID="A91">
    <owl:oneOf rdf:nodeID="A92"/>
    <rdf:type rdf:resource="http://www.w3.org/2000/01/rdf-schema#Datatype"/>
  </rdf:Description>
  <rdf:Description rdf:nodeID="A93">
    <owl:onProperty rdf:resource="#hasBreakdownStructure"/>
    <owl:minCardinality rdf:datatype="http://www.w3.org/2001/XMLSchema#nonNegativeInteger">1</owl:minCardinality>
    <rdf:type rdf:resource="http://www.w3.org/2002/07/owl#Restriction"/>
  </rdf:Description>
  <rdf:Description rdf:nodeID="A94">
    <rdf:rest rdf:nodeID="A95"/>
    <rdf:first>Absolute</rdf:first>
  </rdf:Description>
  <rdf:Description rdf:nodeID="A96">
    <owl:onProperty rdf:resource="#belongsToInformationContent"/>
    <owl:maxCardinality rdf:datatype="http://www.w3.org/2001/XMLSchema#nonNegativeInteger">1</owl:maxCardinality>
    <rdf:type rdf:resource="http://www.w3.org/2002/07/owl#Restriction"/>
  </rdf:Description>
  <rdf:Description rdf:about="#Bounds">
    <vs:term_status>stable</vs:term_status>
    <rdfs:label xml:lang="en">Bounds restriction</rdfs:label>
    <rdfs:comment xml:lang="en">Bounds restriction specifies that the value is a number and has to fall within a range of values. It is defined by complex restriction of IDS. In this ontology, it is defined as a restriction type, which specifies the restriction formulation.</rdfs:comment>
    <rdf:type rdf:resource="https://w3id.org/loin/v2/ids#RestrictionType"/>
  </rdf:Description>
  <rdf:Description rdf:nodeID="A97">
    <rdf:rest rdf:nodeID="A98"/>
    <rdf:first>NotRequested</rdf:first>
  </rdf:Description>
  <rdf:Description rdf:nodeID="A51">
    <rdf:rest rdf:nodeID="A99"/>
    <rdf:first>ConstructiveGeometry</rdf:first>
  </rdf:Description>
  <rdf:Description rdf:about="#Actor">
    <vs:term_status>stable</vs:term_status>
    <rdfs:subClassOf rdf:resource="http://www.w3.org/2002/07/owl#Thing"/>
    <rdfs:label>Actor</rdfs:label>
    <rdfs:comment xml:lang="en">Actor is a contextual aspect according to BS EN 17412-1 (2020)</rdfs:comment>
    <rdf:type rdf:resource="http://www.w3.org/2002/07/owl#Class"/>
  </rdf:Description>
  <rdf:Description rdf:about="#DocumentSpecification">
    <vs:term_status>stable</vs:term_status>
    <rdfs:subClassOf rdf:resource="http://www.w3.org/2002/07/owl#Thing"/>
    <rdfs:label xml:lang="en">Document specification</rdfs:label>
    <rdfs:comment xml:lang="en">Additional specification of document for information need according to ISO 7817-3</rdfs:comment>
    <rdf:type rdf:resource="http://www.w3.org/2002/07/owl#Class"/>
  </rdf:Description>
  <rdf:Description rdf:nodeID="A100">
    <owl:onProperty rdf:resource="https://w3id.org/loin/v2/ids#hasApplicability"/>
    <owl:minCardinality rdf:datatype="http://www.w3.org/2001/XMLSchema#nonNegativeInteger">1</owl:minCardinality>
    <rdf:type rdf:resource="http://www.w3.org/2002/07/owl#Restriction"/>
  </rdf:Description>
  <rdf:Description rdf:nodeID="A72">
    <owl:onProperty rdf:resource="https://w3id.org/tempo#conceptGUID"/>
    <owl:onDataRange rdf:resource="https://w3id.org/tempo#GUIDType"/>
    <owl:minQualifiedCardinality rdf:datatype="http://www.w3.org/2001/XMLSchema#nonNegativeInteger">1</owl:minQualifiedCardinality>
    <rdf:type rdf:resource="http://www.w3.org/2002/07/owl#Restriction"/>
  </rdf:Description>
  <rdf:Description rdf:nodeID="A66">
    <owl:onProperty rdf:resource="https://w3id.org/tempo#conceptGUID"/>
    <owl:onDataRange rdf:resource="https://w3id.org/tempo#GUIDType"/>
    <owl:maxQualifiedCardinality rdf:datatype="http://www.w3.org/2001/XMLSchema#nonNegativeInteger">1</owl:maxQualifiedCardinality>
    <rdf:type rdf:resource="http://www.w3.org/2002/07/owl#Restriction"/>
  </rdf:Description>
  <rdf:Description rdf:nodeID="A26">
    <owl:onProperty rdf:resource="https://w3id.org/tempo#conceptGUID"/>
    <owl:onDataRange rdf:resource="https://w3id.org/tempo#GUIDType"/>
    <owl:maxQualifiedCardinality rdf:datatype="http://www.w3.org/2001/XMLSchema#nonNegativeInteger">1</owl:maxQualifiedCardinality>
    <rdf:type rdf:resource="http://www.w3.org/2002/07/owl#Restriction"/>
  </rdf:Description>
  <rdf:Description rdf:about="#Identification">
    <vs:term_status>stable</vs:term_status>
    <rdfs:subClassOf rdf:nodeID="A93"/>
    <rdfs:subClassOf rdf:resource="http://www.w3.org/2002/07/owl#Thing"/>
    <rdfs:label xml:lang="en">Identification</rdfs:label>
    <rdfs:comment xml:lang="en">Identification is a term for positioning the object in a breakdown structure according to BS EN 17412-1 (2020)</rdfs:comment>
    <rdf:type rdf:resource="http://www.w3.org/2002/07/owl#Class"/>
  </rdf:Description>
  <rdf:Description rdf:about="#SpecificationInstance">
    <vs:term_status>stable</vs:term_status>
    <rdfs:label xml:lang="en">Specification</rdfs:label>
    <rdfs:comment xml:lang="en">Documents such as technical specifications according to notes according to notes of BS EN 17412-1 (2020)</rdfs:comment>
    <rdf:type rdf:resource="#DocumentContent"/>
  </rdf:Description>
  <rdf:Description rdf:about="#hasGeometricalInformation">
    <vs:term_status>stable</vs:term_status>
    <rdfs:subPropertyOf rdf:resource="#hasInformation"/>
    <rdfs:range rdf:resource="#GeometricalInformation"/>
    <rdfs:label xml:lang="en">has geometrical information</rdfs:label>
    <rdfs:domain rdf:resource="#SpecificationPerObjectType"/>
    <rdfs:comment xml:lang="en">The object property relates the geometrical information with a LOIN object according to ISO 7817-3</rdfs:comment>
    <rdf:type rdf:resource="http://www.w3.org/2002/07/owl#ObjectProperty"/>
  </rdf:Description>
  <rdf:Description rdf:about="#specifiedByIdentifier">
    <vs:term_status>stable</vs:term_status>
    <rdfs:subPropertyOf rdf:resource="http://www.w3.org/2002/07/owl#topObjectProperty"/>
    <rdfs:range rdf:resource="#Identifier"/>
    <rdfs:label>specified by identifier</rdfs:label>
    <rdfs:domain rdf:resource="#InformationContent"/>
    <rdf:type rdf:resource="http://www.w3.org/2002/07/owl#ObjectProperty"/>
  </rdf:Description>
  <rdf:Description rdf:about="#hasParametricBehaviour">
    <vs:term_status>stable</vs:term_status>
    <rdfs:subPropertyOf rdf:resource="http://www.w3.org/2002/07/owl#topDataProperty"/>
    <rdfs:range rdf:nodeID="A101"/>
    <rdfs:label xml:lang="en">has parametric behaviour</rdfs:label>
    <rdfs:domain rdf:resource="#ParametricBehaviour"/>
    <rdf:type rdf:resource="http://www.w3.org/2002/07/owl#DatatypeProperty"/>
  </rdf:Description>
  <rdf:Description rdf:nodeID="A23">
    <owl:qualifiedCardinality rdf:datatype="http://www.w3.org/2001/XMLSchema#nonNegativeInteger">1</owl:qualifiedCardinality>
    <owl:onProperty rdf:resource="#requested"/>
    <owl:onDataRange rdf:resource="http://www.w3.org/2001/XMLSchema#boolean"/>
    <rdf:type rdf:resource="http://www.w3.org/2002/07/owl#Restriction"/>
  </rdf:Description>
  <rdf:Description rdf:nodeID="A102">
    <owl:onProperty rdf:resource="#hasDescriptionInLanguage"/>
    <owl:cardinality rdf:datatype="http://www.w3.org/2001/XMLSchema#nonNegativeInteger">1</owl:cardinality>
    <rdf:type rdf:resource="http://www.w3.org/2002/07/owl#Restriction"/>
  </rdf:Description>
  <rdf:Description rdf:nodeID="A103">
    <owl:oneOf rdf:nodeID="A104"/>
    <rdf:type rdf:resource="http://www.w3.org/2000/01/rdf-schema#Datatype"/>
  </rdf:Description>
  <rdf:Description rdf:about="https://w3id.org/loin/v2/icdd#isRelatedToContainerLinkset">
    <vs:term_status>stable</vs:term_status>
    <rdfs:range rdf:resource="https://standards.iso.org/iso/21597/-1/ed-1/en/Container#Linkset"/>
    <rdfs:label xml:lang="en">is related to container linkset</rdfs:label>
    <rdfs:domain rdf:resource="#RequiredDocument"/>
    <rdfs:comment xml:lang="en">The object property is an extension with ICDD. It relates ontological document defined by BS EN 17412-1(2020) with container linkset or data set</rdfs:comment>
    <rdf:type rdf:resource="http://www.w3.org/2002/07/owl#ObjectProperty"/>
  </rdf:Description>
  <rdf:Description rdf:nodeID="A105">
    <owl:onProperty rdf:resource="#hasUnit"/>
    <owl:minCardinality rdf:datatype="http://www.w3.org/2001/XMLSchema#nonNegativeInteger">0</owl:minCardinality>
    <rdf:type rdf:resource="http://www.w3.org/2002/07/owl#Restriction"/>
  </rdf:Description>
  <rdf:Description rdf:about="#Pattern">
    <vs:term_status>stable</vs:term_status>
    <rdfs:label xml:lang="en">Pattern restriction</rdfs:label>
    <rdfs:comment xml:lang="en">Pattern restriction with regex method specifies advanced pattern matching. In this ontology, it is defined as a restriction type, which specifies the restriction formulation.</rdfs:comment>
    <rdf:type rdf:resource="https://w3id.org/loin/v2/ids#RestrictionType"/>
  </rdf:Description>
  <rdf:Description rdf:nodeID="A106">
    <owl:someValuesFrom rdf:resource="#Dimensionality"/>
    <owl:onProperty rdf:resource="#hasGeometrySpecification"/>
    <rdf:type rdf:resource="http://www.w3.org/2002/07/owl#Restriction"/>
  </rdf:Description>
  <rdf:Description rdf:nodeID="A107">
    <owl:onProperty rdf:resource="https://w3id.org/tempo#conceptGUID"/>
    <owl:onDataRange rdf:resource="https://w3id.org/tempo#GUIDType"/>
    <owl:minQualifiedCardinality rdf:datatype="http://www.w3.org/2001/XMLSchema#nonNegativeInteger">1</owl:minQualifiedCardinality>
    <rdf:type rdf:resource="http://www.w3.org/2002/07/owl#Restriction"/>
  </rdf:Description>
  <rdf:Description rdf:nodeID="A108">
    <owl:someValuesFrom rdf:resource="#DocumentType"/>
    <owl:onProperty rdf:resource="#hasDocumentSpecification"/>
    <rdf:type rdf:resource="http://www.w3.org/2002/07/owl#Restriction"/>
  </rdf:Description>
  <rdf:Description rdf:about="#costEstimation">
    <vs:term_status>stable</vs:term_status>
    <rdfs:label xml:lang="en">Cost estimation</rdfs:label>
    <rdfs:comment xml:lang="en">Cost estimation, an example of IDM purpose from BS EN 17412-1 (2020) - Annex B</rdfs:comment>
    <rdf:type rdf:resource="#Purpose"/>
  </rdf:Description>
  <rdf:Description rdf:about="#SimpleValue">
    <vs:term_status>stable</vs:term_status>
    <rdfs:label xml:lang="en">Simple value restriction</rdfs:label>
    <rdfs:comment xml:lang="en">Simple value restriction specifies the exact allowed value. In this ontology, it is defined as a restriction type, which specifies the restriction formulation.</rdfs:comment>
    <rdf:type rdf:resource="https://w3id.org/loin/v2/ids#RestrictionType"/>
  </rdf:Description>
  <rdf:Description rdf:nodeID="A109">
    <rdf:rest rdf:nodeID="A81"/>
    <rdf:first>L1</rdf:first>
  </rdf:Description>
  <rdf:Description rdf:about="#hasInformationContent">
    <vs:term_status>stable</vs:term_status>
    <rdfs:subPropertyOf rdf:resource="http://www.w3.org/2002/07/owl#topObjectProperty"/>
    <rdfs:range rdf:resource="#InformationContent"/>
    <rdfs:label xml:lang="en">has alphanumerical informaton content</rdfs:label>
    <rdfs:domain rdf:resource="#AlphanumericalInformation"/>
    <rdfs:comment xml:lang="en">The object property relates the detailed content with alphanumerical information according to BS EN 17412-1 (2020)</rdfs:comment>
    <rdf:type rdf:resource="http://www.w3.org/2002/07/owl#ObjectProperty"/>
  </rdf:Description>
  <rdf:Description rdf:about="#AlphanumericalInformation">
    <rdfs:subClassOf rdf:resource="#Information"/>
    <rdfs:subClassOf rdf:nodeID="A59"/>
    <rdfs:subClassOf rdf:nodeID="A53"/>
    <rdfs:comment xml:lang="en">Alphanumerical information is a term for specifying the information need according to ISO 7817-3</rdfs:comment>
    <vs:term_status>stable</vs:term_status>
    <rdfs:subClassOf rdf:nodeID="A107"/>
    <rdfs:subClassOf rdf:nodeID="A27"/>
    <rdfs:subClassOf rdf:nodeID="A85"/>
    <rdf:type rdf:resource="http://www.w3.org/2002/07/owl#Class"/>
    <rdfs:subClassOf rdf:nodeID="A105"/>
    <rdfs:label xml:lang="en">Alphanumerical information</rdfs:label>
    <rdfs:subClassOf rdf:nodeID="A110"/>
    <rdfs:subClassOf rdf:nodeID="A58"/>
  </rdf:Description>
  <rdf:Description rdf:about="#hasInformation">
    <rdfs:subPropertyOf rdf:resource="http://www.w3.org/2002/07/owl#topObjectProperty"/>
    <rdfs:range rdf:resource="#Information"/>
    <rdfs:label xml:lang="en">has information</rdfs:label>
    <rdfs:domain rdf:resource="#SpecificationPerObjectType"/>
    <rdfs:comment xml:lang="en">Proxy property for the three information specification relationships</rdfs:comment>
    <rdf:type rdf:resource="http://www.w3.org/2002/07/owl#ObjectProperty"/>
  </rdf:Description>
  <rdf:Description rdf:nodeID="A111">
    <owl:onProperty rdf:resource="#hasObjectType"/>
    <owl:minCardinality rdf:datatype="http://www.w3.org/2001/XMLSchema#nonNegativeInteger">1</owl:minCardinality>
    <rdf:type rdf:resource="http://www.w3.org/2002/07/owl#Restriction"/>
  </rdf:Description>
  <rdf:Description rdf:about="#Signed_Document">
    <vs:term_status>stable</vs:term_status>
    <rdfs:label xml:lang="en">Signed document</rdfs:label>
    <rdfs:comment xml:lang="en">Documents such as test certificates, insurance policies, delivery notes according to notes of BS EN 17412-1 (2020)</rdfs:comment>
    <rdf:type rdf:resource="#DocumentContent"/>
  </rdf:Description>
  <rdf:Description rdf:nodeID="A112">
    <owl:onProperty rdf:resource="#hasDescriptionInLanguage"/>
    <owl:cardinality rdf:datatype="http://www.w3.org/2001/XMLSchema#nonNegativeInteger">1</owl:cardinality>
    <rdf:type rdf:resource="http://www.w3.org/2002/07/owl#Restriction"/>
  </rdf:Description>
  <rdf:Description rdf:nodeID="A113">
    <owl:onProperty rdf:resource="https://w3id.org/loin/v2/ids#restrictionFormulation"/>
    <owl:cardinality rdf:datatype="http://www.w3.org/2001/XMLSchema#nonNegativeInteger">1</owl:cardinality>
    <rdf:type rdf:resource="http://www.w3.org/2002/07/owl#Restriction"/>
  </rdf:Description>
  <rdf:Description rdf:about="#hasIdentification">
    <vs:term_status>stable</vs:term_status>
    <rdfs:subPropertyOf rdf:resource="http://www.w3.org/2002/07/owl#topObjectProperty"/>
    <rdfs:range rdf:resource="#Identification"/>
    <rdfs:label xml:lang="en">has identification</rdfs:label>
    <rdfs:domain rdf:resource="#AlphanumericalInformation"/>
    <rdfs:comment xml:lang="en">The object property relates the identification of a breakdown structure with an alphanumerical information according to BS EN 17412-1 (2020)</rdfs:comment>
    <rdf:type rdf:resource="http://www.w3.org/2002/07/owl#ObjectProperty"/>
  </rdf:Description>
  <rdf:Description rdf:about="https://w3id.org/loin/v2/ids#restrictionFormulation">
    <vs:term_status>stable</vs:term_status>
    <rdfs:range rdf:resource="http://www.w3.org/2001/XMLSchema#string"/>
    <rdfs:label xml:lang="en">Constraint text formulated for facet parameters</rdfs:label>
    <rdfs:domain rdf:resource="https://w3id.org/loin/v2/ids#FacetParameter"/>
    <rdfs:comment xml:lang="en">Restriction formulation is for formulating facet parameter value, that is used by IDS definition.</rdfs:comment>
    <rdf:type rdf:resource="http://www.w3.org/2002/07/owl#DatatypeProperty"/>
  </rdf:Description>
  <rdf:Description rdf:nodeID="A0">
    <owl:onProperty rdf:resource="#hasSpecification"/>
    <owl:maxCardinality rdf:datatype="http://www.w3.org/2001/XMLSchema#nonNegativeInteger">0</owl:maxCardinality>
    <rdf:type rdf:resource="http://www.w3.org/2002/07/owl#Restriction"/>
  </rdf:Description>
  <rdf:Description rdf:nodeID="A114">
    <owl:onProperty rdf:resource="#informationDeliveryMilestone"/>
    <owl:onDataRange rdf:resource="http://www.w3.org/2001/XMLSchema#string"/>
    <owl:maxQualifiedCardinality rdf:datatype="http://www.w3.org/2001/XMLSchema#nonNegativeInteger">1</owl:maxQualifiedCardinality>
    <rdf:type rdf:resource="http://www.w3.org/2002/07/owl#Restriction"/>
  </rdf:Description>
  <rdf:Description rdf:about="#SendingActor">
    <vs:term_status>stable</vs:term_status>
    <rdfs:subClassOf rdf:resource="#Actor"/>
    <rdfs:label xml:lang="en">Sending actor</rdfs:label>
    <rdfs:comment xml:lang="en">Sending actor is a party for information delivery according to ISO 19650-1 (2018)</rdfs:comment>
    <rdf:type rdf:resource="http://www.w3.org/2002/07/owl#Class"/>
  </rdf:Description>
  <rdf:Description rdf:nodeID="A115">
    <rdf:rest rdf:resource="http://www.w3.org/1999/02/22-rdf-syntax-ns#nil"/>
    <rdf:first rdf:resource="#OntologyDataDefinition"/>
  </rdf:Description>
  <rdf:Description rdf:nodeID="A116">
    <owl:oneOf rdf:nodeID="A62"/>
    <rdf:type rdf:resource="http://www.w3.org/2000/01/rdf-schema#Datatype"/>
  </rdf:Description>
  <rdf:Description rdf:about="https://w3id.org/loin/v2/ids#Entity">
    <vs:term_status>stable</vs:term_status>
    <rdfs:subClassOf rdf:nodeID="A117"/>
    <rdfs:subClassOf rdf:resource="https://w3id.org/loin/v2/ids#FacetDefinition"/>
    <rdfs:label xml:lang="en">Entity</rdfs:label>
    <rdfs:comment xml:lang="en">Entity is a facet of Information Delivery Specification (IDS), a standard developed by buildingSMART International</rdfs:comment>
    <rdf:type rdf:resource="http://www.w3.org/2002/07/owl#Class"/>
  </rdf:Description>
  <rdf:Description rdf:nodeID="A70">
    <owl:onProperty rdf:resource="#hasDescriptionInLanguage"/>
    <owl:onDataRange rdf:resource="http://www.w3.org/1999/02/22-rdf-syntax-ns#langString"/>
    <owl:maxQualifiedCardinality rdf:datatype="http://www.w3.org/2001/XMLSchema#nonNegativeInteger">0</owl:maxQualifiedCardinality>
    <rdf:type rdf:resource="http://www.w3.org/2002/07/owl#Restriction"/>
  </rdf:Description>
  <rdf:Description rdf:nodeID="A118">
    <rdf:rest rdf:resource="http://www.w3.org/1999/02/22-rdf-syntax-ns#nil"/>
    <rdf:first>L5</rdf:first>
  </rdf:Description>
  <rdf:Description rdf:nodeID="A43">
    <schema:memberOf rdf:nodeID="A83"/>
    <schema:name>Liu Liu</schema:name>
    <schema:email rdf:resource="mailto:liu.liu-m6r@rub.de"/>
    <rdf:type rdf:resource="https://schema.org/Person"/>
    <schema:identifier rdf:resource="https://orcid.org/0000-0001-5907-7609"/>
  </rdf:Description>
  <rdf:Description rdf:about="#hasDescriptionInLanguage">
    <owl:equivalentProperty rdf:resource="https://w3id.org/isoprops#hasDescriptionInLanguage"/>
    <rdfs:subPropertyOf rdf:resource="http://www.w3.org/2002/07/owl#topDataProperty"/>
    <rdfs:range rdf:resource="http://www.w3.org/1999/02/22-rdf-syntax-ns#langString"/>
    <rdfs:label xml:lang="en">Description in Language</rdfs:label>
    <rdf:type rdf:resource="http://www.w3.org/2002/07/owl#DatatypeProperty"/>
  </rdf:Description>
  <rdf:Description rdf:about="#DocumentType">
    <vs:term_status>stable</vs:term_status>
    <rdfs:subClassOf rdf:resource="#DocumentSpecification"/>
    <rdfs:label xml:lang="en">Document type</rdfs:label>
    <rdfs:comment xml:lang="en">Specifies the file typ of the required document</rdfs:comment>
    <rdf:type rdf:resource="http://www.w3.org/2002/07/owl#Class"/>
  </rdf:Description>
  <rdf:Description rdf:about="#GeometrySpecification">
    <vs:term_status>stable</vs:term_status>
    <rdfs:subClassOf rdf:resource="http://www.w3.org/2002/07/owl#Thing"/>
    <rdfs:label xml:lang="en">Geometrical information specification</rdfs:label>
    <rdfs:comment xml:lang="en">Additional specification of geometrical information for information need according to BS EN 17412-1 (2020)</rdfs:comment>
    <rdf:type rdf:resource="http://www.w3.org/2002/07/owl#Class"/>
  </rdf:Description>
  <rdf:Description rdf:nodeID="A101">
    <owl:oneOf rdf:nodeID="A119"/>
    <rdf:type rdf:resource="http://www.w3.org/2000/01/rdf-schema#Datatype"/>
  </rdf:Description>
  <rdf:Description rdf:about="#Handdrawn_Sketches">
    <vs:term_status>stable</vs:term_status>
    <rdfs:label xml:lang="en">Handdrawn sketches</rdfs:label>
    <rdfs:comment xml:lang="en">Documents such as such as initial sketches, site plans according to notes of BS EN 17412-1 (2020)</rdfs:comment>
    <rdf:type rdf:resource="#DocumentContent"/>
  </rdf:Description>
  <rdf:Description rdf:nodeID="A104">
    <rdf:rest rdf:nodeID="A94"/>
    <rdf:first>NotRequested</rdf:first>
  </rdf:Description>
  <rdf:Description rdf:about="#hasIntendedUse">
    <owl:equivalentProperty rdf:resource="https://w3id.org/tempo#hasIntendedUse"/>
    <rdfs:subPropertyOf rdf:resource="http://www.w3.org/2002/07/owl#topObjectProperty"/>
    <rdfs:range rdf:resource="https://w3id.org/tempo#IntendedUse"/>
    <rdfs:label xml:lang="en">has Intended Use</rdfs:label>
    <rdfs:domain rdf:resource="#AlphanumericalInformation"/>
    <rdfs:comment xml:lang="en">The object property relates the alphanumerical information with the intened use</rdfs:comment>
    <rdf:type rdf:resource="http://www.w3.org/2002/07/owl#ObjectProperty"/>
  </rdf:Description>
  <rdf:Description rdf:nodeID="A42">
    <schema:identifier rdf:resource="https://orcid.org/0000-0001-6058-7614"/>
    <rdf:type rdf:resource="https://schema.org/Person"/>
    <schema:memberOf rdf:nodeID="A120"/>
    <schema:email rdf:resource="mailto:sven.zentgraf@rub.de"/>
    <schema:name>Sven Zentgraf</schema:name>
  </rdf:Description>
  <rdf:Description rdf:nodeID="A121">
    <rdf:rest rdf:nodeID="A1"/>
    <rdf:first>L1</rdf:first>
  </rdf:Description>
  <rdf:Description rdf:nodeID="A122">
    <owl:onProperty rdf:resource="https://w3id.org/loin/v2/ids#hasPropertyName"/>
    <owl:cardinality rdf:datatype="http://www.w3.org/2001/XMLSchema#nonNegativeInteger">1</owl:cardinality>
    <rdf:type rdf:resource="http://www.w3.org/2002/07/owl#Restriction"/>
  </rdf:Description>
  <rdf:Description rdf:about="#hasDocumentSpecification">
    <vs:term_status>stable</vs:term_status>
    <rdfs:subPropertyOf rdf:resource="http://www.w3.org/2002/07/owl#topObjectProperty"/>
    <rdfs:range rdf:resource="#DocumentSpecification"/>
    <rdfs:label xml:lang="en">has documentaton specification</rdfs:label>
    <rdfs:domain rdf:resource="#RequiredDocument"/>
    <rdfs:comment xml:lang="en">The object property relates the document specifications with a document according to ISO 7817-3</rdfs:comment>
    <rdf:type rdf:resource="http://www.w3.org/2002/07/owl#ObjectProperty"/>
  </rdf:Description>
  <rdf:Description rdf:nodeID="A123">
    <owl:onProperty rdf:resource="#hasBreakdownStructure"/>
    <owl:cardinality rdf:datatype="http://www.w3.org/2001/XMLSchema#nonNegativeInteger">1</owl:cardinality>
    <rdf:type rdf:resource="http://www.w3.org/2002/07/owl#Restriction"/>
  </rdf:Description>
  <rdf:Description rdf:about="#hasRequirementType">
    <vs:term_status>stable</vs:term_status>
    <rdfs:subPropertyOf rdf:resource="http://www.w3.org/2002/07/owl#topObjectProperty"/>
    <rdfs:range rdf:resource="https://w3id.org/loin/v2/ids#RequirementType"/>
    <rdfs:label xml:lang="en">has requirement type</rdfs:label>
    <rdfs:domain rdf:resource="https://w3id.org/loin/v2/ids#FacetDefinition"/>
    <rdfs:comment xml:lang="en">relates the requirement type with the defined requirements in IDS data definition</rdfs:comment>
    <rdf:type rdf:resource="http://www.w3.org/2002/07/owl#ObjectProperty"/>
  </rdf:Description>
  <rdf:Description rdf:nodeID="A50">
    <rdf:rest rdf:nodeID="A109"/>
    <rdf:first>NotRequested</rdf:first>
  </rdf:Description>
  <rdf:Description rdf:about="#parametric">
    <vs:term_status>stable</vs:term_status>
    <rdfs:label xml:lang="en">parametric</rdfs:label>
    <rdfs:comment xml:lang="en">Parametric, an example of parametric behaviour according to notes of geometrical information specification for information need in BS EN 17412-1 (2020)</rdfs:comment>
    <rdf:type rdf:resource="#ParametricBehaviour"/>
  </rdf:Description>
  <rdf:Description rdf:nodeID="A25">
    <owl:onProperty rdf:resource="#hasDocument"/>
    <owl:onClass rdf:resource="#RequiredDocument"/>
    <owl:minQualifiedCardinality rdf:datatype="http://www.w3.org/2001/XMLSchema#nonNegativeInteger">0</owl:minQualifiedCardinality>
    <rdf:type rdf:resource="http://www.w3.org/2002/07/owl#Restriction"/>
  </rdf:Description>
  <rdf:Description rdf:about="#Functional">
    <vs:term_status>stable</vs:term_status>
    <rdfs:label xml:lang="en">Functional structure</rdfs:label>
    <rdfs:comment xml:lang="en">An example of breakdown structure type according to BS EN 17412-1 (2020)</rdfs:comment>
    <rdf:type rdf:resource="#BreakdownStructureType"/>
  </rdf:Description>
  <rdf:Description rdf:about="#hasSendingActor">
    <vs:term_status>stable</vs:term_status>
    <rdfs:subPropertyOf rdf:resource="http://www.w3.org/2002/07/owl#topObjectProperty"/>
    <rdfs:range rdf:resource="#SendingActor"/>
    <rdfs:label xml:lang="en">has Sending Actor</rdfs:label>
    <rdfs:domain rdf:resource="#Prerequisites"/>
    <rdfs:comment xml:lang="en">The object property relates the  with the sending actor  according to ISO 7817</rdfs:comment>
    <rdf:type rdf:resource="http://www.w3.org/2002/07/owl#ObjectProperty"/>
  </rdf:Description>
  <rdf:Description rdf:about="https://w3id.org/loin/v2/ids#FacetDefinition">
    <vs:term_status>stable</vs:term_status>
    <rdfs:subClassOf rdf:resource="http://www.w3.org/2000/01/rdf-schema#Resource"/>
    <rdfs:label xml:lang="en">IDS facet definition</rdfs:label>
    <rdfs:comment xml:lang="en">IDS facet definition is used to define a facet to apply the requirement or to require the information according to IDS standard developed by buildingSMART International</rdfs:comment>
    <rdf:type rdf:resource="http://www.w3.org/2002/07/owl#Class"/>
  </rdf:Description>
  <rdf:Description rdf:about="#value">
    <vs:term_status>stable</vs:term_status>
    <rdfs:subPropertyOf rdf:resource="http://www.w3.org/2002/07/owl#topDataProperty"/>
    <rdfs:label xml:lang="en">value</rdfs:label>
    <rdfs:comment xml:lang="en">value for general definition</rdfs:comment>
    <rdf:type rdf:resource="http://www.w3.org/2002/07/owl#DatatypeProperty"/>
  </rdf:Description>
  <rdf:Description rdf:about="#Appearance">
    <vs:term_status>stable</vs:term_status>
    <rdfs:subClassOf rdf:nodeID="A124"/>
    <rdfs:subClassOf rdf:resource="#GeometrySpecification"/>
    <rdfs:label xml:lang="en">Appearance</rdfs:label>
    <rdfs:comment xml:lang="en">Appearance as a geometrical information specification for information need according to ISO 7817-3</rdfs:comment>
    <rdf:type rdf:resource="http://www.w3.org/2002/07/owl#Class"/>
  </rdf:Description>
  <rdf:Description rdf:about="https://w3id.org/loin/v2/ids#RequirementType">
    <vs:term_status>stable</vs:term_status>
    <owl:oneOf rdf:nodeID="A125"/>
    <rdfs:subClassOf rdf:resource="http://www.w3.org/2000/01/rdf-schema#Resource"/>
    <rdfs:label xml:lang="en">IDS requirement type</rdfs:label>
    <rdfs:comment xml:lang="en">IDS requirement type is used to specify a requirement, if it is optional or mandatory according to IDS standard developed by buildingSMART International</rdfs:comment>
    <rdf:type rdf:resource="http://www.w3.org/2002/07/owl#Class"/>
  </rdf:Description>
  <rdf:Description rdf:nodeID="A8">
    <owl:qualifiedCardinality rdf:datatype="http://www.w3.org/2001/XMLSchema#nonNegativeInteger">1</owl:qualifiedCardinality>
    <owl:onProperty rdf:resource="#hasDimensionality"/>
    <owl:onDataRange rdf:nodeID="A56"/>
    <rdf:type rdf:resource="http://www.w3.org/2002/07/owl#Restriction"/>
  </rdf:Description>
  <rdf:Description rdf:nodeID="A126">
    <owl:onProperty rdf:resource="https://w3id.org/tempo#conceptGUID"/>
    <owl:onDataRange rdf:resource="https://w3id.org/tempo#GUIDType"/>
    <owl:minQualifiedCardinality rdf:datatype="http://www.w3.org/2001/XMLSchema#nonNegativeInteger">0</owl:minQualifiedCardinality>
    <rdf:type rdf:resource="http://www.w3.org/2002/07/owl#Restriction"/>
  </rdf:Description>
  <rdf:Description rdf:nodeID="A127">
    <owl:onProperty rdf:resource="https://w3id.org/tempo#conceptGUID"/>
    <owl:onDataRange rdf:resource="https://w3id.org/tempo#GUIDType"/>
    <owl:maxQualifiedCardinality rdf:datatype="http://www.w3.org/2001/XMLSchema#nonNegativeInteger">1</owl:maxQualifiedCardinality>
    <rdf:type rdf:resource="http://www.w3.org/2002/07/owl#Restriction"/>
  </rdf:Description>
  <rdf:Description rdf:nodeID="A125">
    <rdf:rest rdf:nodeID="A128"/>
    <rdf:first>Required</rdf:first>
  </rdf:Description>
  <rdf:Description rdf:about="#hasSpecification">
    <rdfs:subPropertyOf rdf:resource="http://www.w3.org/2002/07/owl#topObjectProperty"/>
    <rdfs:range rdf:resource="#Specification"/>
    <rdfs:label xml:lang="en">Specification</rdfs:label>
    <rdfs:domain rdf:resource="#LevelOfInformationNeed"/>
    <rdfs:comment xml:lang="en">The object property relates the LOIN with the specification according to ISO 7817</rdfs:comment>
    <rdf:type rdf:resource="http://www.w3.org/2002/07/owl#ObjectProperty"/>
  </rdf:Description>
  <rdf:Description rdf:nodeID="A61">
    <owl:onProperty rdf:resource="https://w3id.org/loin/v2/ids#restrictionFormulation"/>
    <owl:cardinality rdf:datatype="http://www.w3.org/2001/XMLSchema#nonNegativeInteger">1</owl:cardinality>
    <rdf:type rdf:resource="http://www.w3.org/2002/07/owl#Restriction"/>
  </rdf:Description>
  <rdf:Description rdf:nodeID="A129">
    <owl:someValuesFrom rdf:resource="#ParametricBehaviour"/>
    <owl:onProperty rdf:resource="#hasGeometrySpecification"/>
    <rdf:type rdf:resource="http://www.w3.org/2002/07/owl#Restriction"/>
  </rdf:Description>
  <rdf:Description rdf:nodeID="A130">
    <owl:onProperty rdf:resource="#purpose"/>
    <owl:onDataRange rdf:resource="http://www.w3.org/2001/XMLSchema#string"/>
    <owl:maxQualifiedCardinality rdf:datatype="http://www.w3.org/2001/XMLSchema#nonNegativeInteger">1</owl:maxQualifiedCardinality>
    <rdf:type rdf:resource="http://www.w3.org/2002/07/owl#Restriction"/>
  </rdf:Description>
  <rdf:Description rdf:nodeID="A131">
    <owl:someValuesFrom rdf:resource="#Detail"/>
    <owl:onProperty rdf:resource="#hasGeometrySpecification"/>
    <rdf:type rdf:resource="http://www.w3.org/2002/07/owl#Restriction"/>
  </rdf:Description>
  <rdf:Description rdf:about="#Purpose">
    <rdfs:subClassOf rdf:nodeID="A112"/>
    <rdfs:subClassOf rdf:resource="http://www.w3.org/2002/07/owl#Thing"/>
    <rdfs:label>Purpose</rdfs:label>
    <rdfs:comment xml:lang="en">Purpose is a contextual aspect according to ISO 7817-3</rdfs:comment>
    <rdf:type rdf:resource="http://www.w3.org/2002/07/owl#Class"/>
  </rdf:Description>
  <rdf:Description rdf:about="#receivingActor">
    <rdfs:subPropertyOf rdf:resource="http://www.w3.org/2002/07/owl#topDataProperty"/>
    <rdfs:range rdf:resource="http://www.w3.org/2001/XMLSchema#string"/>
    <rdfs:label xml:lang="en">Receiving actor</rdfs:label>
    <rdf:type rdf:resource="http://www.w3.org/2002/07/owl#DatatypeProperty"/>
  </rdf:Description>
  <rdf:Description rdf:about="https://w3id.org/loin/v2/ids#hasApplicability">
    <vs:term_status>stable</vs:term_status>
    <rdfs:range rdf:resource="https://w3id.org/loin/v2/ids#FacetDefinition"/>
    <rdfs:label xml:lang="en">has applicability</rdfs:label>
    <rdfs:domain rdf:resource="https://w3id.org/loin/v2/ids#DataDefinition"/>
    <rdfs:comment xml:lang="en">The object property describes the applicability of a facet for the specification according to IDS definition</rdfs:comment>
    <rdf:type rdf:resource="http://www.w3.org/2002/07/owl#ObjectProperty"/>
  </rdf:Description>
  <rdf:Description rdf:about="#Manual">
    <vs:term_status>stable</vs:term_status>
    <rdfs:label>Manual</rdfs:label>
    <rdfs:comment xml:lang="en">Documents such as maintenance and user manuals according to notes of BS EN 17412-1 (2020)</rdfs:comment>
    <rdf:type rdf:resource="#DocumentContent"/>
  </rdf:Description>
  <rdf:Description rdf:about="#Hard_Copy">
    <vs:term_status>stable</vs:term_status>
    <rdfs:label xml:lang="en">Hand copy</rdfs:label>
    <rdfs:comment xml:lang="en">Documents of geometrical information or alphanumerical information can also be considered as documents according to notes of BS EN 17412-1 (2020).</rdfs:comment>
    <rdf:type rdf:resource="#DocumentContent"/>
  </rdf:Description>
  <rdf:Description rdf:nodeID="A75">
    <owl:onProperty rdf:resource="https://w3id.org/loin/v2/ids#hasRestrictionType"/>
    <owl:cardinality rdf:datatype="http://www.w3.org/2001/XMLSchema#nonNegativeInteger">1</owl:cardinality>
    <rdf:type rdf:resource="http://www.w3.org/2002/07/owl#Restriction"/>
  </rdf:Description>
  <rdf:Description rdf:about="#hasUnit">
    <rdfs:subPropertyOf rdf:resource="http://www.w3.org/2002/07/owl#topObjectProperty"/>
    <rdfs:range rdf:resource="https://w3id.org/tempo#Unit"/>
    <rdfs:label xml:lang="en">The object property relates the alphanumerical information with the unit according to ISO 7817</rdfs:label>
    <rdfs:domain rdf:resource="#AlphanumericalInformation"/>
    <rdf:type rdf:resource="http://www.w3.org/2002/07/owl#ObjectProperty"/>
  </rdf:Description>
  <rdf:Description rdf:about="#hasReceivingActor">
    <vs:term_status>stable</vs:term_status>
    <rdfs:subPropertyOf rdf:resource="http://www.w3.org/2002/07/owl#topObjectProperty"/>
    <rdfs:range rdf:resource="#ReceivingActor"/>
    <rdfs:label xml:lang="en">has receiving actor</rdfs:label>
    <rdfs:domain rdf:resource="#Prerequisites"/>
    <rdfs:comment xml:lang="en">The object property relates the prerequisites with the receiving actor according to ISO 7817-3</rdfs:comment>
    <rdf:type rdf:resource="http://www.w3.org/2002/07/owl#ObjectProperty"/>
  </rdf:Description>
  <rdf:Description rdf:about="#sendingActor">
    <rdfs:subPropertyOf rdf:resource="http://www.w3.org/2002/07/owl#topDataProperty"/>
    <rdfs:range rdf:resource="http://www.w3.org/2001/XMLSchema#string"/>
    <rdfs:label xml:lang="en">Sending actor</rdfs:label>
    <rdf:type rdf:resource="http://www.w3.org/2002/07/owl#DatatypeProperty"/>
  </rdf:Description>
  <rdf:Description rdf:about="#GeometricalInformation">
    <rdfs:subClassOf rdf:nodeID="A131"/>
    <rdfs:comment xml:lang="en">Geometrical information is a term for specifying the information need according to BS EN 17412-1 (2020)</rdfs:comment>
    <rdfs:subClassOf rdf:resource="#Information"/>
    <rdfs:subClassOf rdf:nodeID="A14"/>
    <rdfs:subClassOf rdf:nodeID="A132"/>
    <rdfs:subClassOf rdf:nodeID="A133"/>
    <rdfs:subClassOf rdf:nodeID="A129"/>
    <rdfs:subClassOf rdf:nodeID="A126"/>
    <rdfs:label xml:lang="en">Geometrical information</rdfs:label>
    <vs:term_status>stable</vs:term_status>
    <rdfs:subClassOf rdf:nodeID="A36"/>
    <rdfs:subClassOf rdf:nodeID="A106"/>
    <rdf:type rdf:resource="http://www.w3.org/2002/07/owl#Class"/>
  </rdf:Description>
  <rdf:Description rdf:about="#RequiredDocument">
    <rdfs:label xml:lang="en">Document</rdfs:label>
    <rdfs:subClassOf rdf:nodeID="A134"/>
    <vs:term_status>stable</vs:term_status>
    <rdfs:subClassOf rdf:nodeID="A96"/>
    <rdfs:subClassOf rdf:nodeID="A9"/>
    <rdfs:subClassOf rdf:nodeID="A135"/>
    <rdfs:subClassOf rdf:nodeID="A108"/>
    <rdfs:subClassOf rdf:nodeID="A35"/>
    <rdfs:subClassOf rdf:resource="http://www.w3.org/2002/07/owl#Thing"/>
    <rdfs:comment xml:lang="en">Document is a term for specifying the documentation of information need according to ISO 7817-3</rdfs:comment>
    <rdfs:subClassOf rdf:nodeID="A136"/>
    <rdf:type rdf:resource="http://www.w3.org/2002/07/owl#Class"/>
    <rdfs:subClassOf rdf:nodeID="A87"/>
  </rdf:Description>
  <rdf:Description rdf:nodeID="A132">
    <owl:onProperty rdf:resource="https://w3id.org/tempo#conceptGUID"/>
    <owl:onDataRange rdf:resource="https://w3id.org/tempo#GUIDType"/>
    <owl:maxQualifiedCardinality rdf:datatype="http://www.w3.org/2001/XMLSchema#nonNegativeInteger">1</owl:maxQualifiedCardinality>
    <rdf:type rdf:resource="http://www.w3.org/2002/07/owl#Restriction"/>
  </rdf:Description>
  <rdf:Description rdf:about="#InformationContent">
    <vs:term_status>stable</vs:term_status>
    <rdfs:subClassOf rdf:resource="http://www.w3.org/2002/07/owl#Thing"/>
    <rdfs:label xml:lang="en">Alphanumerical information content</rdfs:label>
    <rdfs:comment xml:lang="en">Alphanumerical information content is a term for specifying the alphanumerical information according to BS EN 17412-1 (2020)</rdfs:comment>
    <rdf:type rdf:resource="http://www.w3.org/2002/07/owl#Class"/>
  </rdf:Description>
  <rdf:Description rdf:about="#hasLocation">
    <vs:term_status>stable</vs:term_status>
    <rdfs:subPropertyOf rdf:resource="http://www.w3.org/2002/07/owl#topDataProperty"/>
    <rdfs:range rdf:nodeID="A103"/>
    <rdfs:label xml:lang="en">has location</rdfs:label>
    <rdfs:domain rdf:resource="#Location"/>
    <rdf:type rdf:resource="http://www.w3.org/2002/07/owl#DatatypeProperty"/>
  </rdf:Description>
  <rdf:Description rdf:about="#IdentifierType">
    <vs:term_status>stable</vs:term_status>
    <rdfs:subClassOf rdf:resource="http://www.w3.org/2002/07/owl#Thing"/>
    <rdfs:label xml:lang="en">Identifier type</rdfs:label>
    <rdfs:comment xml:lang="en">Identifier type is used to specify the identifier in a breakdown structure according to BS EN 17412-1 (2020)</rdfs:comment>
    <rdf:type rdf:resource="http://www.w3.org/2002/07/owl#Class"/>
  </rdf:Description>
  <rdf:Description rdf:about="#hasDocument">
    <vs:term_status>stable</vs:term_status>
    <rdfs:subPropertyOf rdf:resource="http://www.w3.org/2002/07/owl#topObjectProperty"/>
    <rdfs:range rdf:resource="#RequiredDocument"/>
    <rdfs:label xml:lang="en">has document</rdfs:label>
    <rdfs:domain rdf:resource="#Documentation"/>
    <rdfs:comment xml:lang="en">The object property relates a set of documents with documentation according to ISO 7817-3</rdfs:comment>
    <rdf:type rdf:resource="http://www.w3.org/2002/07/owl#ObjectProperty"/>
  </rdf:Description>
  <rdf:Description rdf:about="https://w3id.org/loin/v2/ids#hasValue">
    <vs:term_status>stable</vs:term_status>
    <rdfs:range rdf:resource="https://w3id.org/loin/v2/ids#Value"/>
    <rdfs:label>has value</rdfs:label>
    <rdfs:domain rdf:resource="https://w3id.org/loin/v2/ids#Property"/>
    <rdfs:domain rdf:resource="https://w3id.org/loin/v2/ids#Material"/>
    <rdfs:domain rdf:resource="https://w3id.org/loin/v2/ids#Attribute"/>
    <rdfs:comment xml:lang="en">relates the value with a facet in IDS data definition</rdfs:comment>
    <rdf:type rdf:resource="http://www.w3.org/2002/07/owl#ObjectProperty"/>
  </rdf:Description>
  <rdf:Description rdf:about="#hasDataTemplate">
    <owl:inverseOf rdf:resource="https://w3id.org/dt#isDataTemplateFor"/>
    <rdfs:subPropertyOf rdf:resource="#hasAlphanumericalInformation"/>
    <rdfs:range rdf:resource="https://w3id.org/dt#DataTemplate"/>
    <rdfs:label>has data template</rdfs:label>
    <rdfs:domain rdf:resource="#AlphanumericalInformation"/>
    <rdf:type rdf:resource="http://www.w3.org/2002/07/owl#ObjectProperty"/>
  </rdf:Description>
  <rdf:Description rdf:nodeID="A137">
    <owl:qualifiedCardinality rdf:datatype="http://www.w3.org/2001/XMLSchema#nonNegativeInteger">1</owl:qualifiedCardinality>
    <owl:onProperty rdf:resource="#hasParametricBehaviour"/>
    <owl:onDataRange rdf:nodeID="A16"/>
    <rdf:type rdf:resource="http://www.w3.org/2002/07/owl#Restriction"/>
  </rdf:Description>
  <rdf:Description rdf:about="#simplified">
    <vs:term_status>stable</vs:term_status>
    <rdfs:label xml:lang="en">simplified</rdfs:label>
    <rdfs:comment xml:lang="en">simplified, an example of detail according to notes of geometrical information specification for information need in BS EN 17412-1 (2020)</rdfs:comment>
    <rdf:type rdf:resource="#Detail"/>
  </rdf:Description>
  <rdf:Description rdf:nodeID="A99">
    <rdf:rest rdf:resource="http://www.w3.org/1999/02/22-rdf-syntax-ns#nil"/>
    <rdf:first>ParametricGeometry</rdf:first>
  </rdf:Description>
  <rdf:Description rdf:about="#belongsToInformationContent">
    <vs:term_status>stable</vs:term_status>
    <rdfs:subPropertyOf rdf:resource="http://www.w3.org/2002/07/owl#topObjectProperty"/>
    <rdfs:range rdf:resource="#InformationContent"/>
    <rdfs:label xml:lang="en">belongs to information content</rdfs:label>
    <rdfs:domain rdf:resource="#RequiredDocument"/>
    <rdfs:comment xml:lang="en">Specification of document, that relates with a respective person</rdfs:comment>
    <rdf:type rdf:resource="http://www.w3.org/2002/07/owl#ObjectProperty"/>
  </rdf:Description>
  <rdf:Description rdf:nodeID="A138">
    <owl:onProperty rdf:resource="https://w3id.org/loin/v2/ids#hasIFCDataType"/>
    <owl:cardinality rdf:datatype="http://www.w3.org/2001/XMLSchema#nonNegativeInteger">1</owl:cardinality>
    <rdf:type rdf:resource="http://www.w3.org/2002/07/owl#Restriction"/>
  </rdf:Description>
  <rdf:Description rdf:nodeID="A63">
    <rdf:rest rdf:nodeID="A139"/>
    <rdf:first>SingleColor</rdf:first>
  </rdf:Description>
  <rdf:Description rdf:nodeID="A69">
    <owl:onProperty rdf:resource="#hasNameInLanguage"/>
    <owl:onDataRange rdf:resource="http://www.w3.org/1999/02/22-rdf-syntax-ns#langString"/>
    <owl:maxQualifiedCardinality rdf:datatype="http://www.w3.org/2001/XMLSchema#nonNegativeInteger">1</owl:maxQualifiedCardinality>
    <rdf:type rdf:resource="http://www.w3.org/2002/07/owl#Restriction"/>
  </rdf:Description>
  <rdf:Description rdf:about="#requested">
    <vs:term_status>stable</vs:term_status>
    <rdfs:subPropertyOf rdf:resource="http://www.w3.org/2002/07/owl#topDataProperty"/>
    <rdfs:range rdf:resource="http://www.w3.org/2001/XMLSchema#boolean"/>
    <rdfs:label>requested</rdfs:label>
    <rdfs:label xml:lang="en">requested as boolean, specifys if Geometrical information is needed according to BS EN 17412-1 (2020)</rdfs:label>
    <rdfs:domain rdf:resource="#GeometrySpecification"/>
    <rdfs:domain rdf:resource="#GeometricalInformation"/>
    <rdfs:domain rdf:resource="#AlphanumericalInformation"/>
    <rdf:type rdf:resource="http://www.w3.org/2002/07/owl#DatatypeProperty"/>
  </rdf:Description>
  <rdf:Description rdf:about="#Identifier">
    <vs:term_status>stable</vs:term_status>
    <rdfs:subClassOf rdf:nodeID="A31"/>
    <rdfs:subClassOf rdf:nodeID="A44"/>
    <rdfs:subClassOf rdf:nodeID="A123"/>
    <rdfs:subClassOf rdf:resource="http://www.w3.org/2002/07/owl#Thing"/>
    <rdfs:label xml:lang="en">Identifier</rdfs:label>
    <rdfs:comment xml:lang="en">Identifier is used to assiging a vaule for positioning the object in a breakdown structure according to BS EN 17412-1 (2020)</rdfs:comment>
    <rdf:type rdf:resource="http://www.w3.org/2002/07/owl#Class"/>
  </rdf:Description>
  <rdf:Description rdf:about="#Detail">
    <vs:term_status>stable</vs:term_status>
    <rdfs:subClassOf rdf:nodeID="A54"/>
    <rdfs:subClassOf rdf:resource="#GeometrySpecification"/>
    <rdfs:label xml:lang="en">Detail</rdfs:label>
    <rdfs:comment xml:lang="en">Detail as a geometrical information specification for information need according to ISO 7817-3</rdfs:comment>
    <rdf:type rdf:resource="http://www.w3.org/2002/07/owl#Class"/>
  </rdf:Description>
  <rdf:Description rdf:nodeID="A110">
    <owl:onProperty rdf:resource="#hasProperty"/>
    <owl:minCardinality rdf:datatype="http://www.w3.org/2001/XMLSchema#nonNegativeInteger">0</owl:minCardinality>
    <rdf:type rdf:resource="http://www.w3.org/2002/07/owl#Restriction"/>
  </rdf:Description>
  <rdf:Description rdf:about="https://w3id.org/loin/v2/ids#hasAttributeName">
    <vs:term_status>stable</vs:term_status>
    <rdfs:range rdf:resource="https://w3id.org/loin/v2/ids#AttributeName"/>
    <rdfs:label xml:lang="en">has attribute name</rdfs:label>
    <rdfs:domain rdf:resource="https://w3id.org/loin/v2/ids#Attribute"/>
    <rdfs:comment xml:lang="en">The object property relates the attribute name with the facet attribute according to IDS definition</rdfs:comment>
    <rdf:type rdf:resource="http://www.w3.org/2002/07/owl#ObjectProperty"/>
  </rdf:Description>
  <rdf:Description rdf:about="#DocumentContent">
    <vs:term_status>stable</vs:term_status>
    <rdfs:subClassOf rdf:resource="#DocumentSpecification"/>
    <rdfs:label xml:lang="en">Document content</rdfs:label>
    <rdfs:comment xml:lang="en">Document specification for content for information need according to ISO 7817-3</rdfs:comment>
    <rdf:type rdf:resource="http://www.w3.org/2002/07/owl#Class"/>
  </rdf:Description>
  <rdf:Description rdf:about="#hasQuantityKind">
    <rdfs:subPropertyOf rdf:resource="http://www.w3.org/2002/07/owl#topObjectProperty"/>
    <rdfs:range rdf:resource="https://w3id.org/tempo#QuantityKind"/>
    <rdfs:label xml:lang="en">The object property relates the alphanumerical information with the quantitiy kind according to ISO 7817-3</rdfs:label>
    <rdfs:domain rdf:resource="#AlphanumericalInformation"/>
    <rdf:type rdf:resource="http://www.w3.org/2002/07/owl#ObjectProperty"/>
  </rdf:Description>
  <rdf:Description rdf:about="#hasPurpose">
    <vs:term_status>stable</vs:term_status>
    <rdfs:subPropertyOf rdf:resource="http://www.w3.org/2002/07/owl#topObjectProperty"/>
    <rdfs:range rdf:resource="#Purpose"/>
    <rdfs:label xml:lang="en">has purpose</rdfs:label>
    <rdfs:domain rdf:resource="#Prerequisites"/>
    <rdfs:comment xml:lang="en">The object property relates the purpose with the prerequisites according to ISO 7817-3</rdfs:comment>
    <rdf:type rdf:resource="http://www.w3.org/2002/07/owl#ObjectProperty"/>
  </rdf:Description>
  <rdf:Description rdf:nodeID="A24">
    <owl:onProperty rdf:resource="https://w3id.org/tempo#conceptGUID"/>
    <owl:onDataRange rdf:resource="https://w3id.org/tempo#GUIDType"/>
    <owl:minQualifiedCardinality rdf:datatype="http://www.w3.org/2001/XMLSchema#nonNegativeInteger">0</owl:minQualifiedCardinality>
    <rdf:type rdf:resource="http://www.w3.org/2002/07/owl#Restriction"/>
  </rdf:Description>
  <rdf:Description rdf:nodeID="A46">
    <owl:qualifiedCardinality rdf:datatype="http://www.w3.org/2001/XMLSchema#nonNegativeInteger">1</owl:qualifiedCardinality>
    <owl:onProperty rdf:resource="#hasLocation"/>
    <owl:onDataRange rdf:nodeID="A140"/>
    <rdf:type rdf:resource="http://www.w3.org/2002/07/owl#Restriction"/>
  </rdf:Description>
  <rdf:Description rdf:about="#hasReferenceSource">
    <rdfs:subPropertyOf rdf:resource="http://www.w3.org/2002/07/owl#topObjectProperty"/>
    <rdfs:range rdf:resource="http://www.w3.org/2002/07/owl#Thing"/>
    <rdfs:range rdf:resource="http://www.w3.org/2001/XMLSchema#anyURI"/>
    <rdfs:label xml:lang="en">has reference source</rdfs:label>
    <rdfs:domain rdf:nodeID="A64"/>
    <rdf:type rdf:resource="http://www.w3.org/2002/07/owl#ObjectProperty"/>
  </rdf:Description>
  <rdf:Description rdf:about="#three-dimensional">
    <vs:term_status>stable</vs:term_status>
    <rdfs:label xml:lang="en">three-dimensional</rdfs:label>
    <rdfs:comment xml:lang="en">Three-dimensional, an example of dimensionality from a geometrical information specification for information need according to BS EN 17412-1 (2020)</rdfs:comment>
    <rdf:type rdf:resource="#Dimensionality"/>
  </rdf:Description>
  <rdf:Description rdf:about="https://w3id.org/loin/v2/ids#Material">
    <vs:term_status>stable</vs:term_status>
    <rdfs:subClassOf rdf:resource="https://w3id.org/loin/v2/ids#FacetDefinition"/>
    <rdfs:label xml:lang="en">Material</rdfs:label>
    <rdfs:comment xml:lang="en">Material is a facet of Information Delivery Specification(IDS), a standard developed by buildingSMART International</rdfs:comment>
    <rdf:type rdf:resource="http://www.w3.org/2002/07/owl#Class"/>
  </rdf:Description>
  <rdf:Description rdf:nodeID="A74">
    <owl:onProperty rdf:resource="https://w3id.org/loin/v2/ids#restrictionFormulation"/>
    <owl:cardinality rdf:datatype="http://www.w3.org/2001/XMLSchema#nonNegativeInteger">1</owl:cardinality>
    <rdf:type rdf:resource="http://www.w3.org/2002/07/owl#Restriction"/>
  </rdf:Description>
  <rdf:Description rdf:nodeID="A128">
    <rdf:rest rdf:nodeID="A45"/>
    <rdf:first>Optional</rdf:first>
  </rdf:Description>
  <rdf:Description rdf:nodeID="A30">
    <owl:oneOf rdf:nodeID="A97"/>
    <rdf:type rdf:resource="http://www.w3.org/2000/01/rdf-schema#Datatype"/>
  </rdf:Description>
  <rdf:Description rdf:about="#purpose">
    <rdfs:subPropertyOf rdf:resource="http://www.w3.org/2002/07/owl#topDataProperty"/>
    <rdfs:range rdf:resource="http://www.w3.org/2001/XMLSchema#string"/>
    <rdfs:label xml:lang="en">purpose</rdfs:label>
    <rdf:type rdf:resource="http://www.w3.org/2002/07/owl#DatatypeProperty"/>
  </rdf:Description>
  <rdf:Description rdf:nodeID="A135">
    <owl:someValuesFrom rdf:resource="#DocumentPurpose"/>
    <owl:onProperty rdf:resource="#hasDocumentSpecification"/>
    <rdf:type rdf:resource="http://www.w3.org/2002/07/owl#Restriction"/>
  </rdf:Description>
  <rdf:Description rdf:nodeID="A41">
    <schema:identifier rdf:resource="https://www.inf.bi.rub.de"/>
    <rdf:type rdf:resource="https://schema.org/Organization"/>
    <schema:name>Chair of Computing in Engineering, Ruhr University Bochum</schema:name>
    <schema:parentOrganization rdf:nodeID="A40"/>
  </rdf:Description>
  <rdf:Description rdf:about="https://w3id.org/loin/v2/ids#PredefinedType">
    <vs:term_status>stable</vs:term_status>
    <rdfs:subClassOf rdf:nodeID="A73"/>
    <rdfs:subClassOf rdf:nodeID="A79"/>
    <rdfs:subClassOf rdf:resource="https://w3id.org/loin/v2/ids#FacetParameter"/>
    <rdfs:label xml:lang="en">Predefined type</rdfs:label>
    <rdfs:comment xml:lang="en">Predefined type must be a valid predefined type from the IFC schema, or any custom text value according to IDS standard developed by buildingSMART International</rdfs:comment>
    <rdf:type rdf:resource="http://www.w3.org/2002/07/owl#Class"/>
  </rdf:Description>
  <rdf:Description rdf:nodeID="A141">
    <owl:someValuesFrom rdf:resource="https://w3id.org/loin/v2/ids#Entity"/>
    <owl:onProperty rdf:resource="https://w3id.org/loin/v2/ids#hasApplicability"/>
    <rdf:type rdf:resource="http://www.w3.org/2002/07/owl#Restriction"/>
  </rdf:Description>
  <rdf:Description rdf:nodeID="A65">
    <rdf:rest rdf:nodeID="A115"/>
    <rdf:first rdf:resource="#BreakdownStructure"/>
  </rdf:Description>
  <rdf:Description rdf:about="#hasBreakdownStructureType">
    <vs:term_status>stable</vs:term_status>
    <rdfs:subPropertyOf rdf:resource="http://www.w3.org/2002/07/owl#topObjectProperty"/>
    <rdfs:range rdf:resource="#BreakdownStructureType"/>
    <rdfs:label xml:lang="en">has breakdown structure type</rdfs:label>
    <rdfs:domain rdf:resource="#BreakdownStructure"/>
    <rdfs:comment xml:lang="en">The object property relates a specific type with the breakdown structure according to BS EN 17412-1 (2020)</rdfs:comment>
    <rdf:type rdf:resource="http://www.w3.org/2002/07/owl#ObjectProperty"/>
  </rdf:Description>
  <rdf:Description rdf:about="https://w3id.org/loin/v2/icdd#isRelatedToContainerParty">
    <vs:term_status>stable</vs:term_status>
    <rdfs:range rdf:resource="https://standards.iso.org/iso/21597/-1/ed-1/en/Container#Party"/>
    <rdfs:label xml:lang="en">is related to container party</rdfs:label>
    <rdfs:domain rdf:resource="#Actor"/>
    <rdfs:comment xml:lang="en">The object property is an extension with ICDD. It relates the actors defined by BS EN 17412-1(2020) with container party</rdfs:comment>
    <rdf:type rdf:resource="http://www.w3.org/2002/07/owl#ObjectProperty"/>
  </rdf:Description>
  <rdf:Description rdf:nodeID="A29">
    <rdf:rest rdf:resource="http://www.w3.org/1999/02/22-rdf-syntax-ns#nil"/>
    <rdf:first>Textures</rdf:first>
  </rdf:Description>
  <rdf:Description rdf:about="https://w3id.org/loin/v2/ids#RestrictionType">
    <vs:term_status>stable</vs:term_status>
    <rdfs:subClassOf rdf:resource="http://www.w3.org/2000/01/rdf-schema#Resource"/>
    <rdfs:label xml:lang="en">Restriction type</rdfs:label>
    <rdfs:comment xml:lang="en">Restriction type is used to specify the value of IDS facet parameter, that is defined in restriction formulation. The restriction types are based on IDS standard developed by buildingSMART International</rdfs:comment>
    <rdf:type rdf:resource="http://www.w3.org/2002/07/owl#Class"/>
  </rdf:Description>
  <rdf:Description rdf:nodeID="A92">
    <rdf:rest rdf:nodeID="A34"/>
    <rdf:first>D0</rdf:first>
  </rdf:Description>
  <rdf:Description rdf:about="https://w3id.org/loin/v2/ids#belongsToPset">
    <vs:term_status>stable</vs:term_status>
    <rdfs:range rdf:resource="https://w3id.org/loin/v2/ids#PsetName"/>
    <rdfs:label xml:lang="en">A property belongs to Property set</rdfs:label>
    <rdfs:domain rdf:resource="https://w3id.org/loin/v2/ids#Property"/>
    <rdfs:comment xml:lang="en">Specification is used for facet property of IDS data definition.</rdfs:comment>
    <rdf:type rdf:resource="http://www.w3.org/2002/07/owl#ObjectProperty"/>
  </rdf:Description>
  <rdf:Description rdf:nodeID="A55">
    <owl:oneOf rdf:nodeID="A121"/>
    <rdf:type rdf:resource="http://www.w3.org/2000/01/rdf-schema#Datatype"/>
  </rdf:Description>
  <rdf:Description rdf:about="#Provided_As_Information">
    <vs:term_status>stable</vs:term_status>
    <rdfs:label xml:lang="en">The document provided as information</rdfs:label>
    <rdfs:comment xml:lang="en">The document delivered by Inquirer as percondition or information</rdfs:comment>
    <rdf:type rdf:resource="#DocumentPurpose"/>
  </rdf:Description>
  <rdf:Description rdf:about="#Prerequisites">
    <rdfs:subClassOf rdf:nodeID="A127"/>
    <rdf:type rdf:resource="http://www.w3.org/2002/07/owl#Class"/>
    <rdfs:subClassOf rdf:nodeID="A90"/>
    <rdfs:comment xml:lang="en">Prerequisites is a term for specifying the prerequisites of a corresponding specification according to ISO 7817-3</rdfs:comment>
    <rdfs:label xml:lang="en">Prerequisites</rdfs:label>
    <rdfs:subClassOf rdf:nodeID="A114"/>
    <rdfs:subClassOf rdf:nodeID="A142"/>
    <rdfs:subClassOf rdf:nodeID="A33"/>
    <rdfs:subClassOf rdf:nodeID="A130"/>
    <rdfs:subClassOf rdf:nodeID="A84"/>
    <rdfs:subClassOf rdf:nodeID="A143"/>
    <rdfs:subClassOf rdf:nodeID="A21"/>
    <rdfs:subClassOf rdf:resource="http://www.w3.org/2002/07/owl#Thing"/>
    <rdfs:subClassOf rdf:nodeID="A60"/>
  </rdf:Description>
  <rdf:Description rdf:nodeID="A98">
    <rdf:rest rdf:nodeID="A144"/>
    <rdf:first>NoColor</rdf:first>
  </rdf:Description>
  <rdf:Description rdf:about="https://w3id.org/loin/v2/ids#hasEntityName">
    <vs:term_status>stable</vs:term_status>
    <rdfs:range rdf:resource="https://w3id.org/loin/v2/ids#EntityName"/>
    <rdfs:label xml:lang="en">has entity name</rdfs:label>
    <rdfs:domain rdf:resource="https://w3id.org/loin/v2/ids#Entity"/>
    <rdfs:comment xml:lang="en">The object property relates the entity name with the facet entity according to IDS definition</rdfs:comment>
    <rdf:type rdf:resource="http://www.w3.org/2002/07/owl#ObjectProperty"/>
  </rdf:Description>
  <rdf:Description rdf:nodeID="A71">
    <owl:onProperty rdf:resource="#hasPrerequisites"/>
    <owl:onClass rdf:resource="#Prerequisites"/>
    <owl:minQualifiedCardinality rdf:datatype="http://www.w3.org/2001/XMLSchema#nonNegativeInteger">0</owl:minQualifiedCardinality>
    <rdf:type rdf:resource="http://www.w3.org/2002/07/owl#Restriction"/>
  </rdf:Description>
  <rdf:Description rdf:nodeID="A136">
    <owl:onProperty rdf:resource="https://w3id.org/tempo#conceptGUID"/>
    <owl:onDataRange rdf:resource="https://w3id.org/tempo#GUIDType"/>
    <owl:minQualifiedCardinality rdf:datatype="http://www.w3.org/2001/XMLSchema#nonNegativeInteger">0</owl:minQualifiedCardinality>
    <rdf:type rdf:resource="http://www.w3.org/2002/07/owl#Restriction"/>
  </rdf:Description>
  <rdf:Description rdf:about="#hasDetail">
    <vs:term_status>stable</vs:term_status>
    <rdfs:subPropertyOf rdf:resource="http://www.w3.org/2002/07/owl#topDataProperty"/>
    <rdfs:range rdf:nodeID="A49"/>
    <rdfs:label xml:lang="en">has detail</rdfs:label>
    <rdfs:domain rdf:resource="#Detail"/>
    <rdf:type rdf:resource="http://www.w3.org/2002/07/owl#DatatypeProperty"/>
  </rdf:Description>
  <rdf:Description rdf:nodeID="A120">
    <schema:identifier rdf:resource="https://www.inf.bi.ruhr-uni-bochum.de/iib/lehrstuhl/mitarbeiter/sven_zentgraf.html.en"/>
    <schema:name>Ruhr University Bochum</schema:name>
  </rdf:Description>
  <rdf:Description rdf:nodeID="A144">
    <rdf:rest rdf:nodeID="A28"/>
    <rdf:first>SingleColor</rdf:first>
  </rdf:Description>
  <rdf:Description rdf:nodeID="A67">
    <owl:onProperty rdf:resource="#hasSpecificationPerObjectType"/>
    <owl:onClass rdf:resource="#SpecificationPerObjectType"/>
    <owl:minQualifiedCardinality rdf:datatype="http://www.w3.org/2001/XMLSchema#nonNegativeInteger">0</owl:minQualifiedCardinality>
    <rdf:type rdf:resource="http://www.w3.org/2002/07/owl#Restriction"/>
  </rdf:Description>
  <rdf:Description rdf:nodeID="A119">
    <rdf:rest rdf:nodeID="A145"/>
    <rdf:first>NotRequested</rdf:first>
  </rdf:Description>
  <rdf:Description rdf:about="https://w3id.org/loin/v2/ids#hasPropertyName">
    <vs:term_status>stable</vs:term_status>
    <rdfs:range rdf:resource="https://w3id.org/loin/v2/ids#PropertyName"/>
    <rdfs:label xml:lang="en">has property name</rdfs:label>
    <rdfs:domain rdf:resource="https://w3id.org/loin/v2/ids#Property"/>
    <rdfs:comment xml:lang="en">The object property relates a property name type with the facet property according to IDS definition</rdfs:comment>
    <rdf:type rdf:resource="http://www.w3.org/2002/07/owl#ObjectProperty"/>
  </rdf:Description>
  <rdf:Description rdf:about="#ReferenceOfStructure">
    <vs:term_status>stable</vs:term_status>
    <rdfs:label xml:lang="en">Reference of an item in a breakdown structure</rdfs:label>
    <rdfs:comment xml:lang="en">Reference, an identifier type in a breakdown structure according to notes of BS EN 17412-1 (2020)</rdfs:comment>
    <rdf:type rdf:resource="#IdentifierType"/>
  </rdf:Description>
  <rdf:Description rdf:about="#Required_with_Supplement">
    <vs:term_status>stable</vs:term_status>
    <rdfs:label xml:lang="en">document required with supplement</rdfs:label>
    <rdfs:comment xml:lang="en">The document required by deliverer with supplement of information</rdfs:comment>
    <rdf:type rdf:resource="#DocumentPurpose"/>
  </rdf:Description>
  <rdf:Description rdf:about="#ReceivingActor">
    <vs:term_status>stable</vs:term_status>
    <rdfs:subClassOf rdf:resource="#Actor"/>
    <rdfs:label xml:lang="en">Receiving actor</rdfs:label>
    <rdfs:comment xml:lang="en">Receiving actor is a party for information delivery according to ISO 19650-1 (2018)</rdfs:comment>
    <rdf:type rdf:resource="http://www.w3.org/2002/07/owl#Class"/>
  </rdf:Description>
  <rdf:Description rdf:about="#Semantic">
    <vs:term_status>stable</vs:term_status>
    <rdfs:label xml:lang="en">Semantic structure</rdfs:label>
    <rdfs:comment xml:lang="en">An example of breakdown structure type according to BS EN 17412-1 (2020)</rdfs:comment>
    <rdf:type rdf:resource="#BreakdownStructureType"/>
  </rdf:Description>
  <rdf:Description rdf:about="#hasAlphanumericalInformation">
    <vs:term_status>stable</vs:term_status>
    <rdfs:subPropertyOf rdf:resource="#hasInformation"/>
    <rdfs:range rdf:resource="#AlphanumericalInformation"/>
    <rdfs:label xml:lang="en">has alphanumerical information</rdfs:label>
    <rdfs:domain rdf:resource="#SpecificationPerObjectType"/>
    <rdfs:comment xml:lang="en">The object property relates an alphanumerical information with a LOIN object according to ISO 7817-3</rdfs:comment>
    <rdf:type rdf:resource="http://www.w3.org/2002/07/owl#ObjectProperty"/>
  </rdf:Description>
  <rdf:Description rdf:about="https://w3id.org/loin/v2/ids#Value">
    <vs:term_status>stable</vs:term_status>
    <rdfs:subClassOf rdf:nodeID="A113"/>
    <rdfs:subClassOf rdf:nodeID="A146"/>
    <rdfs:subClassOf rdf:resource="https://w3id.org/loin/v2/ids#FacetParameter"/>
    <rdfs:label>Value</rdfs:label>
    <rdfs:comment>Value can be any custom value according to IDS standard developed by buildingSMART International</rdfs:comment>
    <rdf:type rdf:resource="http://www.w3.org/2002/07/owl#Class"/>
  </rdf:Description>
  <rdf:Description rdf:nodeID="A10">
    <owl:onProperty rdf:resource="https://w3id.org/loin/v2/ids#hasRestrictionType"/>
    <owl:hasValue rdf:resource="#SimpleValue"/>
    <rdf:type rdf:resource="http://www.w3.org/2002/07/owl#Restriction"/>
  </rdf:Description>
  <rdf:Description rdf:nodeID="A139">
    <rdf:rest rdf:nodeID="A80"/>
    <rdf:first>MaterialColor</rdf:first>
  </rdf:Description>
  <rdf:Description rdf:about="#structuralAnalysis">
    <vs:term_status>stable</vs:term_status>
    <rdfs:label xml:lang="en">Structural analysis</rdfs:label>
    <rdfs:comment xml:lang="en">Structural analysis, an example of IDM purpose from BS EN 17412-1 (2020) - Annex B</rdfs:comment>
    <rdf:type rdf:resource="#Purpose"/>
  </rdf:Description>
  <rdf:Description rdf:nodeID="A38">
    <rdf:rest rdf:resource="http://www.w3.org/1999/02/22-rdf-syntax-ns#nil"/>
    <rdf:first>L5</rdf:first>
  </rdf:Description>
  <rdf:Description rdf:about="#relative">
    <vs:term_status>stable</vs:term_status>
    <rdfs:label xml:lang="en">relative location</rdfs:label>
    <rdfs:comment xml:lang="en">Relative, an example of location according to notes of geometrical information specification for information need in BS EN 17412-1 (2020)</rdfs:comment>
    <rdf:type rdf:resource="#Location"/>
  </rdf:Description>
  <rdf:Description rdf:nodeID="A68">
    <owl:onProperty rdf:resource="#hasNameInLanguage"/>
    <owl:onDataRange rdf:resource="http://www.w3.org/1999/02/22-rdf-syntax-ns#langString"/>
    <owl:minQualifiedCardinality rdf:datatype="http://www.w3.org/2001/XMLSchema#nonNegativeInteger">1</owl:minQualifiedCardinality>
    <rdf:type rdf:resource="http://www.w3.org/2002/07/owl#Restriction"/>
  </rdf:Description>
  <rdf:Description rdf:nodeID="A117">
    <owl:onProperty rdf:resource="https://w3id.org/loin/v2/ids#hasEntityName"/>
    <owl:cardinality rdf:datatype="http://www.w3.org/2001/XMLSchema#nonNegativeInteger">1</owl:cardinality>
    <rdf:type rdf:resource="http://www.w3.org/2002/07/owl#Restriction"/>
  </rdf:Description>
  <rdf:Description rdf:about="#hasDimensionality">
    <vs:term_status>stable</vs:term_status>
    <rdfs:subPropertyOf rdf:resource="http://www.w3.org/2002/07/owl#topDataProperty"/>
    <rdfs:range rdf:nodeID="A91"/>
    <rdfs:label xml:lang="en">has detail</rdfs:label>
    <rdfs:domain rdf:resource="#Dimensionality"/>
    <rdf:type rdf:resource="http://www.w3.org/2002/07/owl#DatatypeProperty"/>
  </rdf:Description>
  <rdf:Description rdf:about="#isRelatedToLoinDocument">
    <vs:term_status>stable</vs:term_status>
    <rdfs:subPropertyOf rdf:resource="http://www.w3.org/2002/07/owl#topObjectProperty"/>
    <rdfs:range rdf:resource="#RequiredDocument"/>
    <rdfs:label>is related to Loin document</rdfs:label>
    <rdfs:domain rdf:resource="#InformationContent"/>
    <rdfs:comment xml:lang="en">The object property relates the alphanumerical information content with document according to BS EN 17412-1(2020)</rdfs:comment>
    <rdf:type rdf:resource="http://www.w3.org/2002/07/owl#ObjectProperty"/>
  </rdf:Description>
  <rdf:Description rdf:nodeID="A134">
    <owl:onProperty rdf:resource="https://w3id.org/tempo#conceptGUID"/>
    <owl:onDataRange rdf:resource="https://w3id.org/tempo#GUIDType"/>
    <owl:maxQualifiedCardinality rdf:datatype="http://www.w3.org/2001/XMLSchema#nonNegativeInteger">1</owl:maxQualifiedCardinality>
    <rdf:type rdf:resource="http://www.w3.org/2002/07/owl#Restriction"/>
  </rdf:Description>
  <rdf:Description rdf:nodeID="A76">
    <owl:onProperty rdf:resource="https://w3id.org/loin/v2/ids#hasRestrictionType"/>
    <owl:cardinality rdf:datatype="http://www.w3.org/2001/XMLSchema#nonNegativeInteger">1</owl:cardinality>
    <rdf:type rdf:resource="http://www.w3.org/2002/07/owl#Restriction"/>
  </rdf:Description>
  <rdf:Description rdf:about="#OntologyDataDefinition">
    <vs:term_status>stable</vs:term_status>
    <rdfs:subClassOf rdf:nodeID="A88"/>
    <rdfs:subClassOf rdf:resource="#InformationContent"/>
    <rdfs:label xml:lang="en">Ontology data definition</rdfs:label>
    <rdfs:comment xml:lang="en">Ontology data definition is an extension of BS EN 17412-1 (2020). It is used to specify the alphanumerical information according to a published or customized ontology</rdfs:comment>
    <rdf:type rdf:resource="http://www.w3.org/2002/07/owl#Class"/>
  </rdf:Description>
  <rdf:Description rdf:about="#two-dimensional">
    <vs:term_status>stable</vs:term_status>
    <rdfs:label xml:lang="en">two-dimensional</rdfs:label>
    <rdfs:comment xml:lang="en">Two-dimensional, an example of dimensionality from a geometrical information specification for information need according to BS EN 17412-1 (2020)</rdfs:comment>
    <rdf:type rdf:resource="#Dimensionality"/>
  </rdf:Description>
  <rdf:Description rdf:nodeID="A140">
    <owl:oneOf rdf:nodeID="A77"/>
    <rdf:type rdf:resource="http://www.w3.org/2000/01/rdf-schema#Datatype"/>
  </rdf:Description>
  <rdf:Description rdf:nodeID="A147">
    <owl:onProperty rdf:resource="#hasAlphanumericalInformation"/>
    <owl:onClass rdf:resource="#AlphanumericalInformation"/>
    <owl:minQualifiedCardinality rdf:datatype="http://www.w3.org/2001/XMLSchema#nonNegativeInteger">0</owl:minQualifiedCardinality>
    <rdf:type rdf:resource="http://www.w3.org/2002/07/owl#Restriction"/>
  </rdf:Description>
  <rdf:Description rdf:about="#zero-dimensional">
    <vs:term_status>stable</vs:term_status>
    <rdfs:label xml:lang="en">zero-dimensional</rdfs:label>
    <rdfs:comment xml:lang="en">zero-dimensional, an example of dimensionality from a geometrical information specification for information need according to BS EN 17412-1 (2020)</rdfs:comment>
    <rdf:type rdf:resource="#Dimensionality"/>
  </rdf:Description>
  <rdf:Description rdf:nodeID="A133">
    <owl:someValuesFrom rdf:resource="#Location"/>
    <owl:onProperty rdf:resource="#hasGeometrySpecification"/>
    <rdf:type rdf:resource="http://www.w3.org/2002/07/owl#Restriction"/>
  </rdf:Description>
  <rdf:Description rdf:about="#hasPrerequisites">
    <rdfs:subPropertyOf rdf:resource="http://www.w3.org/2002/07/owl#topObjectProperty"/>
    <rdfs:range rdf:resource="#Prerequisites"/>
    <rdfs:label xml:lang="en">has Prerequisites</rdfs:label>
    <rdfs:domain rdf:resource="#Specification"/>
    <rdfs:comment xml:lang="en">The object property relates the specification with the prerequisites</rdfs:comment>
    <rdf:type rdf:resource="http://www.w3.org/2002/07/owl#ObjectProperty"/>
  </rdf:Description>
  <rdf:Description rdf:about="#Used_As_Template">
    <vs:term_status>stable</vs:term_status>
    <rdfs:label xml:lang="en">The document as template</rdfs:label>
    <rdfs:comment xml:lang="en">The document required by deliverer should be used as template</rdfs:comment>
    <rdf:type rdf:resource="#DocumentPurpose"/>
  </rdf:Description>
  <rdf:Description rdf:about="#ParametricBehaviour">
    <vs:term_status>stable</vs:term_status>
    <rdfs:subClassOf rdf:nodeID="A137"/>
    <rdfs:subClassOf rdf:resource="#GeometrySpecification"/>
    <rdfs:label xml:lang="en">Parametric behaviour</rdfs:label>
    <rdfs:comment xml:lang="en">Parametric behaviour as a geometrical information specification for information need according to ISO 7817-3</rdfs:comment>
    <rdf:type rdf:resource="http://www.w3.org/2002/07/owl#Class"/>
  </rdf:Description>
  <rdf:Description rdf:nodeID="A148">
    <owl:onProperty rdf:resource="#hasGeometricalInformation"/>
    <owl:cardinality rdf:datatype="http://www.w3.org/2001/XMLSchema#nonNegativeInteger">1</owl:cardinality>
    <rdf:type rdf:resource="http://www.w3.org/2002/07/owl#Restriction"/>
  </rdf:Description>
  <rdf:Description rdf:about="https://w3id.org/loin/v2/ids#Property">
    <vs:term_status>stable</vs:term_status>
    <rdfs:subClassOf rdf:nodeID="A122"/>
    <rdfs:subClassOf rdf:nodeID="A138"/>
    <rdfs:subClassOf rdf:nodeID="A32"/>
    <rdfs:subClassOf rdf:resource="https://w3id.org/loin/v2/ids#FacetDefinition"/>
    <rdfs:label xml:lang="en">Property</rdfs:label>
    <rdfs:comment xml:lang="en">Property is a facet of Information Delivery Specification(IDS), a standard developed by buildingSMART International</rdfs:comment>
    <rdf:type rdf:resource="http://www.w3.org/2002/07/owl#Class"/>
  </rdf:Description>
  <rdf:Description rdf:about="#Index">
    <vs:term_status>stable</vs:term_status>
    <rdfs:label xml:lang="en">Index of an item in a breakdown structure</rdfs:label>
    <rdfs:comment xml:lang="en">Index, an identifier type according to notes of BS EN 17412-1 (2020)</rdfs:comment>
    <rdf:type rdf:resource="#IdentifierType"/>
  </rdf:Description>
  <rdf:Description rdf:about="#DocumentPurpose">
    <vs:term_status>stable</vs:term_status>
    <rdfs:subClassOf rdf:resource="#DocumentSpecification"/>
    <rdfs:label xml:lang="en">Document purpose</rdfs:label>
    <rdfs:comment xml:lang="en">Document purpose is a extension according to ISO 7817-3. It specifies the use of document</rdfs:comment>
    <rdf:type rdf:resource="http://www.w3.org/2002/07/owl#Class"/>
  </rdf:Description>
  <rdf:Description rdf:nodeID="A146">
    <owl:onProperty rdf:resource="https://w3id.org/loin/v2/ids#hasRestrictionType"/>
    <owl:cardinality rdf:datatype="http://www.w3.org/2001/XMLSchema#nonNegativeInteger">1</owl:cardinality>
    <rdf:type rdf:resource="http://www.w3.org/2002/07/owl#Restriction"/>
  </rdf:Description>
  <rdf:Description rdf:about="#NotRequested">
    <loin:requested rdf:datatype="http://www.w3.org/2001/XMLSchema#boolean">false</loin:requested>
    <vs:term_status>stable</vs:term_status>
    <rdfs:label xml:lang="en">Geometry not requested</rdfs:label>
    <rdfs:comment xml:lang="en">Geometry information is not requested</rdfs:comment>
    <rdf:type rdf:resource="#GeometricalInformation"/>
  </rdf:Description>
  <rdf:Description rdf:nodeID="A89">
    <rdf:rest rdf:nodeID="A118"/>
    <rdf:first>L4</rdf:first>
  </rdf:Description>
  <rdf:Description rdf:nodeID="A11">
    <rdf:rest rdf:resource="http://www.w3.org/1999/02/22-rdf-syntax-ns#nil"/>
    <rdf:first>D3</rdf:first>
  </rdf:Description>
  <rdf:Description rdf:about="#SpecificationPerObjectType">
    <rdfs:subClassOf rdf:nodeID="A149"/>
    <rdfs:subClassOf rdf:resource="https://w3id.org/tempo#ConceptType"/>
    <rdfs:subClassOf rdf:nodeID="A111"/>
    <rdfs:label xml:lang="en">Specification per Object Type</rdfs:label>
    <vs:term_status>stable</vs:term_status>
    <rdfs:subClassOf rdf:nodeID="A148"/>
    <rdfs:comment xml:lang="en">SpecificationPerObjectType is a contextual aspect according to  ISO 7817-3</rdfs:comment>
    <rdf:type rdf:resource="http://www.w3.org/2002/07/owl#Class"/>
    <rdfs:subClassOf rdf:resource="http://www.w3.org/2002/07/owl#Thing"/>
    <rdfs:subClassOf rdf:nodeID="A147"/>
  </rdf:Description>
  <rdf:Description rdf:about="#fireSmokeSimulation">
    <vs:term_status>stable</vs:term_status>
    <rdfs:label xml:lang="en">Fire and smoke simulation</rdfs:label>
    <rdfs:comment xml:lang="en">Fire and smoke simulation, an example of IDM purpose from BS EN 17412-1 (2020) - Annex B</rdfs:comment>
    <rdf:type rdf:resource="#Purpose"/>
  </rdf:Description>
  <rdf:Description rdf:nodeID="A95">
    <rdf:rest rdf:resource="http://www.w3.org/1999/02/22-rdf-syntax-ns#nil"/>
    <rdf:first>Relative</rdf:first>
  </rdf:Description>
  <rdf:Description rdf:nodeID="A142">
    <owl:onProperty rdf:resource="#informationDeliveryMilestone"/>
    <owl:onDataRange rdf:resource="http://www.w3.org/2001/XMLSchema#string"/>
    <owl:minQualifiedCardinality rdf:datatype="http://www.w3.org/2001/XMLSchema#nonNegativeInteger">0</owl:minQualifiedCardinality>
    <rdf:type rdf:resource="http://www.w3.org/2002/07/owl#Restriction"/>
  </rdf:Description>
  <rdf:Description rdf:nodeID="A57">
    <rdf:rest rdf:nodeID="A3"/>
    <rdf:first>D0</rdf:first>
  </rdf:Description>
  <rdf:Description rdf:nodeID="A145">
    <rdf:rest rdf:nodeID="A52"/>
    <rdf:first>ExplicitGeometry</rdf:first>
  </rdf:Description>
  <rdf:Description rdf:about="https://w3id.org/loin/v2/ids#DataDefinition">
    <vs:term_status>stable</vs:term_status>
    <rdfs:subClassOf rdf:nodeID="A141"/>
    <rdfs:subClassOf rdf:nodeID="A15"/>
    <rdfs:subClassOf rdf:nodeID="A100"/>
    <rdfs:subClassOf rdf:nodeID="A102"/>
    <rdfs:subClassOf rdf:resource="#InformationContent"/>
    <rdfs:label xml:lang="en">IDS data definition</rdfs:label>
    <rdfs:comment xml:lang="en">IDS data definition is used to specify the alphanumerical information according to Information Delivery Specification (IDS) developed by buildingSMART International</rdfs:comment>
    <rdf:type rdf:resource="http://www.w3.org/2002/07/owl#Class"/>
  </rdf:Description>
  <rdf:Description rdf:nodeID="A124">
    <owl:qualifiedCardinality rdf:datatype="http://www.w3.org/2001/XMLSchema#nonNegativeInteger">1</owl:qualifiedCardinality>
    <owl:onProperty rdf:resource="#hasAppearance"/>
    <owl:onDataRange rdf:nodeID="A116"/>
    <rdf:type rdf:resource="http://www.w3.org/2002/07/owl#Restriction"/>
  </rdf:Description>
  <rdf:Description rdf:nodeID="A48">
    <owl:onProperty rdf:resource="https://w3id.org/loin/v2/ids#hasRestrictionType"/>
    <owl:cardinality rdf:datatype="http://www.w3.org/2001/XMLSchema#nonNegativeInteger">1</owl:cardinality>
    <rdf:type rdf:resource="http://www.w3.org/2002/07/owl#Restriction"/>
  </rdf:Description>
  <rdf:Description rdf:nodeID="A149">
    <owl:onProperty rdf:resource="#hasDocumentation"/>
    <owl:cardinality rdf:datatype="http://www.w3.org/2001/XMLSchema#nonNegativeInteger">1</owl:cardinality>
    <rdf:type rdf:resource="http://www.w3.org/2002/07/owl#Restriction"/>
  </rdf:Description>
  <rdf:Description rdf:nodeID="A143">
    <owl:onProperty rdf:resource="https://w3id.org/tempo#conceptGUID"/>
    <owl:onDataRange rdf:resource="https://w3id.org/tempo#GUIDType"/>
    <owl:minQualifiedCardinality rdf:datatype="http://www.w3.org/2001/XMLSchema#nonNegativeInteger">0</owl:minQualifiedCardinality>
    <rdf:type rdf:resource="http://www.w3.org/2002/07/owl#Restriction"/>
  </rdf:Description>
  <rdf:Description rdf:nodeID="A13">
    <schema:name>Ruhr University Bochum</schema:name>
    <schema:identifier rdf:resource="https://www.inf.bi.ruhr-uni-bochum.de/iib/lehrstuhl/mitarbeiter/philipp_hagedorn.html.en"/>
  </rdf:Description>
</rdf:RDF>

<!-- Created with TopBraid -->
